\documentclass[handout]{ximera}

\input{../preamble}

\outcome{Differentiate a power series}

\title{3.13 Differentiation of Power Series}

\begin{document}

\begin{abstract}
We differentiate power series term by term.
\end{abstract}

\maketitle



Suppose that the power series 
\[
\sum_{n=0}^\infty a_n x^n
\]
converges for all $x$ in some open interval $I$. Then, on this interval, the power series represents a differentiable function and its derivative is given by 
\[
\frac{d}{dx} \left( \sum_{n=0}^\infty a_n x^n \right) = \sum_{n=0}^\infty  \frac{d}{dx}\big( a_n x^n \big)  
= \sum_{n=1}^\infty   n\cdot a_n x^{n-1}
\]
In other words, the derivative of a power series is a power series. and the derivative is computed term by term, as we would differentiate a polynomial.

\begin{example}[example 1]
Find the derivative of the power series
\[
\sum_{n=0}^\infty x^n
\]
This power series converges on the interval $(-1, 1)$.
On that interval, its derivative is given by
\[
\frac{d}{dx}\left( \sum_{n=0}^\infty x^n \right)= \sum_{n=0}^\infty \frac{d}{dx} \big(x^n\big) = \sum_{n=1}^\infty nx^{n-1}.
\]
We can re-index to rewrite this as
\[
\sum_{n=1}^\infty nx^{n-1} = \sum_{n=0}^\infty (n+1)x^n
\]
We have seen that the original power series above represents the function 
\[
f(x) = \frac{1}{1-x} = \sum_{n=0}^\infty x^n
\]
on the interval $(-1, 1)$. The derivative of this function is
\[
f'(x) = \frac{1}{(1-x)^2} \;\; \text{(verify)}
\]
Thus, we have a power series representation for this function:
\[
\frac{1}{(1-x)^2} = \sum_{n=0}^\infty (n+1)x^n
\]
\end{example}

\begin{remark}
It is possible that the power series representation of the derivative does not converge at an endpoint of the interval of 
convergence of the original function even if the power series representation of original 
function does converge at that endpoint.
\end{remark}

\begin{problem}(problem 1)
Find the derivatives of the following power series. 
Also, compare the interval of convergence of the original series to its derivative.
\[
a) \; \sum_{n=1}^\infty \frac{x^n}{n},\qquad  b) \; \sum_{n=0}^\infty \frac{x^n}{2^n},
\]
\[
 c) \; \sum_{n=0}^\infty \frac{x^n}{n!},\qquad d) \; \sum_{n=0}^\infty x^{2n}
\]
\end{problem}

\end{document}






