\documentclass[handout]{ximera}

\input{../preamble}

\outcome{Find the length of a curve}

\title{2.4 Arc Length}

\begin{document}

\begin{abstract}
We find the length of a curved segment.
\end{abstract}

\maketitle

\section{Arc Length}

\begin{theorem}[Arc Length] The length of the graph of the differentiable function, $y = f(x)$, from $x = a$ to $x = b$, is given by
\[
L = \int_a^b \sqrt{1+ f'(x)^2} \; dx.
\]
\end{theorem}

\begin{example}[example 1]
Find the length of the curve $y = 3x + 2$ from $x = 0$ to $x = 4$. \\
Since the graph of this function is a line, calculus is not required to find the length of the indicated segment.
Instead, we can use the distance formula, 
\[
d = \sqrt{(x_2 - x_1)^2 + (y_2-y_1)^2},
\]
 with the points $(0,2)$ and $(4, 14)$
to get 
\[
d = \sqrt{(4-0)^2 + (14-2)^2} = \sqrt{4^2 + 12^2} = \sqrt{160} = 4\sqrt{10}.
\]
We will also use the formula from the above theorem as a verification that the theorem is correct.
Since $f(x) = 3x+2$, we have $f'(x) = 3$ and the length of the segment is
\[
L = \int_0^4 \sqrt{1 + 3^2} \;dx = \int_0^4 \sqrt{10} \; dx = \sqrt{10}x\bigg|_0^4 = 4\sqrt{10},
\]
as expected.
\end{example}



\begin{problem}(problem 1a)
Find the length of the curve $ y = 2x - 5$ from $x = 2$ to $x = 5$ using the arc length formula.\\

$f'(x) = \answer{2}$\\

$\sqrt{1+f'(x)^2} = \answer{\sqrt{5}}$\\

Arc length = $\answer{3\sqrt{5}}$.
\end{problem}



\begin{problem}(problem 1b)
Find the length of the curve $y = 2x - 5$ from $x = 2$ to $x = 5$ using the distance formula.\\

The endpoints of the line segment are $(2, \answer{-1})$ and $(5, \answer{5})$\\

$d = \sqrt{(x_2 - x_1)^2 + (y_2 - y_1)^2} = \sqrt{(\answer{3})^2 + (\answer{6})^2}$\\

Arc length = $\answer{3\sqrt{5}}$.
\end{problem}




\begin{example}[example 2]
 Find the length of the graph of 
$y = 1+ x^{3/2}$ 
from  $x = 0$ to $x = 4$.\\
First, $f(x) = x^{3/2} + 1$ and so $f'(x) = \frac32 x^{1/2}$. 
Then the arc length is
\[
L = \int_0^4 \sqrt{1 + \left(\frac32 x^{1/2}\right)^2} \; dx = \int_0^4 \sqrt{1 + \frac94 x} \;dx.
\]
To compute this integral, we will use a $u$-substitution with $u = 1+\frac94 x$ and $du = \frac94 \; dx$.
Thus, the anti-derivative is,
\[
\int \sqrt{1+\frac94 x} \; dx = \int \frac49 \sqrt u \; du = \frac49 \cdot \frac23 u^{3/2} + C = \frac{8}{27} \left(1 + \frac94 x \right)^{3/2} + C.
\]

Returning to our computation of arc length, 
\[
L = \frac{8}{27} \left(1 + \frac94 x \right)^{3/2} \bigg|_0^4 = \frac{8}{27} (10^{3/2} - 1).
\]
\end{example}


\begin{problem}(problem 2a)
Find the length of the curve $y = 2 + 4x^{3/2}$ from $x = 0$ to $x = 1$\\

$f'(x) = \answer{6x^{1/2}}$\\

$\sqrt{1+f'(x)^2} = \answer{\sqrt{1+ 36x}}$\\

Arc length = $\answer{\frac{1}{54} (37^{3/2} -1)}$
\end{problem}



\begin{problem}(problem 2b)
Find the length of the curve $y = 3 + 2x^{3/2}$ from $x = 7$ to $x = 11$\\

$f'(x) = \answer{3x^{1/2}}$\\

$\sqrt{1+f'(x)^2} = \answer{\sqrt{1+ 9x}}$\\

Arc length = $\answer{\frac{2}{27} (488)}$
\end{problem}




\begin{example}[example 3] Find the length of the graph of 
$y = \frac{x^3}{12} + \frac{1}{x}$ from $x = 1$ to $x = 2$.\\
In this example, computing a simplified form of the integrand is laborious, so we will proceed slowly.
First, $f(x) = \frac{x^3}{12} + x^{-1}$, so $f'(x) = \frac{x^2}{4} - \frac{1}{x^2}$ and
\[
f'(x)^2 = \left( \frac{x^2}{4} - \frac{1}{x^2} \right)^2 = \frac{x^4}{16} - \frac12 + \frac{1}{x^4}.
\]
Next, we add one:
\[
1 + f'(x)^2 = \frac{x^4}{16} + \frac12 + \frac{1}{x^4},
\]
and the key to this problem is that this expression is a perfect square:
\[
\frac{x^4}{16} + \frac12 + \frac{1}{x^4} = \left( \frac{x^2}{4} + \frac{1}{x^2}\right)^2.
\]
Now, we can compute the square root:
\[
\sqrt{1+f'(x)^2} = \sqrt{\left( \frac{x^2}{4} + \frac{1}{x^2}\right)^2 } = \frac{x^2}{4} + \frac{1}{x^2}.
\]
Finally, we can integrate to get the arc length:
\begin{align*}
L &= \int_1^2 \sqrt{1+f'(x)^2} \; dx \\
  &= \int_1^2 \left(\frac{x^2}{4} + \frac{1}{x^2} \right) \; dx  \\
  &= \int_1^2 \left(\frac{x^2}{4} + x^{-2} \right) \; dx \\
  &= \left(\frac{x^3}{12} + \frac{x^{-1}}{-1} \right) \bigg|_1^2 \\
  &= \left(\frac{x^3}{12} - \frac{1}{x} \right) \bigg|_1^2 \\
  &= \left(\frac23 - \frac12\right) - \left(\frac{1}{12} - 1\right) \\
  &= \frac{13}{12}.  
\end{align*}
\end{example}




\begin{problem}(problem 3a)
Find the length of the curve $\displaystyle{y = \frac{x^4}{4} + \frac{1}{8x^2}}$ from $x = 1$ to $x = 2$\\

$f'(x) = \answer{x^3 - 1/(4x^3)}$\\

$f'(x)^2 =$

\begin{multipleChoice}
\choice{$\displaystyle{x^6 + \frac{1}{16x^6}}$}
\choice{$\displaystyle{x^6 -\frac14 + \frac{1}{16x^6}}$}
\choice[correct]{$\displaystyle{x^6 -\frac12 + \frac{1}{16x^6}}$}
\end{multipleChoice}

$1+f'(x)^2 = \left(\answer{x^3 + \frac{1}{4x^3}}\right)^2$\\

Arc length = $\answer{123/32}$
\end{problem}




\begin{problem}(problem 3b)
Find the length of the curve $\displaystyle{y = \frac{x^2}{8} - \ln(x)}$ from $x = 2$ to $x = 4$\\

$f'(x) = \answer{x/4 - 1/x}$\\

$f'(x)^2 =$

\begin{multipleChoice}
\choice{$\displaystyle{\frac{x^2}{16} + \frac{1}{x^2}}$}
\choice{$\displaystyle{\frac{x^2}{16} -\frac14 + \frac{1}{x^2}}$}
\choice[correct]{$\displaystyle{\frac{x^2}{16} -\frac12 + \frac{1}{x^2}}$}
\end{multipleChoice}

$1+f'(x)^2 = \left(\answer{x/4 + 1/x}\right)^2$\\

Arc length = $\answer{3/2 + \ln 2}$
\end{problem}


\begin{problem}(problem 3c)
Find the length of the curve $y = \ln(\sec(x))$ from $x = 0$ to $x = \pi/4$.

$f'(x) = \answer{\tan(x)}$\\

$1 + f'(x)^2 =$

\begin{multipleChoice}
\choice[correct]{$\sec^2(x)$}
\choice{$\tan^2(x)$}
\choice{$\cos^2(x)$}
\end{multipleChoice}


Arc length = $\answer{\ln(1 + \sqrt 2)}$
\end{problem}



\begin{problem}(problem 3d)
Find the length of the curve $y = \frac{e^x + e^{-x}}{2}$ from $x = 0$ to $x = 1$.

$f'(x) = \answer{\frac{e^x - e^{-x}}{2}}$\\

$1 + f'(x)^2 =$

\begin{multipleChoice}
\choice{$\left(\frac{e^{x} - e^{-x}}{2}\right)^2$}
\choice[correct]{$\left(\frac{e^{x} + e^{-x}}{2}\right)^2$}
\choice{$\left(\frac{e^{x} + e^{-x}}{4}\right)^2$}
\end{multipleChoice}


Arc length = $\answer{\frac{e^2 - 1}{2e}}$
\end{problem}





\section{Video Lesson}


\begin{center}
\begin{foldable}
\unfoldable{Here is a detailed, lecture style video on arc length:}
\youtube{GFXmeteU-_M}
\end{foldable}
\end{center}

\section{Theoretical Justifications}

\begin{image}
\begin{tikzpicture}
\begin{axis}[axis x line=  center, axis y line = center, legend pos =  north west, xmin=-0.5, 
ymin=-0.01, xmax = 3.3, ymax = 2.2, axis equal image, xtick={0.001,1,2,3},ytick={1.414,2},
xticklabels={$x_0=a$,$x_{i-1}$,$x_i$,$b=x_n$}, yticklabels={$f(x_{i-1})$,$f(x_i$)},
title={$L_i = \sqrt{(x_i - x_{i-1})^2 +\left[f(x_i) -f(x_{i-1})\right]^2}$}]
 
\addplot[domain=0:3, samples = 100, color=blue, thick]{2*sin(deg(pi*x/4))}; %node[right] {$y = e^x$};
%\addlegendentry{$y=f(x)$};
\addplot[color=red, thick] coordinates {(0,0) (1,1.414)(2,2)(3,1.414)} ; %y-axis
%\addlegendentry{polygonal path}

\addplot[thin, dashed] coordinates {(1,0) (1,1.414)} ;
\addplot[thin, dashed] coordinates {(2,0) (2,2)} ;
\addplot[<->,thin] coordinates {(1,0.5) (2, 0.5)};
\node at (axis cs:1.5,0.65) {$\Delta x$};



%\addplot[&lt;-&gt;] coordinates {(-1.3,0) (4.3,0)} node[right] {$x$}; %x-axis
%\addplot[thin] coordinates {(1.57,0.1) (1.57, -0.1)} node[below] {$2$};
%\node at (axis cs: 2,2.1){$y = f(x)$};
%\node at (axis cs: 2,-.6){$f(x)$ is continuous at $x = 2$};
%\addplot[smooth,mark=*,blue] plot coordinates {(1.57,1.5)};
 
\end{axis}
\end{tikzpicture}

\end{image}


In this section, we derive the arc length formula.
Suppose $f(x)$ is a differentiable function on the open interval $(a,b)$ and continuous on the 
closed interval $[a,b]$. Let $\Delta x = \frac{b-a}{n}$ and let $x_i = a + i\cdot \Delta x$ for 
$i = 0, 1, 2, 3, \ldots, n$.  Note that $x_0 = a$ and $x_n = a + n \cdot \Delta x = b$.
Next, to approximate the arc length, connect the adjacent points $(x_{i-1}, f(x_{i-1}))$ and
$(x_i, f(x_i))$ with straight line segments for $i = 1, 2, \ldots n.$ From the distance formula,
the length of the $i^{th}$ segment is
\[
L_i = \sqrt{(x_i - x_{i-1})^2 + \left[f(x_i) -f(x_{i-1})\right]^2} 
\]






%which can be rewritten as
%\[
%L_i = (x_i- x_{i-1}) \sqrt{1 + \frac{\left[f(x_i) -f(x_{i-1})\right]^2}{(x_i - x_{i-1})^2}} = 
%\Delta x \cdot \sqrt{1 + \left[ \frac{f(x_i) -f(x_{i-1})}{x_i - x_{i-1}} \right]^2}
%\]
Now, we apply the Mean Value Theorem to $f(x)$ on the interval $[x_{i-1}, x_i]$ to conclude that
\[
f(x_i) -f(x_{i-1})  = f'(x_i^*)(x_i - x_{i-1}) = f'(x_i^*) \cdot \Delta x
\]
for some number $x_i^*$ in the interval $(x_{i -1}, x_i)$. Thus,

\[
L_i = \sqrt{ (\Delta x)^2 + f'(x_i^*)^2 \cdot (\Delta x)^2} = \sqrt{ 1 + f'(x_i^*)^2 }\cdot \Delta x, \; i = 1, 2, \ldots n.
\]

Returning to the arc length, $L$, of $ y = f(x)$ on $[a,b]$, we have
\[
L \approx \sum_{i=1}^n L_i = \sum_{i=1}^n   \sqrt{1 + f'(x_i^*)^2} \cdot \Delta x.
\]
Taking the limit as $n \to \infty$, we define the arc length as 
\[
L = \lim_{n \to \infty} \sum_{i=1}^n   \sqrt{1 + f'(x_i^*)^2} \cdot \Delta x = \int_a^b \sqrt{1 + f'(x)^2} \; dx.
\]



\end{document}








