\documentclass{ximera}

\input{../preamble}

\outcome{Compute integrals involving powers and products of trigonometric functions}

\title{2.2 Trigonometric Integrals}

\begin{document}

\begin{abstract}
We compute integrals involving powers and products of trigonometric functions.
\end{abstract}

\maketitle

\section{Trigonometric Identities}

The following are the Pythagorean Trigonometric Identities 
(named for \link[Pythagoras of Samos]{https://en.wikipedia.org/wiki/Pythagoras}) which hold for all angles,
$\theta$, in the domains of the functions involved:
\[
\sin^2(\theta) + \cos^2(\theta) = 1,
\]
\[
1 + \tan^2(\theta) = \sec^2(\theta),
\]
and
\[
1 + \cot^2(\theta) = \csc^2(\theta).
\]


Next, we have the half-angle formulas:

\[
\sin^2(\theta) = \frac{1-\cos(2\theta)}{2},
\]

and

\[
\cos^2(\theta) = \frac{1+\cos(2\theta)}{2}.
\]
We will find the half-angle formulas useful for integrating even powers of sine and cosine.

\section{Integrating powers of sine and cosine}

In this section, we compute integrals of the form
\[
\int \sin^m(x) \cos^n(x) \; dx
\]
The method we use depends on whether $m$ and $n$ are even or odd.

\subsection{Case 1: $m$ or $n$ is odd}
In this case, the technique involves preparing and performing a $u$-substitution. The key is to use the Pythagorean 
Identity $\sin^2 \theta + \cos^2 \theta = 1$ to convert
sines to cosines or vice-versa.

\begin{example}[example 1]
Compute
\[
\int \sin^4(x) \cos(x) \, dx
\]
This problem is solved using the substitution $u = \sin(x)$, so that $du = \cos(x) \; dx$.
\begin{align*}
\int \sin^4(x) \cos(x) \, dx &= \int u^4 \, du\\
                             &= \frac{u^5}{5} + C\\
                             &= \frac15 \sin^5(x) + C
\end{align*}

\end{example}



\begin{problem}(problem 1a) 
Compute $\displaystyle{\int \sin^6(x)\cos(x) \, dx}$\\

Let $u = \answer{\sin(x)}$, \; then $du = \answer{\cos(x) dx}$.\\

Substituting gives
\[
\int \sin^6(x)\cos(x) \, dx = \int \answer{u^6} \; du
\]

Finally
\[
\int \sin^{6}(x)\cos(x) \, dx = \answer{1/7 \sin^7(x)} + C
\]

\end{problem}



\begin{problem}(problem 1b) 
Compute $\displaystyle{\int \sin(x)\cos^4(x) \, dx}$\\

Let $u = \answer{\cos(x)}$, \; then $du = \answer{-\sin(x) dx}$.\\

Substituting gives 
\[
\int \sin(x)\cos^4(x) \, dx = \int \answer{-u^4} \; du
\]

Finally 
\[
\int \sin(x)\cos^4(x) \, dx = \answer{-1/5 \cos^5(x)} + C
\]

\end{problem}



\begin{problem}(problem 1c)
Compute $\displaystyle{\int \sin^{10}(3x)\cos(3x) \, dx}$\\

Let $u = \answer{\sin(3x)}$, \; then $du = \answer{3\cos(3x) dx}$.\\

Substituting gives 
\[
\int \sin^{10}(3x)\cos(3x) \, dx = \int \answer{\frac13 u^{10}} \; du
\]

Finally
\[
\int \sin^{10}(3x)\cos(3x) \, dx = \answer{\frac{1}{33} \sin^{11}(3x)} + C
\]

\end{problem}



In the next example, we need to prepare for the $u$-substitution. 



\begin{example}[example 2]
Compute $\displaystyle{\int \sin^4(x)\cos^3(x) \; dx}$\\


Prepare for substitution by rewriting the odd power of cosine.
\[
\cos^3(x) = \cos^2(x) \cos(x) = \left[1 - \sin^2(x)\right] \cos(x).
\]

Rewrite the original integral.
\[
\int \sin^4(x)\cos^3(x) \; dx = \int \sin^4(x)\left[1 - \sin^2(x)\right] \cos(x) \; dx
\]
Make the substitution \, $u = \sin(x)$,  \, $du = \cos(x) \, dx$.
\begin{align*}
\int \sin^4(x)\cos^3(x) \; dx &= \int u^4 (1-u^2) \; du\\
   &= \int (u^4 -u^6) \; du\\
  &= \frac{u^5}{5} - \frac{u^7}{7} + C \\
  &= \frac15 \sin^5(x) - \frac17 \sin^7(x) + C
\end{align*}
  
\end{example}



\begin{problem}(problem 2a)
Compute $\displaystyle{\int \sin^6(x)\cos^3(x) \; dx}$\\

Rewrite the odd power of cosine as

\begin{multipleChoice}
\choice{$\cos^3(x) = \left[\sin^2(x)- 1\right] \cos(x)$} 
\choice[correct]{$\cos^3(x) = \left[1 - \sin^2(x)\right] \cos(x)$}
\choice{$\cos^3(x) = \left[1 - \sin(x)\right]^2 \cos(x)$}
\end{multipleChoice}

Next, let $u = \answer{\sin(x)}$ so that $du = \answer{\cos(x) dx}$.\\

Substituting gives 
\[
\int \sin^6(x)\cos^3(x) \; dx= \int \answer{u^6(1-u^2)} \; du
\]

Finally 
\[
\int \sin^6(x)\cos^3(x) \; dx= \answer{\sin^7(x)/7 -  \sin^9(x)/9} + C
\]

\end{problem}



\begin{problem}{\color{gray}(problem 2b)} 
Compute $\displaystyle{\int \sin^3(x)\cos^2(x) \; dx}$\\

Rewrite the odd power of sine as:

\begin{multipleChoice}
\choice{$\sin^3(x) = \left[1 - \cos(x)\right]^2 \sin(x)$}
\choice{$\sin^3(x) = \left[\cos^2(x)- 1\right] \sin(x)$} 
\choice[correct]{$\sin^3(x) = \left[1 - \cos^2(x)\right] \sin(x)$}
\end{multipleChoice}

Next, let $u = \answer{\cos(x)}$ so that $du = \answer{-\sin(x) dx}$.\\

Substituting gives
\[
\int \sin^3(x)\cos^2(x) \; dx= \int \answer{-u^2(1-u^2)} \; du.
\]

Finally
\[
\int \sin^3(x)\cos^2(x) \; dx= \answer{\cos^5(x)/5 - \cos^3(x)/3} + C.
\]

\end{problem}



\begin{problem}{\color{gray}(problem 2c)}
Compute $\displaystyle{\int 3\sin^8(2x)\cos^3(2x) \; dx}$\\

Rewrite the odd power of cosine as:

\begin{multipleChoice}
\choice[correct]{$\cos^3(2x) = \left[1 - \sin^2(2x)\right] \cos(2x)$}
\choice{$\cos^3(2x) = \left[\sin^2(2x)- 1\right] \cos(2x)$} 
\choice{$\cos^3(2x) = \left[1 - \sin(2x)\right]^2 \cos(2x)$}
\end{multipleChoice}

Next, let $u = \answer{\sin(2x)}$ so that $du = \answer{2\cos(2x) dx}$.\\

Substituting gives
\[
\int 3\sin^8(2x)\cos^3(2x) \; dx= \int \answer{3/2 u^8(1-u^2)} \; du
\]

Finally
\[
\int 3\sin^8(2x)\cos^3(2x) \; dx= \answer{\frac16 \sin^9(2x)- \frac{3}{22} \sin^{11}(2x)} + C
\]
\end{problem}


\begin{problem}(problem 2d)
Compute $\displaystyle{\int \cos^3(4x) \; dx}$\\

Rewrite the odd power of cosine as:

\begin{multipleChoice}
\choice{$\cos^3(4x) = \left[\sin^2(4x)- 1\right] \cos(4x)$} 
\choice[correct]{$\cos^3(4x) = \left[1 - \sin^2(4x)\right] \cos(4x)$}
\choice{$\cos^3(4x) = \left[1 - \sin(4x)\right]^2 \cos(4x)$}
\end{multipleChoice}

Next, let $u = \answer{\sin(4x)}$ so that $du = \answer{4\cos(4x) dx}$.\\

Substituting gives
\[
\int \cos^3(4x) \; dx= \int \answer{1/4 (1-u^2)} \; du
\]

Finally
\[
\int \cos^3(4x) \; dx= \answer{\frac14 \sin(4x) - \frac{1}{12} \sin^3(4x) } + C
\]

\end{problem}





\begin{example}[example 3]
Compute $\displaystyle{\int \sin^8(x)\cos^5(x) \; dx}$\\

Prepare for substitution by rewriting the odd power of cosine.
\[
\cos^5(x) = \cos^4(x) \cos(x) = \left[1 - \sin^2(x)\right]^2 \cos(x).
\]

Rewrite the original integral.
\[
\int \sin^8(x)\cos^5(x) \; dx = \int \sin^8(x)\left[1 - \sin^2(x)\right]^2 \cos(x) \; dx.
\]

Make the substitution $u = \sin(x), \; du = \cos(x) \, dx$.
\begin{align*}
\int \sin^8(x)\cos^5(x) \; dx &= \int u^8 (1-u^2)^2 \; du\\
   &= \int u^8 (1-2u^2 + u^4) \; du\\
   &= \int (u^8 -2u^{10} + u^{12}) \; du\\
  &= \tfrac19 u^9 - \tfrac{2}{11}u^{11} + \tfrac{1}{13} u^{13} + C \\
  &= \tfrac19 \sin^9(x) - \tfrac{2}{11} \sin^{11}(x)  + \tfrac{1}{13} \sin^{13}(x) + C.
\end{align*}
  
\end{example}



\begin{problem}(problem 3a) 
Compute $\displaystyle{\int \sin^5(x)\cos^6(x) \; dx}$\\

Rewrite the odd power of sine as:

\begin{multipleChoice}
\choice{$\sin^5(x) = \left[1 - \cos^4(x)\right] \sin(x)$}
\choice{$\sin^5(x) = \left[1 + \cos^4(x)\right] \sin(x)$} 
\choice[correct]{$\sin^5(x) = \left[1 - 2\cos^2(x) + \cos^4(x)\right] \sin(x)$}
\end{multipleChoice}

Next, let $u = \answer{\cos(x)}$ so that $du = \answer{-\sin(x) dx}$.\\

Substituting gives
\[
\int \sin^5(x)\cos^6(x) \; dx= \int \answer{-u^6(1-2u^2 + u^4)} \; du
\]

Finally
\[
\int \sin^5(x)\cos^6(x) \; dx= \answer{-1/7 \cos^7(x) + 2/9 \cos^9(x) - 1/11 \cos^{11}(x)} + C
\]

\end{problem}



\begin{problem}{\color{gray}(problem 3b)} 
Compute $\displaystyle{\int \sin^2(6x)\cos^5(6x) \; dx}$\\

Rewrite the odd power of cosine as:

\begin{multipleChoice}
\choice[correct]{$\cos^5(6x) = \left[1 - 2\sin^2(6x) + \sin^4(6x)\right] \cos(6x)$}
\choice{$\cos^5(6x) = \left[1 - \sin^4(6x)\right] \cos(6x)$}
\choice{$\cos^5(6x) = \left[1 + \sin^4(6x)\right] \cos(6x)$} 
\end{multipleChoice}

Next, let $u = \answer{\sin(6x)}$ so that $du = \answer{6 \cos(x) dx}$.\\

Substituting gives
\[
\int \sin^2(6x)\cos^5(6x) \; dx= \int \answer{1/6 u^2(1-2u^2 + u^4)} \; du
\]

Finally
\[
\int \sin^2(6x)\cos^5(6x) \; dx= \answer{1/18 \sin^3(6x) - 1/15 \sin^5(6x) + 1/42 \sin^7(6x)} + C
\]
\end{problem}



\begin{problem}{\color{gray}(problem 3c)} 
Compute $\displaystyle{\int \sin^5(x) \; dx}$\\

Rewrite the odd power of sine as:

\begin{multipleChoice}
\choice{$\sin^5(x) = \left[1 - \cos^4(x)\right] \sin(x)$}
\choice{$\sin^5(x) = \left[1 + \cos^4(x)\right] \sin(x)$} 
\choice[correct]{$\sin^5(x) = \left[1 - 2\cos^2(x) + \cos^4(x)\right] \sin(x)$}
\end{multipleChoice}

Next, let $u = \answer{\cos(x)}$ so that $du = \answer{-\sin(x) dx}$.\\

Substituting gives
\[
\int \sin^5(x) \; dx= \int \answer{-(1-2u^2 + u^4)} \; du
\]

Finally
\[
\int \sin^5(x) \; dx= \answer{- \cos(x) + 2/3 \cos^3(x) - 1/5 \cos^5(x)} + C
\]

\end{problem}

In the next example, both powers are odd.  In this case, we have to choose which one to rewrite.



\begin{example}[example 4]
Compute $\displaystyle{\int \sin^7(x)\cos^5(x) \; dx}$\\

Prepare for substitution by rewriting the smaller odd power.
\[
\cos^5(x) = \cos^4(x) \cos(x) = \left[1-\sin^2(x)\right]^2 \cos(x).
\]

Rewrite the original integral.
\[
\int \sin^7(x)\cos^5(x) \; dx = \int \sin^7(x)\left[1 - \sin^2(x)\right]^2 \cos(x) \; dx.
\]

Make the substitution $u = \sin(x), \; du = \cos(x) \, dx$.
\begin{align*}
\int \sin^7(x)\cos^5(x) \; dx  &= \int u^7 (1-u^2)^2 \; du\\
   &= \int u^7(1 - 2u^2 + u^4) \; du\\
   &= \int (u^7 - 2u^9 + u^{11}) \; du\\
  &= \tfrac18 u^8 - \tfrac15 u^{10} + \tfrac{1}{12}u^{12}+ C \\
  &= \tfrac18 \sin^8(x) - \tfrac15 \sin^{10}(x) + \tfrac{1}{12} \sin^{12}(x)+ C
\end{align*}

\end{example}





\begin{problem}{\color{gray}(problem 4a)}
Compute $\displaystyle{\int \sin^5(x)\cos^7(x) \; dx}$

Which trig function should be rewritten?

\begin{multipleChoice}
\choice[correct]{$\sin^5(x)$}
\choice{$\cos^7(x)$}
\end{multipleChoice}

Rewrite the odd power of sine as:
\begin{multipleChoice}
\choice{$\sin^5(x) = \left[1 - \cos^4(x)\right] \sin(x)$}
\choice{$\sin^5(x) = \left[\cos^4(x)- 1\right] \sin(x)$} 
\choice[correct]{$\sin^5(x) = \left[1 - 2\cos^2(x) + \cos^4(x)\right] \sin(x)$}
\end{multipleChoice}

Next, let $u = \answer{\cos(x)}$ so that $du = \answer{-\sin(x) dx}$.\\

Substituting gives
\[
\int \sin^5(x)\cos^7(x) \; dx= \int \answer{-(1-2u^2 + u^4)u^7} \; du
\]

Finally
\[
\int \sin^5(x)\cos^7(x) \; dx= \answer{-\cos^8(x)/8 + \cos^{10}(x)/5 - \cos^{12}(x)/12} + C
\]
\end{problem}



\begin{problem}(problem 4b)
Compute $\displaystyle{\int \sin^9(x)\cos^3(x) \; dx}$\\

Which trig function should be rewritten?
\begin{multipleChoice}
\choice{$\sin^9(x)$}
\choice[correct]{$\cos^3(x)$}
\end{multipleChoice}

Rewrite the odd power of cosine as:
\begin{multipleChoice}
\choice{$\cos^3(x) = \left[\sin^2(x)- 1\right] \cos(x)$} 
\choice[correct]{$\cos^3(x) = \left[1 - \sin^2(x)\right] \cos(x)$}
\choice{$\cos^3(x) = \left[1 - \sin(x)\right]^2 \cos(x)$}
\end{multipleChoice}

Next, let $u = \answer{\sin(x)}$ so that $du = \answer{\cos(x) dx}$.\\

Substituting gives
\[
\int \sin^9(x)\cos^3(x) \; dx= \int \answer{u^9(1 - u^2)} \; du
\]

Finally
\[
\int \sin^9(x)\cos^3(x) \; dx= \answer{\sin^{10}(x)/(10) - \sin^{12}(x)/(12) } + C
\]
\end{problem}




\subsection{Case 2: $m$ and $n$ are both even}
In this section, we compute integrals of the form
\[
\int \sin^m(x) \cos^n(x) \; dx
\]
where $m$ and $n$ are both even.\\
We will use the half-angle formulas
\[
\sin^2 \theta = \frac{1 - \cos 2\theta}{2} \; \text{and} \; \cos^2 \theta = \frac{1 + \cos 2\theta}{2}
\]

\begin{example}[example 5]
Compute $\displaystyle{\int \sin^2(x) \; dx}$

Rewrite the integral using a half-angle formula.

\begin{align*}
\int \sin^2(x) \; dx &= \int \left[\frac12- \frac12\cos(2x)\right]  \; dx\\
  &= \frac{x}{2}  - \frac{1}{4}\sin(2x) + C.
\end{align*}
\end{example}

\begin{problem}(problem 5)
Compute $\displaystyle{\int \cos^2(x) \; dx}$
\begin{multipleChoice}
\choice[correct]{$\frac{x}{2}  + \frac{1}{4}\sin(2x) + C$} 
\choice{$\frac{x}{2}  - \frac{1}{4}\cos(2x) + C$}
\choice{$\frac{x}{2}  + \frac{1}{4}\cos(2x) + C$}
\end{multipleChoice}
\end{problem}

\begin{example}[example 6]
Compute the indefinite integral:
\[
\int \sin^4(x) \; dx.
\]
Rewrite the integral using the half-angle formula for sine.

\begin{align*}
\int \sin^4(x) \; dx &= \int \left[\tfrac12- \tfrac12\cos(2x)\right] \cdot \left[\tfrac12 - \tfrac12\cos(2x)\right] \; dx\\
  &=  \int \left[\tfrac14 - \tfrac12\cos(2x) + \tfrac14\cos^2(2x)\right] \; dx \\
  &= \int \left( \tfrac14 - \tfrac12 \cos(2x) + \tfrac14 
  \left[\tfrac12 + \tfrac12\cos(4x)\right]\right) \; dx  \;\; \textup{(half-angle again)} \\
  &= \int \left[\tfrac14 - \tfrac12 \cos(2x) +\tfrac18 + \tfrac18\cos(4x)\right] \; dx\\
  &=  \int \left[\tfrac38 - \tfrac12 \cos(2x) + \tfrac18\cos(4x)\right] \; dx \;\; \textup{(now we can integrate)}\\
  &= \tfrac38 x - \tfrac14 \sin(2x) + \tfrac{1}{32}\sin(4x) + C.
\end{align*}
\end{example}




\begin{problem}(problem 6a)
Compute $\displaystyle{\int \cos^4(x) \; dx}$


Use a half angle formula to rewrite: $\cos^4(x)=$

\begin{multipleChoice}
\choice{$\tfrac14  + \tfrac14\cos^2(2x)$}
\choice{$\tfrac14 - \tfrac12\cos(2x) + \tfrac14\cos^2(2x)$}
\choice[correct]{$\tfrac14 + \tfrac12\cos(2x) + \tfrac14\cos^2(2x)$}
\end{multipleChoice}

Use a half angle formula again to obtain, $\cos^4(x) = $

\begin{multipleChoice}
\choice{$\tfrac18 + \tfrac12\cos(2x) + \tfrac18 \cos(4x)$}
\choice{$\tfrac14 + \tfrac12\cos(2x) + \tfrac18 \cos(4x)$}
\choice[correct]{$\tfrac38 + \tfrac12\cos(2x) + \tfrac18 \cos(4x)$}
\end{multipleChoice}

Finally,
\[
\int \cos^4(x) \; dx = \answer{\frac{3x}{8} +\frac14 \sin(2x) + \frac{1}{32}\sin(4x)} + C
\]
\end{problem}



\begin{problem}(problem 6b)
Compute $\displaystyle{\int \sin^2(3x)\cos^2(3x) \; dx}$


Use the half angle formulas to rewrite: $\sin^2(3x) \cos^2(3x)=$

\begin{multipleChoice}
\choice{$\tfrac14 + \tfrac14\cos^2(6x)$}
\choice{$\tfrac14 - \tfrac14\sin^2(6x)$}
\choice[correct]{$\tfrac14 - \tfrac14\cos^2(6x)$}
\end{multipleChoice}

Use a half angle formula again to obtain, $\sin^2(3x) \cos^2(3x)=$

\begin{multipleChoice}
\choice{$\tfrac38  - \tfrac18 \cos(12x)$}
\choice{$\tfrac18  + \tfrac18 \cos(12x)$}
\choice[correct]{$\tfrac18  - \tfrac18 \cos(12x)$}
\end{multipleChoice}

Finally,
\[
\int \sin^2(3x)\cos^2(3x) \; dx = \answer{\frac18 x - \frac{1}{96} \sin(12x)} + C.
\]

\end{problem}


%Rewrite the integral using the half-angle formulas.

%\begin{align*}
%\int \sin^2(x)\cos^2(x) \; dx &= \int \left[\tfrac12- \tfrac12\cos(2x)\right] \cdot \left[\tfrac12 + \tfrac12\cos(2x)\right] \; dx\\
%  &=  \int \left[\tfrac14 - \tfrac14\cos^2(2x)\right] \; dx \\
%  &= \int \left( \tfrac14 - \tfrac14 \left[\tfrac12 + \tfrac12\cos(4x)\right]\right) \; dx  \;\; \textup{(half-angle again)} \\
%  &= \int \left[\tfrac14 -\tfrac18 - \tfrac18\cos(4x)\right] \; dx\\
%  &=  \int \left[\tfrac18 - \tfrac18\cos(4x)\right] \; dx \;\; \textup{(now we can integrate)}\\
%  &= \tfrac18 x  - \tfrac{1}{32}\sin(4x) + C.
%\end{align*}
%\end{example}



\section{Powers of Secant and Tangent}
In this section, we compute integrals of the form
\[
\int \sec^m(x)\tan^n(x) \; dx,
\]
where either $m$ is odd or $n$ is even. We will use the identity
\[
1+\tan^2 \theta = \sec^2 \theta
\]
to prepare a $u$-substitution.


\subsection{Case 1: $m$ is even}
\begin{example}[example 7]
Compute $\displaystyle{\int \tan^4(x) \sec^2(x)\;dx}$

Make the substitution $u = \tan(x), \; du = \sec^2(x) \, dx$.

\begin{align*}
\int \tan^4(x) \sec^2(x)\;dx &= \int u^4 du\\
&=  \frac{u^5}{5} + C  \\
&= \frac15\tan^5(x)  + C
\end{align*}
\end{example} 



\begin{example}[example 8]
Compute $\displaystyle{\int \tan^4(x) \sec^6(x)\;dx}$

Prepare for $u$-substitution by rewriting the even power of secant.
\[
\sec^6(x) = \sec^4(x) \sec^2(x) = \left[1+\tan^2(x)\right]^2 \sec^2(x)
\]

Rewrite the original integral.

\[
\int \tan^4(x) \sec^6(x)\;dx = \int \tan^4(x) \left[1+\tan^2(x)\right]^2 \sec^2(x) \; dx
\]

Make the substitution $u = \tan(x), \; du = \sec^2(x) \, dx$.


\begin{align*}
\int \tan^4(x) \sec^6(x)\;dx &= \int u^4 (1+u^2)^2 du\\
&= \int u^4(1+2u^2 + u^4) \; du \\
&= \int (u^4 + 2u^6 + u^8) \; du \\
&=  \tfrac15 u^5 + \tfrac27 u^7 + \tfrac19 u^9 + C  \\
&= \tfrac15\tan^5(x)  + \tfrac27 \tan^7(x) + \tfrac19 \tan^9(x) + C
\end{align*}
\end{example} 



\begin{problem}(problem 8a)
Compute the indefinite integral:
\[
\int \tan^6(x) \sec^4(x)\;dx = \answer{\frac17 \tan^7(x) + \frac19 \tan^9(x)} + C.
\]
\end{problem}

\begin{problem}(problem 8b)
Compute the indefinite integral:
\[
\int \tan^{1/3}(x) \sec^4(x)\;dx = \answer{\frac34 \tan^{4/3}(x) + \frac{3}{10} \tan^{10/3}(x)} + C.
\]
\end{problem}

\begin{problem}(problem 8c)
Compute the indefinite integral:
\[
\int  \sec^4(3x)\;dx = \answer{\frac13 \tan(3x) + \frac19 \tan^3(3x)} + C.
\]
\end{problem}


\subsection{Case 2: $n$ is odd}


\begin{example}[example 9]

Compute
\[
\int \sec^5(x) \tan(x) \, dx.
\]
To find an anti-derivative, we will make the substitution $u = \sec(x)$, as it is the inside of a composition
and its differential, $du = \sec(x)\tan(x) \, dx$, is present as a factor. 
This substitution transforms the original integral as follows:
\[
\int \sec^5(x) \tan(x) \, dx = \int \sec^4(x) \sec(x) \tan(x) \, dx= \int u^4 \, du,
\]
which is an integral that can be computed from the power rule giving
\begin{align*}
\int \sec^5(x) \tan(x) \, dx &= \int \sec^4(x) \sec(x) \tan(x) \, dx\\
                             &= \int u^4 \, du\\
                             &= \frac{u^5}{5} + C\\
                             &= \frac15 \sec^5(x) + C.
\end{align*}

\end{example}



\begin{example}[example 10]
Compute the indefinite integral:
\[
\int \tan^5(x) \sec^3(x)\;dx.
\]
When $n$ is odd, we use the substitution $u = \sec(x)$,
which implies $du = \sec(x) \tan(x) \; dx$ or $dx = \frac{du}{\sec(x)\tan(x)}$.
We begin by just substituting for $dx$:
\begin{align*}
\int \tan^5(x) \sec^3(x)\;dx &= \int \tan^5(x) \sec^3(x) \frac{du}{\sec(x)\tan(x)}\\
&= \int \tan^4(x) \sec^2(x) \; du & \text{(cancelling)}\\
&= \int \tan^4(x) u^2 \; du & \text{(use Pythagorean identity)}\\
&= \int \left[\tan^2(x)\right]^2 u^2 \; du \\
&= \int \left[\sec^2(x) -1\right]^2 u^2 \; du \\
&= \int \left(u^2 -1\right)^2 u^2 \; du \\
&= \int \left(u^4 - 2u^2 +1\right) u^2 \; du & \text{(distribute $u^2$)}\\
&= \int \left(u^6 - 2u^4 +u^2\right) \; du & \text{(now integrate)}\\
&=  \frac{u^7}{7} - \frac{2u^5}{5} + \frac{u^3}{3} + C  \\
&= \frac17\sec^7(x) - \frac25 \sec^5(x) + \frac13 \sec^3(x) + C & \text{(back substituting)}
\end{align*}
\end{example}

\begin{problem}
Compute the indefinite integral:
\[
\int \tan^3(x) \sec^5(x)\;dx = \answer{\frac17 \sec^7(x) - \frac15 \sec^5(x)} + C.
\]
\end{problem}

\begin{problem}
Compute the indefinite integral:
\[
\int \tan^5(x) \sec^7(x)\;dx = \answer{\frac{1}{11} \sec^{11}(x) + \frac17 \sec^7(x) -\frac29 \sec^9(x)} + C.
\]
\end{problem}





\section{Odd Powers of Secant}
\begin{example}
Compute the indefinite integral:
\[
\int \sec(x) \; dx.
\]
This integral is computed by using a $u$-substitution after rewriting the integrand
by multiplying by 1 in the following way:
\[
\int \sec(x) \; dx = \int \sec(x) \cdot \frac{\sec(x) + \tan(x)}{\sec(x) + \tan(x)} \; dx.
\]
After distributing $\sec(x)$ we get
\[
\int \sec(x) \; dx = \int \frac{\sec^2(x) + \sec(x)\tan(x)}{\sec(x) + \tan(x)} \; dx.
\]
Now we observe that the numerator is the derivative of the denominator which suggests the substitution
$u = \sec(x) + \tan(x)$. We have $du = [ \sec(x)\tan(x) + \sec^2(x)] \; dx$ and the integral becomes
\begin{align*}
\int \sec(x) \; dx &= \int \frac{\sec^2(x) + \sec(x)\tan(x)}{\sec(x) + \tan(x)} \; dx\\
&= \int \frac{1}{u} \; du\\
&= \ln|u| + C\\
&= \ln|\sec(x) + \tan(x)|.
\end{align*}

\end{example}

%The integral of $\sec^3(x)$ was handled in the Integration by parts section
%yielding
%\[
%\int \sec^3(x) \; dx = \frac12 \sec(x) \tan(x) + \frac12 \ln|\sec(x) + \tan(x)| + C.
%\]
Furthermore, IBP also gave a reduction formula for higher powers of $\sec(x)$:
\[
\int \sec^n(x) \; dx =  \frac{1}{n-1}\sec^{n-2}(x)\tan(x) + \frac{n-2}{n-1}\int \sec^{n-2}(x) \; dx. 
\]
This formula is particularly useful if
the power is odd, since if $n$ is odd, $n-2$ is also odd.  Therefore, if we repeat the formula enough times, 
we will eventually be left with $\int \sec(x) \, dx$
which we have just solved.

\begin{example}
Use the above reduction of powers formula twice to compute the indefinite integral
\[
\int \sec^5(x) \; dx.
\]
We have $n =5$, and the formula gives
\[
\int \sec^5(x) \; dx = \frac14 \sec^3(x)\tan(x) + \frac34 \int \sec^3(x) \; dx.
\]
We will use the reduction of powers formula once again, this time with $n=3$:
\begin{align*}
\int \sec^5(x) \; dx &= \frac14 \sec^3(x)\tan(x) + \frac34 \int \sec^3(x) \; dx\\
&= \frac14 \sec^3(x)\tan(x) + \frac34\left(\frac12\sec(x)\tan(x) + \frac12\int \sec(x) \; dx\right)\\
&=\frac14 \sec^3(x)\tan(x) + \frac38\sec(x)\tan(x) + \frac38 \int \sec(x) \; dx \\
&=\frac14 \sec^3(x)\tan(x) + \frac38\sec(x)\tan(x) + \frac38\ln|\sec(x) + \tan(x)| + C
\end{align*}
\end{example}



%\begin{center}
%\begin{foldable}
%\unfoldable{Here is a video of Example 1}
%\youtube{Yy6QXnFlnXs} %vid of example 1
%\end{foldable}
%\end{center}





\begin{center}
\begin{foldable}
\unfoldable{Here are two detailed, lecture style videos on trigonometric integrals:}
\youtube{qbRIlTVP_2E}
\youtube{G0R-dItF4EA}
\end{foldable}
\end{center}





\end{document}


\begin{example} %example #15
Find $h'(x)$ if $h(x) = x^{\sin(x)}$.\\
We will use the fact that the exponential and logarithm functions are inverses,
\[e^{\ln(x)} = x,\]
and the exponent property of logarithms, 
\[\ln(x^n) = n\ln(x),\]
to rewrite $h(x)$.  We have 
\[h(x) = x^{\sin(x)} = e^{\ln(x^{\sin(x)})} = e^{\sin(x)\ln(x)}\]
and we can now compute $h'(x)$ using a combination of the chain rule and product rule.
We can write $h(x)$ as a composition, $f(g(x))$ with 
\[g(x) = \sin(x)\ln(x) \quad \text{and} \quad f(x) = e^x.\]
Then to find $g'(x)$ we us the product rule and we get $g'(x) = \frac{\sin(x)}{x} + \cos(x)\ln(x)$.
Next $f'(x) = e^x$ and 
hence $f'(g(x)) = e^{g(x)} = e^{\sin(x)\ln(x)} = x^{\sin(x)}$.
We can then conclude $h'(x) = f'(g(x))g'(x) = x^{\sin(x)} \left[ \frac{\sin(x)}{x} + \cos(x)\ln(x)\right]$.
\end{example}

%more question formats below













%\begin{verbatim}
\begin{question}
What is your favorite color?
\begin{multipleChoice}
\choice[correct]{Rainbow}
\choice{Blue}
\choice{Green}
\choice{Red}
\end{multipleChoice}
\begin{freeResponse}
Hello
\end{freeResponse}
\end{question}
%\end{verbatim}





\begin{question}
  Which one will you choose?
  \begin{multipleChoice}
    \choice[correct]{I'm correct.}
    \choice{I'm wrong.}
    \choice{I'm wrong too.}
  \end{multipleChoice}
\end{question}


\begin{question}
  Which one will you choose?
  \begin{selectAll}
    \choice[correct]{I'm correct.}
    \choice{I'm wrong.}
    \choice[correct]{I'm also correct.}
    \choice{I'm wrong too.}
  \end{selectAll}
\end{question}


\begin{freeResponse}
What is the chain rule used for?
\end{freeResponse}
