\documentclass[handout]{ximera}
\usepackage{tcolorbox}
\input{../preamble}

\outcome{Compute the derivative of a product.}

\title{2.5 Product Rule}


\begin{document}

\begin{abstract}
We compute the derivative of a product.
\end{abstract}

\maketitle


\begin{center}
\bf{The Product Rule}
\end{center}


\[[f(x) \cdot g(x)]' = f'(x)g(x) + f(x)g'(x)\]

In words, the derivative of a product is the derivative of the first times the second plus the first 
times the derivative of the second.\\

\begin{example}[example 1]
Find 
\[
\frac{d}{dx} [(x^2 + 5x+3)(x^3 - 6x^2 -7)]
\]

Use the product rule with 
\[
f(x) = x^2 + 5x+3
\]
and
\[
g(x) = x^3 -6x^2 -7.
\]
With these choices, we have
\[
f'(x) = 2x + 5
\]
and 
\[
g'(x) = 3x^2 - 12x.
\]
The product rule then gives
\[
\frac{d}{dx} [(x^2 + 5x+3)(x^3 - 6x^2 -7)]\\
=(2x+5)(x^3-6x^2 -7) + (x^2 + 5x+3)(3x^2 -12x).
\]
\end{example}


\begin{problem} (problem 1)
  Compute
  \[
  \frac{d}{dx}[(x^2 - 3x +1)(x^3 + 4x^2 -2)]
  \]
  
    \begin{hint}
      Use the Product Rule with $x^2 -3x+1$ and $x^3 +4x^2-2$.
    \end{hint}
    \begin{hint}
      $(fg)' = f'g+g'f$.
    \end{hint}
    \begin{hint}
      The derivative of $x^2 -3x+1$ is $2x-3$
    \end{hint}
    \begin{hint}
      The derivative of $x^3 + 4x^2 -2$ is $3x^2 +8x$
    \end{hint}
    
		The derivative of $(x^2 - 3x +1)(x^3 + 4x^2 -2)$ with respect to $x$ is
		 $\answer{(2x-3)(x^3+4x^2-2)+(x^2-3x+1)(3x^2+8x)}$
		
\end{problem}




\begin{example}[example 2]
Find 
\[
\frac{d}{dx} x^3e^x
\]

Use the product rule with 
\[
f(x) = x^3
\]
and
\[
g(x) = e^x.
\]
With these choices, we have
\[
f'(x) = 3x^2
\]
and 
\[
g'(x) = e^x.
\]
The product rule then gives
\[
\frac{d}{dx}x^3e^x = 3x^2e^x + x^3e^x\\
=(x^3 + 3x^2)e^x.
\]
\end{example}

\begin{problem}(problem 2)
  Compute
  \[
  \frac{d}{dx} \sqrt x e^x
  \]
  
    \begin{hint}
      Use the Product Rule with $\sqrt x$ and $e^x$.
    \end{hint}
    \begin{hint}
      $(fg)' = f'g+g'f$.
    \end{hint}
    \begin{hint}
      The derivative of $\sqrt x$ is $\frac{1}{2\sqrt x}$
    \end{hint}
    \begin{hint}
      The derivative of $e^x$ is $e^x$
    \end{hint}
    
		The derivative of $\sqrt x e^x$ with respect to $x$ is
		 $\answer{(\sqrt x + 1/(2\sqrt x))e^x}$
		
\end{problem}




\begin{example}[example 3]
Find $h'(x)$ if $h(x) = x^3\sin(x)$.\\
We write $h(x)$ as a product: $h(x) = f(x)\cdot g(x)$ with 
\[f(x) = x^3 \quad \text{and} \quad g(x) = \sin(x).\]
To use the product rule, we need the derivatives:
\[f'(x) = 3x^2 \quad \text{and} \quad g'(x) = \cos(x).\]
We can now write the derivative:
\begin{align*}
h'(x) &= f'(x)g(x) + f(x)g'(x) \\
&= 3x^2\sin(x) + x^3\cos(x).
\end{align*}
\end{example}

\begin{center}
\begin{foldable}
\unfoldable{Here is a video of the preceding example}
\youtube{1BEIrnZ_OkU} %vid of example 1
\end{foldable}
\end{center}



\begin{problem}(problem 3a)
  Compute
  \[
  \frac{d}{dx} x^4\sin(x)
  \]
  
    \begin{hint}
      Use the Product Rule with $x^4$ and $\sin(x)$.
    \end{hint}
    \begin{hint}
      $(fg)' = f'g+g'f$.
    \end{hint}
    \begin{hint}
      The derivative of $x^4$ is $4x^3$
    \end{hint}
    \begin{hint}
      The derivative of $\sin(x)$ is $\cos(x)$
    \end{hint}
    
		The derivative of $x^4\sin(x)$ with respect to $x$ is
		 $\answer{4x^3\sin(x) + x^4\cos(x)}$
		
\end{problem}


\begin{problem}(problem 3b)
  Compute
  \[
  \frac{d}{dx} 2\sqrt x\sin(x)
  \]
  
    \begin{hint}
      Use the Product Rule with $2\sqrt x$ and $\sin(x)$.
    \end{hint}
    \begin{hint}
      $(fg)' = f'g+g'f$.
    \end{hint}
    \begin{hint}
      The derivative of $2\sqrt x$ is $\frac{1}{\sqrt x}$
    \end{hint}
    \begin{hint}
      The derivative of $\sin(x)$ is $\cos(x)$
    \end{hint}
    
		The derivative of $2\sqrt x\sin(x)$ with respect to $x$ is
		 $\answer{\frac{\sin(x)}{\sqrt x} + 2\sqrt x\cos(x)}$
		
\end{problem}


\begin{example}[example 4]
Find $h'(x)$ if $h(x) = 3x^5\cos(x)$.\\
We write $h(x)$ as a product: $h(x) = f(x)\cdot g(x)$ with
 \[f(x) = 3x^5 \quad \text{and} \quad g(x) = \cos(x).\] 
To use the product rule, we need the derivatives
\[f'(x) = 15x^4 \quad \text{and} \quad g'(x) = -\sin(x).\] 
We can now write the derivative:
\begin{align*}
h'(x) &= f'(x)g(x) + f(x)g'(x)\\
&=  15x^4 \cos(x) +3x^5(-\sin(x)) \\
&= 15x^4 \cos(x) - 3x^5\sin(x).
\end{align*}
\end{example}


\begin{center}
\begin{foldable}
\unfoldable{Here is a video of the preceding example}
\youtube{3Ka_23hiuXc} %vid of example 2
\end{foldable}
\end{center}


\begin{problem}(problem 4a)
  Compute
  \[
  \frac{d}{dx} x^5\cos(x)
  \]
  
    \begin{hint}
      Use the Product Rule with $x^5$ and $\cos(x)$.
    \end{hint}
    \begin{hint}
      $(fg)' = f'g+g'f$.
    \end{hint}
    \begin{hint}
      The derivative of $x^5$ is $5x^4$
    \end{hint}
    \begin{hint}
      The derivative of $\cos(x)$ is $-\sin(x)$
    \end{hint}
    
		The derivative of $x^5\cos(x)$ with respect to $x$ is
		 $\answer{5x^4\cos(x) - x^5\sin(x)}$
		
\end{problem}



\begin{problem}(problem 4b)
  Compute
  \[
  \frac{d}{dx} \sqrt[3]x \cos(x)
  \]
  
    \begin{hint}
      Use the Product Rule with $\sqrt[3] x$ and $\cos(x)$.
    \end{hint}
    \begin{hint}
      $(fg)' = f'g+g'f$.
    \end{hint}
    \begin{hint}
      The derivative of $\sqrt[3]x$ is $\frac{1}{3\sqrt[3]x^2}$
    \end{hint}
    \begin{hint}
      The derivative of $\cos(x)$ is $-\sin(x)$
    \end{hint}
    
		The derivative of $\sqrt[3]x\cos(x)$ with respect to $x$ is
		 $\answer{-x^{1/3}\sin(x) + (1/3)x^{-2/3}\cos(x)}$
		
\end{problem}


\begin{example}[example 5]
Find $h'(x)$ if $h(x) = (x^2 - 5x - 2)e^x$.\\
We write $h(x)$ as a product: $h(x) = f(x) \cdot g(x)$ with
\[f(x) = x^2 - 5x -2 \quad \text{and} \quad g(x) = e^x.\]
To use the product rule, we need the derivatives:
\[f'(x) = 2x - 5 \quad \text{and} \quad g'(x)= e^x.\]
We can now write the derivative:
\begin{align*}
h'(x) &= f'(x)g(x) + f(x)g'(x) \\
&= (2x - 5)e^x+ (x^2 - 5x - 2)e^x  \\
&= (x^2 - 5x - 2 + 2x - 5)e^x \\
&= (x^2 - 3x - 7)e^x.
\end{align*}
\end{example}


\begin{center}
\begin{foldable}
\unfoldable{Here is a video of the preceding example}
\youtube{DaVxKhW7ZGY} %vid of example 3
\end{foldable}
\end{center}


\begin{problem}(problem 5)
  Compute
  \[
  \frac{d}{dx} (x^3 - 5x^2 + 3x -2)e^x
  \]
  
    \begin{hint}
      Use the Product Rule with $x^3 - 5x^2 + 3x -2$ and $e^x$.
    \end{hint}
    \begin{hint}
      $(fg)' = f'g+g'f$.
    \end{hint}
    \begin{hint}
      The derivative of $x^3 - 5x^2 + 3x -2$ is $3x^2 - 10x + 3$
    \end{hint}
    \begin{hint}
      The derivative of $e^x$ is itself
    \end{hint}
    \begin{hint}
      Factor out $e^x$ and combine like terms 
    \end{hint}
		The derivative of $(x^3 - 5x^2 + 3x -2)e^x$ with respect to $x$ is
		 $\answer{(x^3 - 2x^2 - 7x +1)e^x}$
		
\end{problem}




\begin{example}[example 6]
Find $h'(x)$ if $h(x) = x\ln(x)$.\\
We write $h(x)$ as a product: $h(x) = f(x) \cdot g(x)$ with
\[f(x) = x \quad \text{and} \quad g(x) = \ln(x).\]
To use the product rule, we need the derivatives:
\[f'(x) = 1 \quad \text{and} \quad g'(x)= \frac{1}{x}.\]
We can now write the derivative:
\begin{align*}
h'(x) &= f'(x)g(x) + f(x)g'(x) \\
&=  1 \cdot \ln(x) + x\frac{1}{x}  \\
&=  \ln(x) + 1.
\end{align*}
\end{example}



\begin{center}
\begin{foldable}
\unfoldable{Here is a video of the preceding example}
\youtube{mJXBsi0uZWA} %vid of example 4
\end{foldable}
\end{center}



\begin{problem}(problem 6)
  Compute
  \[
  \frac{d}{dx} x^3\ln(x)
  \]
  
    \begin{hint}
      Use the Product Rule with $x^3$ and $\ln(x)$.
    \end{hint}
    \begin{hint}
      $(fg)' = f'g+g'f$.
    \end{hint}
    \begin{hint}
      The derivative of $x^3$ is $3x^2$
    \end{hint}
    \begin{hint}
      The derivative of $\ln(x)$ is $1/x$
    \end{hint}
		The derivative of $x^3\ln(x)$ with respect to $x$ is
		 $\answer{x^2(3 \ln(x) + 1)}$
		
\end{problem}


\begin{example}[example 7]
Find $h'(x)$ if $h(x) = e^x\sin(x)$.\\
We write $h(x)$ as a product: $h(x) = f(x)\cdot g(x)$ with
\[f(x) = e^x \quad \text{and} \quad g(x) = \sin(x).\]
To use the product rule, we need the derivatives:
\[f'(x) = e^x \quad \text{and} \quad g'(x) = \cos(x).\]
We can now write the derivative:
\begin{align*}
h'(x) &= f'(x)g(x) + f(x)g'(x) \\
&= e^x \sin(x) + e^x \cos(x) \\
&= e^x[\sin(x) +  \cos(x)].
\end{align*}
\end{example}


\begin{center}
\begin{foldable}
\unfoldable{Here is a video of the preceding example}
\youtube{hZC3kMNKHa0} %vid of example 5
\end{foldable}
\end{center}



\begin{problem}(problem 7)
  Compute
  \[
  \frac{d}{dx} 3e^x \cos(x)
  \]
  
    \begin{hint}
      Use the Product Rule with $3e^x$ and $\cos(x)$.
    \end{hint}
    \begin{hint}
      $(fg)' = f'g+g'f$.
    \end{hint}
    \begin{hint}
      The derivative of $3e^x$ is itself
    \end{hint}
    \begin{hint}
      The derivative of $\cos(x)$ is $-\sin(x)$
    \end{hint}
		\begin{hint}
      Factor out $3e^x$
    \end{hint}
		The derivative of $3e^x\cos(x)$ with respect to $x$ is
		 $\answer{3e^x(\cos(x) - \sin(x))}$
		
\end{problem}




\begin{center}
\begin{foldable}
\unfoldable{Here is a detailed, lecture style video on the Product Rule:}
\youtube{gK9hyA8kcJc}
\end{foldable}
\end{center}

We conclude this section with a derivation of the product rule using the definition of the derivative.
\begin{align*}
\left[f(x)g(x)\right]' &= \lim_{h \to 0} \frac{f(x+h)g(x+h)-f(x)g(x)}{h}\\[5pt] 
&= \lim_{h \to 0} \frac{f(x+h)g(x+h)- f(x)g(x+h) + f(x)g(x+h) - f(x)g(x)}{h}\\[5pt] 
&= \lim_{h \to 0} \frac{f(x+h)g(x+h)- f(x)g(x+h)}{h} + \frac{f(x)g(x+h) - f(x)g(x)}{h} \\[5pt] 
&=  \lim_{h \to 0} \frac{g(x+h)\left[f(x+h)- f(x)\right]}{h} + \frac{f(x)\left[g(x+h) - g(x)\right]}{h}\\[5pt] 
&= g(x)f'(x) + f(x)g'(x).
\end{align*}


\end{document}



