\documentclass{ximera}

\input{../preamble}

\outcome{Learn properties of indefinite integrals}

\title{4.2 Properties of Indefinite Integrals}


\begin{document}

\begin{abstract}
In this section we examine several properties of the indefinite integral.
\end{abstract}

\maketitle

\section{Properties of Indefinite Integrals}

\begin{theorem}[Constant Multiple Rule]
\[\int cf(x) \ dx = c\int f(x) \ dx\]
where c is a constant.
\end{theorem}


\begin{example}[example 1]
\[
\int 5\cos(x) \ dx = 5 \int \cos(x) \ dx = 5\sin(x) +C.
\]
\end{example}


\begin{problem}(problem 1a)
\ Compute
%\[
%\int 8\cos(x) \ dx.
%\]

\begin{hint}
$\frac{d}{dx} \sin(x) = \cos(x)$
\end{hint}
\begin{hint}
\begin{center}
Do not add the +C to your answer
\end{center}
\end{hint}

\[
\int 8\cos(x) \ dx =
\answer[given]{8\sin(x)} \ +  C
\]
\end{problem}



\begin{problem}(problem 1b)
Compute
%\[
%\int 4\sin(x) \ dx.
%\]

\begin{hint}
$\frac{d}{dx} \cos(x) = -\sin(x)$
\end{hint}
\begin{hint}
\begin{center}
Do not add the +C to your answer
\end{center}
\end{hint}

\[
\int 4\sin(x) \ dx =
\answer[given]{-4\cos(x)} \ +  C
\]
\end{problem}



\begin{example}[example 2]
\[
\int 3\sec^2(x) \ dx = 3 \int \sec^2(x) \ dx = 3\tan(x) +C.
\]
\end{example}



\begin{problem}(problem 2a)
Compute
%\[
%\int 5\sec^2(x) \ dx.
%\]

\begin{hint}
$\frac{d}{dx} \tan(x) = \sec^2(x)$
\end{hint}
\begin{hint}
\begin{center}
Do not add the +C to your answer
\end{center}
\end{hint}

\[
\int 5\sec^2(x) \ dx =
\answer[given]{5\tan(x)} \ +  C
\]
\end{problem}


\begin{problem}(problem 2b)
Compute
%\[
%\int 2\csc^2(x) \ dx.
%\]

\begin{hint}
$\frac{d}{dx} \cot(x) = -\csc^2(x)$
\end{hint}
\begin{hint}
\begin{center}
Do not add the +C to your answer
\end{center}
\end{hint}

\[
\int 2\csc^2(x) \ dx =
\answer[given]{-2\cot(x)} \ +  C
\]
\end{problem}


\begin{example}[example 3]
\[
\int 2e^x \ dx = 2 \int e^x \ dx = 2e^x +C.
\]
\end{example}


\begin{problem}(problem 3a)
Compute
%\[
%\int 7e^x \ dx.
%\]

\begin{hint}
$\frac{d}{dx} e^x = e^x$
\end{hint}
\begin{hint}
\begin{center}
Do not add the +C to your answer
\end{center}
\end{hint}

\[
\int 7e^x \ dx =
\answer[given]{7e^x} \ +  C
\]
\end{problem}


\begin{problem}(problem 3b)
Compute
%\[
%\int \frac{e^x}{3} \ dx.
%\]

\begin{hint}
$\frac{d}{dx} e^x = e^x$
\end{hint}
\begin{hint}
\begin{center}
Do not add the +C to your answer
\end{center}
\end{hint}

\[
\int \frac{e^x}{3} \ dx =
\answer[given]{e^x /3} \ +  C
\]
\end{problem}


\begin{example}[example 4]
\[
\int \frac{4}{1+x^2} \ dx = 4 \int \frac{1}{1+x^2} \ dx = 4\tan^{-1}(x) +C.
\]
\end{example}



\begin{problem}(problem 4a)
Compute
%\[
%\int \frac{9}{1+x^2} \ dx.
%\]

\begin{hint}
$\frac{d}{dx} \tan^{-1}(x) = \frac{1}{1+x^2}$
\end{hint}
\begin{hint}
\begin{center}
Do not add the +C to your answer
\end{center}
\end{hint}

\[
\int \frac{9}{1+x^2} \ dx =
\answer[given]{9\tan^{-1}(x)} \ +  C
\]
\end{problem}

\begin{problem}(problem 4b)
Compute
%\[
%\int \frac{6}{\sqrt{1-x^2}} \ dx.
%\]

\begin{hint}
$\frac{d}{dx} \sin^{-1}(x) = \frac{1}{\sqrt{1-x^2}}$
\end{hint}
\begin{hint}
\begin{center}
Do not add the +C to your answer
\end{center}
\end{hint}

\[
\int \frac{6}{\sqrt{1-x^2}} \ dx =
\answer[given]{6\sin^{-1}(x)} \ +  C
\]
\end{problem}


\begin{example}[example 5]
\[
\int \frac{7}{12x} \ dx = \frac{7}{12} \int \frac{1}{x} \ dx = \frac{7}{12} \ln|x| +C.
\]
\end{example}


\begin{problem}(problem 5a)
Compute
%\[
%\int \frac{5}{x} \ dx.
%\]

\begin{hint}
$\frac{d}{dx} \ln|x| = \frac{1}{x}$
\end{hint}
\begin{hint}
\begin{center}
Do not add the +C to your answer
\end{center}
\end{hint}

\[
\int \frac{5}{x} \ dx =
\answer[given]{5\ln|x|} \ +  C
\]
\end{problem}

\begin{problem}(problem 5b)
Compute
%\[
%\int \frac{1}{2x} \ dx.
%\]

\begin{hint}
$\frac{d}{dx} \ln|x| = \frac{1}{x}$
\end{hint}
\begin{hint}
\begin{center}
Do not add the +C to your answer
\end{center}
\end{hint}

\[
\int \frac{1}{2x} \ dx =
\answer[given]{\ln|x| /2} \ +  C
\]
\end{problem}


\begin{example}[example 6]
\[
\int 4x^7 \ dx = 4 \int x^7 \ dx = 4\cdot \frac{x^8}{8} +C 
= \frac{x^8}{2}.
\]
\end{example}


\begin{problem}(problem 6a)
Compute 
%\[
%\int 6x^4 \ dx.
%\]

\begin{hint}
Use the power rule with $n=4$
\end{hint}
\begin{hint}
The Power Rule says $\int x^n \ dx = \frac{x^{n+1}}{n+1} +$ C
\end{hint}
\begin{hint}
\begin{center}
Do not add the +C to your answer
\end{center}
\end{hint}

\[
\int 6x^4 \ dx =
\answer[given]{6x^5 /5} \ + C
\]
\end{problem}


\begin{problem}(problem 6b)
Compute 
%\[
%\int 8x^3 \ dx.
%\]

\begin{hint}
Use the power rule with $n=3$
\end{hint}
\begin{hint}
The Power Rule says $\int x^n \ dx = \frac{x^{n+1}}{n+1} +$ C
\end{hint}
\begin{hint}
\begin{center}
Do not add the +C to your answer
\end{center}
\end{hint}

\[
\int 8x^3 \ dx =
\answer[given]{2x^4} \ + C
\]
\end{problem}


\begin{example}[example 7]
$\begin{aligned}[t]
\int \frac{3}{5x^2} \ dx &= \frac{3}{5} \int \frac{1}{x^2} \ dx \\[3pt]
&=\frac{3}{5} \int x^{-2} \ dx \\[3pt]
&= \frac{3}{5} \cdot \frac{x^{-1}}{-1} +C \\[5pt]
&= -\frac{3}{5} \cdot \frac{1}{x} +C \\[5pt]
&= -\frac{3}{5x} +C.
\end{aligned}$
\end{example}


\begin{problem}(problem 7a)
Compute 
%\[
%\int \frac{3}{x^2} \ dx.
%\]

\begin{hint}
Negative exponents: $\frac{3}{x^2} = 3x^{-2}$
\end{hint}
\begin{hint}
Use the power rule with $n=-2$
\end{hint}
\begin{hint}
The Power Rule says $\int x^n \ dx = \frac{x^{n+1}}{n+1} +$ C
\end{hint}
\begin{hint}
\begin{center}
Do not add the +C to your answer
\end{center}
\end{hint}

\[
\int \frac{3}{x^2} \ dx =
\answer[given]{-3x^{-1}} \ + C
\]
\end{problem}


\begin{problem}(problem 7b)
Compute 
%\[
%\int \frac{4}{5x^6} \ dx.
%\]

\begin{hint}
Negative exponents: $\frac{4}{5x^6} = \frac45 x^{-6}$
\end{hint}
\begin{hint}
Use the power rule with $n=-6$
\end{hint}
\begin{hint}
The Power Rule says $\int x^n \ dx = \frac{x^{n+1}}{n+1} +$ C
\end{hint}
\begin{hint}
\begin{center}
Do not add the +C to your answer
\end{center}
\end{hint}

\[
\int \frac{4}{5x^6} \ dx =
\answer[given]{-4/25 x^{-5}} \ + C
\]
\end{problem}


\begin{example}[example 8]
$\begin{aligned}[t]
\int 4\sqrt[3]x  \ dx &= 4 \int \sqrt[3] x \  dx  \\
&= 4 \int x^{1/3} \ dx \\
&= 4 \cdot \frac{x^{4/3}}{4/3} +C \\[3pt]
&= 4 \cdot \frac{3}{4} \cdot x^{4/3} +C \\[3pt]
&= 3x^{4/3} +C \\
&= 3\sqrt[3] {x^4} +C \\
&= 3x\sqrt[3] x +C.
\end{aligned}$
\end{example}


\begin{problem}(problem 8a)
Compute 
%\[
%\int 3\sqrt x \ dx.
%\]

\begin{hint}
Rational exponents: $\sqrt x = x^{1/2}$
\end{hint}
\begin{hint}
Use the power rule with $n=1/2$
\end{hint}
\begin{hint}
The Power Rule says $\int x^n \ dx = \frac{x^{n+1}}{n+1} +$ C
\end{hint}
\begin{hint}
\begin{center}
Do not add the +C to your answer
\end{center}
\end{hint}

\[
\int 3\sqrt x \ dx =
\answer[given]{2x^{3/2}} \ + C
\]
\end{problem}


\begin{problem}(problem 8b)
Compute 
\[
\int 5\sqrt[4]x \ dx.
\]

\begin{hint}
Rational exponents: $\sqrt[4]x = x^{1/4}$
\end{hint}
\begin{hint}
Use the power rule with $n=1/2$
\end{hint}
\begin{hint}
The Power Rule says $\int x^n \ dx = \frac{x^{n+1}}{n+1} +$ C
\end{hint}
\begin{hint}
\begin{center}
Do not add the +C to your answer
\end{center}
\end{hint}

\[
\int 5\sqrt[4]x \ dx =
\answer[given]{4x^{5/4}} \ + C
\]
\end{problem}



\begin{theorem}[Sum And Difference Rules]
The integral of a sum or difference is the sum or difference of the integrals:
\[
\int \left[f(x)\pm g(x)\right] \ dx = \int f(x) \; dx  \pm  \int g(x) \; dx.
\]
\end{theorem}



\begin{example}[example 9]
\[
\int \left(\cos(x) + e^x\right) \ dx = \sin(x) + e^x + C.
\]
\end{example}

\begin{problem}(problem 9a)
Compute
\[
\int \big(1 + \cos(x) \big) \ dx.
\]

\begin{hint}
$\frac{d}{dx} x = 1$
\end{hint}
\begin{hint}
$\frac{d}{dx} \sin(x) = \cos(x)$
\end{hint}
\begin{hint}
\begin{center}
Do not add the +C to your answer
\end{center}
\end{hint}

\[
\int \left[1 + \cos(x) \right] \ dx =
\answer[given]{x + \sin(x)} \ +  C
\]
\end{problem}


\begin{problem}(problem 9b)
Compute
\[
\int \left[e^x + \sin(x) \right] \ dx.
\]

\begin{hint}
$\frac{d}{dx} e^x = e^x$
\end{hint}
\begin{hint}
$\frac{d}{dx} \cos(x) = -\sin(x)$
\end{hint}
\begin{hint}
\begin{center}
Do not add the +C to your answer
\end{center}
\end{hint}

\[
\int \left(e^x + \sin(x) \right) \ dx =
\answer[given]{e^x -\cos(x)} \ +  C
\]
\end{problem}


\begin{example}[example 10]
\[
\int \left(1 - e^x\right) \ dx = x - e^x + C.
\]
\end{example}

\begin{problem}(problem 10)
Compute
\[
\int (3e^x - 4x) \; dx = \answer{3e^x - 2x^2} + C.
\]
\end{problem}



\begin{example}[example 11]
\[
\int \left(x^2 - x\right) \ dx = \dfrac{x^3}{3} - \dfrac{x^2}{2} + C.
\]
\end{example}


\begin{problem}(problem 11)
Compute
\[
\int (x^5 - x^3) \; dx = \answer{1/6 x^6 - 1/4 x^4} + C.
\]
\end{problem}




\begin{example}[example 12]
\[
\int \left(x + \sec^2(x)\right) \ dx = \frac{x^2}{2} + \tan(x) + C.
\]
\end{example}

\begin{problem}(problem 12a)
Compute
\[
\int \big(1 + \sec(x)\tan(x) \big) \ dx.
\]

\begin{hint}
$\frac{d}{dx} x = 1$
\end{hint}
\begin{hint}
$\frac{d}{dx} \sec(x) = \sec(x)\tan(x)$
\end{hint}
\begin{hint}
\begin{center}
Do not add the +C to your answer
\end{center}
\end{hint}

\[
\int \big(1 + \sec(x)\tan(x) \big) \ dx =
\answer[given]{x + \sec(x)} \ +  C
\]
\end{problem}


\begin{problem}(problem 12b)
Compute
\[
\int \left(x + \csc^2(x) \right) \ dx.
\]

\begin{hint}
$\frac{d}{dx} x^2 = 2x$
\end{hint}
\begin{hint}
$\frac{d}{dx} \cot(x) = -\csc^2(x)$
\end{hint}
\begin{hint}
\begin{center}
Do not add the +C to your answer
\end{center}
\end{hint}

\[
\int \left(x + \csc^2(x) \right) \ dx =
\answer[given]{x^2 /2 - \cot(x)} \ +  C
\]
\end{problem}



\begin{example}[example 13]
\[
\int \left[3\cos(x) - 2\sin(x)\right] \ dx = 3\sin(x) + 2\cos(x) + C.
\]
\end{example}


\begin{problem}(problem 13)
Compute
\[
\int \left[4\sin(t) - 6\cos(t)\right] \; dt = \answer{-4\cos(t) - 6\sin(t)} + C.
\]
\end{problem}

\begin{example}[example 14]
\[
\int 4\csc(x)\big[\csc(x) - \cot(x)\big] \ dx = \int \big(4\csc^2(x)  - 4\csc(x)\cot(x)\big) \ dx
\]
\[
 = -4\cot(x) + 4\csc(x) + C
= 4\csc(x) - 4 \cot(x) + C.
\]
\end{example}



\begin{problem}(problem 14a)
Compute
\[
\int \sec(x)\big[\sec(x) + \tan(x) \big] \ dx.
\]

\begin{hint}
Distribute $\sec(x)$
\end{hint}
\begin{hint}
$\frac{d}{dx} \tan(x) = \sec^2(x)$
\end{hint}
\begin{hint}
$\frac{d}{dx} \sec(x) = \sec(x)\tan(x)$
\end{hint}
\begin{hint}
\begin{center}
Do not add the +C to your answer
\end{center}
\end{hint}

\[
\int \sec(x)\big[\sec(x) + \tan(x) \big] \ dx =
\answer[given]{\tan(x) + \sec(x)} \ +  C
\]
\end{problem}




\begin{problem}(problem 14b)
Compute
\[
\int 3\cot(x)\left[2\csc(x) - \tan(x)\right]\; dx = \answer{-6\csc(x) - 3x} + C.
\]
\end{problem}



\begin{example}[example 15]
\[
\int x^2 + \dfrac{1}{x^2} \ dx = \int x^2 + x^{-2} \ dx = \dfrac{x^3}{3} + \dfrac{x^{-1}}{-1} + C 
= \dfrac{x^3}{3} - \dfrac{1}{x} + C.
\]

\end{example}


\begin{example}[example 16]
\[
\int \dfrac{x+2}{x} \ dx = \int \dfrac{x}{x} + \dfrac{2}{x} \ dx = \int 1 + \dfrac{2}{x} \ dx = x + 2\ln|x| +C.
\]

\end{example}


\begin{problem}(problem 16)
Compute
\[
\int \dfrac{x^3 + 3x^2 - 4x + 5}{x^2} \ dx.
\]

\begin{hint}
Divide each term by $x^2$
\end{hint}
\begin{hint}
Use the power rule where appropriate ($n\neq -1$)
\end{hint}
\begin{hint}
\begin{center}
Do not add the +C to your answer
\end{center}
\end{hint}

\[
\int  \dfrac{x^3 + 3x^2 - 4x + 5}{x^2} \ dx =
\answer[given]{x^2 /2 + 3x - 4\ln|x| -5/x} \ +  C
\]
\end{problem}



\begin{example}[example 17]
\[
\int \left(3x^2 - \dfrac{3}{x} - \dfrac{1}{1+x^2}\right) \ dx = x^3 - 3\ln|x| - \tan^{-1}(x) + C.
\]
\end{example}


\begin{problem}(problem 17)
Compute
\[
\int \left(\frac{2}{x^3} - \frac{3}{x} \right) \; dx = \answer{-x^{-2} -3\ln|x|} + C.
\]
\end{problem}

\begin{example}[example 18]
$\begin{aligned}[t]
\int \big(\sqrt x + \sqrt[3] x \big) \ dx &= \int \big(x^{1/2} + x^{1/3}\big) \ dx \\
&= \frac{x^{3/2}}{3/2} + \frac{x^{4/3}}{4/3} + C \\
&= \tfrac{2}{3} x^{3/2} + \tfrac{3}{4} x^{4/3} + C \\
&= \tfrac{2}{3} \sqrt {x^3} + \tfrac{3}{4}  \sqrt[3] {x^4} + C \\
&= \tfrac{2}{3} x\sqrt x + \tfrac{3}{4} x \sqrt[3] x + C.
\end{aligned}$
\end{example}


\begin{problem}(problem 18)
Compute
\[
\int x\big(\sqrt x + \sqrt[3] x \big) \ dx.
\]

\begin{hint}
Distribute the x (add exponents)
\end{hint}
\begin{hint}
Use the power rule where appropriate ($n\neq -1$)
\end{hint}
\begin{hint}
\begin{center}
Do not add the +C to your answer
\end{center}
\end{hint}

\[
\int  x\big(\sqrt x + \sqrt[3] x \big) \ dx =
\answer[given]{2/5 x^{5/2} + 3/7 x^{7/3}} \ +  C
\]
\end{problem}


\begin{example}[example 19]
\[
\int x^2(x^2 - 3x + 4) \ dx = \int (x^4 - 3x^3 + 4x^2) \ dx = \frac15 x^5 - \frac{3}{4}x^4 + \frac43 x^3 + C.
\]

\end{example}

\begin{problem}(problem 19)
Compute
\[
\int \left(x^4 - 2x^3 + 6x^2 - 8x + 7 \right) \; dx = \answer{ x^5/5 - x^4/2 + 2x^3 - 4x^2 + 7x} + C.
\]
\end{problem}

%\begin{theorem}(Difference Rule)
%If $\int f(x) \ dx = F(x) + C$ and $\int g(x) \ dx = G(x) + C$, then
%\[\int \big(f(x)-g(x)\big) \ dx = F(x) - G(x) + C\]
%\end{theorem}
%In words, the integral of a difference is the difference of the integrals.




\section{Initial Value Problems}


One reason we might be interested in computing an indefinite integral is to solve a differential equation. Consider the following initial value problem:\\
Given, $f'(x) = h(x)$ and $f(x_0) = y_0$, find $f(x)$.\\
The condition, $f(x_0) = y_0$, is called an initial condition. The main step in slving this problem is to observe that the function $f(x)$ that we seek is an anti-derivative of the given function $h(x)$. Hence, to find $f(x)$ we will compute the definite integral, 

\[f(x) = \int f'(x) \ dx = \int h(x) \ dx.\]

Lets look at some examples.

\begin{example}[example 20]
Solve the initial value problem:
\[f'(x) = x - 3, \ f(2) = 4.\]

First, 
\[f(x) = \int f'(x) \ dx = \int (x-3)  \ dx = \frac{x^2}{2} - 3x + C.\]
Then, we use the initial condition, $f(2) = 4$, to find the 
appropriate value of the constant $C$.
\[f(2) = \frac{2^2}{2} - 3(2) + C = -4 + C = 4,\]
which yields $C = 8$.
So, the final answer is  $f(x) = \frac{x^2}{2} -3x + 8.$
\end{example}

\begin{example}[example 21]
Solve the initial value problem:
\[f'(x) = 2\cos(x) -3\sin(x), \ f(0) = 1.\]

First, 
\[f(x) = \int f'(x) \ dx = \int \big[2\cos(x) -3\sin(x)\big]  \ dx =
 2\sin(x) + 3\cos(x) + C.\]
Then, we use the initial condition, $f(0) = 1$, to find the 
appropriate value of the constant $C$.
\[f(0) = 2\sin(0) + 3\cos(0) + C = 0 + 3 + C = 1,\]
which yields $C = -2$.
So, the final answer is  $f(x) = 2\sin(x) + 3\cos(x)-2.$
\end{example}

\begin{problem}(problem 21a)
Solve the initial value problem:
\[f'(x) = x-4, \ f(2) = 0.\]
\begin{hint}
anti-differentiate $f'(x)$
\end{hint}
\begin{hint}
Solve for the constant of integration, $C$
\end{hint}
\[f(x) = \answer{\frac{x^2}{2} - 4x + 6}.\]
\end{problem}

\begin{problem}(problem 21b)
Solve the initial value problem:
\[f'(x) = 3\cos(x), \ f(0) = -2.\]
\begin{hint}
anti-differentiate $f'(x)$
\end{hint}
\begin{hint}
Solve for the constant of integration, $C$
\end{hint}
\[f(x) = \answer{3\sin(x) - 2}.\]
\end{problem}

\begin{problem}(problem 21c)
Solve the initial value problem:
\[f'(x) = \frac{1}{x}, \ f(-1) = 5.\]
\begin{hint}
anti-differentiate $f'(x)$
\end{hint}
\begin{hint}
Solve for the constant of integration, $C$
\end{hint}
\[f(x) = \answer{\ln|x| + 5}.\]
\end{problem}

\begin{problem}(problem 21d)
Solve the initial value problem:
\[f'(x) = e^{2x}, \ f(0) = 1.\]
\begin{hint}
Anti-differentiate $f'(x)$
\end{hint}
\begin{hint}
Solve for the constant of integration, $C$
\end{hint}
\[f(x) = \answer{\frac{e^{2x}}{2} + \frac12}.\]
\end{problem}


\end{document}
