\documentclass[handout]{ximera}

\input{../preamble}

\outcome{Compute an anti-derivative by reversing the chain rule.}

\title{4.3 Substitution}



\begin{document}

\begin{abstract}
In this section we learn to reverse the chain rule by making a substitution.
\end{abstract}

\maketitle

\section{U-Substitution}

Suppose that $f(x)$ is an anti-derivative of $f(x)$, i.e., $F'(x) = f(x)$. 
Consider the composition, $F(g(x))$, where $g(x)$ is a differentiable function. What is the derivative of 
$F(g(x))$? According to the chain rule,
\[
\frac{d}{dx} F\left(g(x)\right) = f\left(g(x)\right)\cdot g'(x).
\]
From the point of view of integration, this differentiation equation 
is equivalent to the anti-differentiation equation:
\[
\int f(g(x))\cdot g'(x) \; dx = F(g(x)) + C.
\]
What this equation would look like if we used familar functions? We will 
let $g(x) = x^2 + 1$ and $f(x) = \cos x$. Composing them gives
\[
 f(g(x)) = \cos(x^2 + 1).
 \]
 Furthermore, the derivative of $g(x)$ is, $g'(x) = 2x$,
  and an anti-derivative of $f(x)$ is, $F(x) = \sin x$. 
  Putting this information into the anti-differentiation equation yields:
\[
\int \cos(x^2 + 1) \cdot 2x \; dx = \sin(x^2 + 1) + C.
\]
This is most easily understood by differentiaing the right hand side using the chain rule(!):
\[
\frac{d}{dx} \sin(x^2+1) = \cos(x^2 + 1) \cdot 2x.
\]
In other words, this equation is difficult to reproduce is we are just staring at the left hand side:
\[
\int \cos(x^2+1) \cdot 2x \; dx.
\]
The technique for systematically finding the anti-derivative,
\[
\int f(g(x)) \; dx,
\]
is to make a \textbf{u-substitution} which is a three step process.
In the first step, the substitution $u = g(x)$ is declared and the integral is re-written in terms of the variable $u$ as
\[
\int f(g(x)) \cdot g'(x) \; dx = \int f(u) \; du.
\]
Notice that the left hand-side has the differential $dx$ and the right hand side has the differential $du$.
We will learn how to convert between differentials.
Step two is to compute the indefinite integral.  Assuming we know an antiderivative for $f(u)$, we get:
\[
\int f(u) \; du = F(u) + C.
\]
The third and final step is to replace the variable $u$ in the previous step with $g(x)$, to obtain
\[
F(u) + C = F(g(x)) + C.
\]
Thus
\[
\int f(g(x)) \cdot g'(x) \; dx = \int f(u) \; du = F(u) + C = F(g(x)) + C.
\]
Refer back to this equation after you have worked through some examples and 
problems to review the method of $u$-substitution.


%We make a u-substitution to fill in the gaps in the following equation, which reverses the chain rule:
%\[\int f(g(x))g'(x) \ dx = F(g(x)) + C. \]
%If we let $ u = g(x)$ then $du = g'(x) \ dx$ and the integral can be rewritten as
%\[\int f(g(x))g'(x) \ dx = \int f(u) \ du \] which equals
%\[F(u) + C\] and back substituting gives \[F(g(x)) + C. \]  Now we can see that \[\int f(g(x))g'(x) \ dx = F(g(x)) + C. \]



\begin{example}[example 1]
Compute 
\[\int 2x\cos(x^2 + 1) \ dx.\]

We will make a u-substitution for the inside of the composition $\cos(x^2 + 1)$:\
\[
\text{let} \;\; u = x^2 + 1.  
\]
We now determine the relationship between the differentials $dx$ and $du$.
Differentiatiating $u$ gives:
\[
\frac{du}{dx} = 2x.
\]
This equation can be written in \textbf{differential form} as
\[
du = 2x \; dx.
\]
For the purpose of our impending computation, we will express this equation in terms of the original differential, $dx$:
\[
dx = \frac{1}{2x} \; du.
\]
We can now proceed with step one and convert the original integral into a simpler one, in the variable, $u$:
\[
\int  2x\cos(x^2 + 1) \; dx = \int 2x\cos u \frac{1}{2x} \; du = \int \cos u \; du.
\]
Notice that \;$`2x$' \; cancelled with its reciprocal. Now for step two, anti-differentiation:
\[
\int \cos u \; du = \sin u + C.
\]
And the coup de grace, step three, we return to the variable $x$:
\[
\sin(u) + C = \sin(x^2 + 1) + C.
\]

Recapping,
\[\int 2x\cos(x^2 + 1) \ dx = \int \cos u \ du =  \sin u + C =  \sin(x^2 + 1) + C.\]


%and the integral can be written as 
%\[\int 2x\cos(x^2 + 1) \ dx = \int \cos(x^2 + 1) \ 2x\  dx = \int \cos(u) \ du.\]
%The last integral can be computed as 
%\[\int \cos(u) \ du = \sin(u) + C\]
%and by back substituting, we have 
%\[\sin(u) + C = \sin(x^2 + 1) + C.\]
%Thus, using u-substitution we can conclude that
%\[\int 2x\cos(x^2 + 1) \ dx =  \sin(x^2 + 1) + C.\]


\end{example}



\begin{problem}(problem 1a) 
Compute: $\displaystyle{\int 3x^2\cos(x^3 + 2) \ dx}$\\
Let $u = \answer{x^3 + 2}$, then $du = \answer{3x^2 dx}$\\
\begin{hint}
Don't forget the `dx' in your answer for `du'
\end{hint}
Convert to an integral in the variable $u$:
\[\int 3x^2\cos(x^3 + 2) \ dx = \int\answer{\cos u du}\]
\begin{hint}
Don't forget the `du' in your integral
\end{hint}
The final answer in terms of $x$ is:

\[\int 3x^2\cos(x^3 + 2) \ dx = \answer{\sin(x^3 + 2)} +C\]
\end{problem}



\begin{problem}(problem 1b) 
Compute: $\displaystyle{\int 5x^4\sin(x^5 -7) \ dx}$.\\
Let $u = \answer{x^5 - 7}$, then $du = \answer{5x^4 dx}$.\\
\begin{hint}
Don't forget the `dx' in your answer for `du'.
\end{hint}
Convert to an integral in the variable $u$:
\[\int 5x^4\sin(x^5 -7) \ dx = \int\answer{\sin u du}\]
\begin{hint}
Don't forget the `du' in your integral.
\end{hint}
The final answer in terms of $x$ is:
\[\int 5x^4\sin(x^5 -7) \ dx = \answer{-\cos(x^5 -7)} +C.\]
\end{problem}


\begin{example}[example 2] 
Compute 
\[\int 2x(x^2 + 1)^4 \ dx.\]
Let $u = x^2 + 1$.  We have,
\[u = x^2 + 1\]
\[du = 2x \ dx\]

and the integral can be written as 
\[\int 2x(x^2 + 1)^4 \ dx = \int (x^2 + 1)^4 \ 2x \  dx = \int u^4 \ du.\]
The last integral can be computed as 
\[\int u^4 \ du = \tfrac{u^5}{5} + C\]
and by back substituting, we have 
\[\tfrac{u^5}{5} + C = \tfrac15(x^2 + 1)^5 + C .\]
Thus, using u-substitution we can conclude that
\[\int 2x(x^2 + 1)^4 \ dx  =  \tfrac15(x^2 + 1)^5 + C .\]
\end{example}



\begin{problem}(problem 2a)
 Compute $\displaystyle{\int 3x^2(x^3 + 2)^6 \ dx}$.\\
Let $u = \answer{x^3 + 2}$, then $du = \answer{3x^2 dx}$.\\
\begin{hint}
Don't forget the `dx' in your answer for `du'.
\end{hint}
Convert to an integral in the variable $u$:
\[\int 3x^2(x^3 + 2)^6 \ dx = \int\answer{u^6 du}\]
\begin{hint}
Don't forget the `du' in your integral.
\end{hint}
The final answer in terms of $x$ is:

\[\int 3x^2(x^3 + 2)^6 \ dx = \answer{(x^3 + 2)^7/7} +C.\]
\end{problem}



\begin{problem}(problem 2b) 
Compute $\displaystyle{\int 4x^3(x^4 -1)^8 \ dx}$.\\
Let $u = \answer{x^4 -1}$, then $du = \answer{4x^3 dx}$.\\
\begin{hint}
Don't forget the `dx' in your answer for `du'.
\end{hint}
Convert to an integral in the variable $u$:
\[\int 4x^3(x^4 -1)^8 \ dx = \int\answer{u^8 du}\]
\begin{hint}
Don't forget the `du' in your integral.
\end{hint}
The final answer in terms of $x$ is:
\[\int 4x^3(x^4 -1)^8 \ dx = \answer{(x^4 -1)^9/9} +C.\]
\end{problem}



\begin{example}[example 3] 
Compute 
\[\int 2xe^{(x^2 + 1)} \ dx.\]
Let $u = x^2 + 1$.  We have,
\[u = x^2 + 1\]
\[du = 2x \ dx\]

\[\int 2xe^{(x^2 + 1)} \ dx = \int e^{(x^2 + 1)} \ 2x\  dx = \int e^u \ du.\]
The last integral can be computed as 
\[\int e^u \ du = e^u + C\]
and by back substituting, we have 
\[e^u + C = e^{(x^2 + 1)} + C.\]
Thus, using u-substitution we can conclude that
\[\int 2xe^{(x^2 + 1)} \ dx =  e^{(x^2 + 1)} + C.\]
\end{example}



\begin{problem}(problem 3a)
 Compute $\displaystyle{\int 3x^2e^{x^3 + 2} \ dx}$.\\
Let $u = \answer{x^3 + 2}$, then $du = \answer{3x^2 dx}$.\\
\begin{hint}
Don't forget the `dx' in your answer for `du'.
\end{hint}
Convert to an integral in the variable $u$:
\[\int 3x^2e^{x^3 + 2} \ dx = \int\answer{e^u du}\]
\begin{hint}
Don't forget the `du' in your integral.
\end{hint}
The final answer in terms of $x$ is:
\[\int 3x^2e^{x^3 + 2} \ dx = \answer{e^{x^3 + 2}} +C.\]
\end{problem}



\begin{problem}(problem 3b) 
Compute $\displaystyle{\int -2xe^{-x^2} \ dx}$.\\
Let $u = \answer{-x^2}$, then $du = \answer{-2x dx}$.\\
\begin{hint}
Don't forget the `dx' in your answer for `du'.
\end{hint}
Convert to an integral in the variable $u$:
\[\int -2xe^{-x^2} \ dx = \int\answer{e^u du}\]
\begin{hint}
Don't forget the `du' in your integral.
\end{hint}
The final answer in terms of $x$ is:
\[\int -2xe^{-x^2} \ dx = \answer{e^{-x^2}} +C.\]
\end{problem}



\begin{example}[example 4] 
Compute 
\[\int 2x\sqrt{x^2 + 1} \ dx.\]
Let $u = x^2 + 1$.  We have,
\[u = x^2 + 1\]
\[du = 2x \ dx\]

\[\int 2x\sqrt{x^2 + 1} \ dx = \int \sqrt{x^2 + 1} \cdot 2x\  dx = \int \sqrt{u} \ du.\]
The last integral can be computed as 
\[\int \sqrt u  \ du = \int u^{1/2} \ du = \tfrac{u^{3/2}}{3/2} + C = \tfrac23 u^{3/2} + C\]
and by back substituting, we have 
\[\tfrac23 u^{3/2}  + C = \frac23 (x^2 + 1)^{3/2} + C.\]
Thus, using u-substitution we can conclude that
\[\int 2x\sqrt{x^2 + 1} \ dx =  \tfrac23 (x^2 + 1)^{3/2} + C.\]
\end{example}



\begin{problem}(problem 4) 
Compute $\displaystyle{\int 4x^3 \sqrt{x^4 +2} \ dx}$.\\
Let $u = \answer{x^4 + 2}$, then $du = \answer{4x^3 dx}$.\\
\begin{hint}
Don't forget the `dx' in your answer for `du'.
\end{hint}
Convert to an integral in the variable $u$:
\[\int 4x^3 \sqrt{x^4 +2} \ dx = \int\answer{\sqrt u du}\]
\begin{hint}
Don't forget the `du' in your integral.
\end{hint}

\[\int 4x^3 \sqrt{x^4 +2} \ dx = \answer{2/3(x^4 +2)^{3/2}} +C.\]
\end{problem}



\begin{example}[example 5] 
Compute 
\[\int \frac{2x}{x^2 + 1} \ dx.\]
Let $u = x^2 + 1$.  We have,
\[u = x^2 + 1\]
\[du = 2x \ dx\]

\[\int \frac{2x}{x^2 + 1} \ dx = \int \frac{1}{x^2 + 1} \cdot 2x\  dx = \int \frac{1}{u} \ du.\]
The last integral can be computed as 
\[\int \frac{1}{u} \ du = \ln|u| + C\]
and by back substituting, we have 
\[\ln|u| + C =  \ln|x^2 + 1| + C=\ln(x^2 + 1) + C.\]
Thus, using u-substitution we can conclude that
\[\int \frac{2x}{x^2 + 1} \ dx =  \ln(x^2 + 1) + C.\]
\end{example}



\begin{problem} (problem 5) 
Compute $\displaystyle{\int \frac{4x^3}{x^4 +2} \ dx}$.\\
Let $u = \answer{x^4 + 2}$, then $du = \answer{4x^3 dx}$.\\
\begin{hint}
Don't forget the `dx' in your answer for `du'.
\end{hint}
Convert to an integral in the variable $u$:
\[\int \frac{4x^3}{x^4 +2} \ dx = \int\answer{1/u du}\]
\begin{hint}
Don't forget the `du' in your integral.
\end{hint}

\[\int \frac{4x^3}{x^4 +2} \ dx = \answer{\ln|x^4 +2|} +C.\]
\end{problem}



\begin{example}[example 6] Compute 
\[\int e^x\sin(e^x) \ dx.\]
We let $u = e^x$.  We have,
\[u = e^x\]
\[du = e^x \ dx\]

and the integral can be written as 
\[\int e^x\sin(e^x) \ dx = \int \sin(e^x) \cdot e^x \  dx = \int \sin u \ du.\]
The last integral can be computed as 
\[\int \sin u \ du = -\cos u + C\]
and by back substituting, we have 
\[-\cos u + C = -\cos(e^x) + C.\]
Thus, using u-substitution we can conclude that
\[\int e^x\sin(e^x) \ dx =  -\cos(e^x) + C.\]
\end{example}



\begin{problem}(problem 6a) 
Compute $\displaystyle{\int e^x\cos(e^x) \ dx}$.\\
Let $u = \answer{e^x}$, then $du = \answer{e^x dx}$.\\
\begin{hint}
Don't forget the `dx' in your answer for `du'.
\end{hint}
Convert to an integral in the variable $u$:
\[\int e^x\cos(e^x) \ dx = \int\answer{e^u du}\]
\begin{hint}
Don't forget the `du' in your integral.
\end{hint}

\[\int e^x\cos(e^x) \ dx = \answer{\sin(e^x)} +C.\]
\end{problem}



\begin{problem}(problem 6b) 
Compute $\displaystyle{\int \frac{\cos(\ln(x))}{x} \ dx}$.\\
Let $u = \answer{\ln(x)}$, then $du = \answer{1/x dx}$.\\
\begin{hint}
Don't forget the `dx' in your answer for `du'.
\end{hint}
Convert to an integral in the variable $u$:
\[\int \frac{\cos(\ln(x))}{x} \ dx = \int\answer{\cos u du}\]
\begin{hint}
Don't forget the `du' in your integral.
\end{hint}

\[\int \frac{\cos(\ln(x))}{x} \ dx = \answer{\sin(\ln(x))} +C.\]
\end{problem}



\begin{example}[example 7] Compute 
\[\int 3x^2\sec(x^3)\tan(x^3) \ dx.\]
Let $u = x^3$.  Then we have,
\[u = x^3\]
\[du = 3x^2 \ dx\]

and the integral can be written as 
\begin{align*}
\int 3x^2\sec(x^3)\tan(x^3) \ dx &= \int \sec(x^3)\tan(x^3) \cdot 3x^2 \ dx\\
&= \int \sec u\tan u \ du.
\end{align*}
The last integral can be computed as 
\[\int \sec u\tan u \ du = \sec u + C\]
and by back substituting, we have 
\[\sec u + C = \sec(x^3) + C.\]
Thus, using u-substitution we can conclude that
\[\int 3x^2\sec(x^3)\tan(x^3) \ dx =  \sec(x^3) + C.\]
\end{example}



\begin{problem}(problem 7a)
\begin{hint}
Let $u = e^x$
\end{hint}
\begin{hint}
Compute $du$
\end{hint}
\[\int e^x\sec(e^x)\tan(e^x) \ dx = \answer{\sec(e^x)} +C.\]
\end{problem}



\begin{problem}(problem 7b)
\begin{hint}
Let $u = x^2$
\end{hint}
\begin{hint}
Compute $du$
\end{hint}
\[\int 2x\csc(x^2)\cot(x^2) \ dx = \answer{-\csc(x^2)} +C.\]
\end{problem}



\begin{example}[example 8] Compute 
\[\int x^3\cos(x^4) \ dx.\]
Let $u = x^4$.  Then,
\[u = x^4\]
\[du = 4x^3 \ dx\]

and the integral can be written as 
\begin{align*}
\int x^3\cos(x^4) \ dx &= \int \cos(x^4) \cdot x^3\  dx \\
&=  \int \cos(x^4)\cdot \tfrac14 \cdot 4x^3\  dx\\
&=  \int \tfrac14\cos u \ du.
\end{align*}
The last integral can be computed as 
\[\int \tfrac14 \cos u \ du = \tfrac14 \sin u + C\]
and by back substituting, we have 
\[\tfrac14 \sin u + C = \tfrac14 \sin(x^4) + C.\]
Thus, using u-substitution we can conclude that
\[\int x^3\cos(x^4) \ dx =  \tfrac14 \sin(x^4) + C.\]
\end{example}

\begin{problem}(problem 8)
\begin{hint}
Let $u = x^2$
\end{hint}
\begin{hint}
Compute $du$
\end{hint}
\[\int x\cos(x^2) \ dx = \answer{\sin(x^2)/2} +C.\]
\end{problem}



\begin{example}[example 9] 
Compute 
\[\int xe^{-x^2} \ dx.\]
Let $u = -x^2 $.  Then we have,
\[u = -x^2\]
\[du = -2x \ dx\]
and the integral can be written as
\begin{align*}
\int xe^{-x^2} \ dx &= \int e^{-x^2} \cdot x\  dx \\
&=  \int e^{-x^2}( -\tfrac12)\ (-2x)\  dx \\
&=  \int -\tfrac12 e^u \ du.
\end{align*}
The last integral can be computed as 
\[ \int -\tfrac12 e^u \ du = -\tfrac12 e^u + C\]
and by back substituting, we have 
\[-\tfrac12 e^u + C = -\tfrac12 e^{-x^2} + C.\]
Thus, using u-substitution we can conclude that
\[\int xe^{-x^2} \ dx =  -\tfrac12 e^{-x^2} + C.\]
\end{example}



\begin{problem}(problem 9a)
\begin{hint}
Let $u = x^3$
\end{hint}
\begin{hint}
Compute $du$
\end{hint}
\[\int x^2e^{x^3} \ dx = \answer{e^{x^3}/3} +C.\]
\end{problem}



\begin{problem}(problem 9b)
\begin{hint}
Let $u = \sqrt x$
\end{hint}
\begin{hint}
Compute $du$
\end{hint}
\[\int \frac{e^{\sqrt x}}{\sqrt x} \ dx = \answer{2e^{\sqrt x}} +C.\]
\end{problem}



\begin{example}[example 10] Compute 
\[\int \sin(3x) \ dx.\]
Let $u = 3x$.  Then we have,
\[u = 3x\]
\[du = 3 \ dx\]
and the integral can be written as 
\[\int\sin(3x) \ dx =  \int \sin(3x) \cdot \tfrac13\cdot 3 \   dx =   \int \tfrac13 \sin u \ du.\]
The last integral can be computed as 
\[ \int \tfrac13 \sin u \ du = -\tfrac13 \cos u  + C\]
and by back substituting, we have 
\[-\tfrac13 \cos u + C = -\tfrac13 \cos(3x) + C.\]
Thus, using u-substitution we can conclude that
\[\int \sin(3x) \ dx =  -\tfrac13 \cos(3x) + C.\]
\end{example}



\begin{problem}(problem 10)
\begin{hint}
Let $u = 3x$
\end{hint}
\begin{hint}
Compute $du$
\end{hint}
\[\int \cos(3x) \ dx = \answer{1/3 \sin(3x)} +C.\]
\end{problem}






\begin{example}[example 11] Compute 
\[\int e^{\frac{x}{2}} \ dx.\]
Let $u = \frac{x}{2}$.  Then we have,
\[u = \frac{x}{2}\]
\[du = \tfrac12 \ dx\]
and the integral can be written as 
\[\int e^{\frac{x}{2}} \ dx =  \int e^{\frac{x}{2}} \cdot 2\cdot \tfrac{1}{2}  \   dx =   \int 2e^u \ du.\]
The last integral can be computed as 
\[\int 2e^u \ du = 2 e^u + C\]
and by back substituting, we have 
\[2e^u + C = 2e^{\frac{x}{2}}+ C.\]
Thus, using u-substitution we can conclude that
\[\int e^{x/2} \ dx = 2e^{x/2} + C.\]
\end{example}



\begin{problem}(problem 11)
\begin{hint}
Let $u = 5x$
\end{hint}
\begin{hint}
Compute $du$
\end{hint}
\[\int e^{5x} \ dx = \answer{1/5 e^{5x}} +C.\]
\end{problem}



\begin{example}[example 12] Compute 
\[\int (4x+3)^5 \ dx.\]
Let $u = 4x+3$. Then we have,
\[u = 4x+3\]
\[du = 4 \ dx\]
and the integral can be written as 
\[\int (4x+3)^5 \ dx =   \int (4x+3)^5 \cdot \tfrac14\cdot 4  \   dx =   \int \tfrac14 u^5 \ du.\]
The last integral can be computed as 
\[\tfrac14  \int u^5 \ du = \tfrac14  \cdot \tfrac{u^6}{6} + C = \tfrac{u^6}{24} + C\]
and by back substituting, we have 
\[\tfrac{u^6}{24} + C = \tfrac{(4x+3)^6}{24}+ C.\]
Thus, using u-substitution we can conclude that
\[\int (4x+3)^5 \ dx = \tfrac{1}{24}(4x+3)^6 + C.\]
\end{example}




\begin{problem}(problem 12)
\begin{hint}
Let $u = 2x - 5$
\end{hint}
\begin{hint}
Compute $du$
\end{hint}
\[\int (2x - 5)^4 \ dx = \answer{\frac{1}{10}(2x-5)^5} +C.\]
\end{problem}



\begin{example}[example 13] Compute 
\[\int \frac{1}{x\ln^2 x} \ dx.\]
Let $u = \ln(x)$. Then we have,
\[u = \ln(x)\]
\[du = \tfrac1x \ dx\]
and the integral can be written as 
\[\int \frac{1}{x\ln^2(x)} \ dx = \int \frac{1}{\ln^2(x)} \cdot \frac{1}{x}\  dx = \int \frac{1}{u^2} \ du.\]
The last integral can be computed as 
\[\int \frac{1}{u^2} \ du = \int u^{-2} \ du = \tfrac{u^{-1}}{-1} + C 
= -\frac{1}{u} + C\]
and by back substituting, we have 
\[-\frac{1}{u} + C =  -\frac{1}{\ln x} + C.\]
Thus, using u-substitution we can conclude that
\[\int \frac{1}{x\ln^2 x} \ dx =  -\frac{1}{\ln x} + C.\]
\end{example}



\begin{problem}(problem 13)
\begin{hint}
Let $u = \ln x$
\end{hint}
\begin{hint}
Compute $du$
\end{hint}
\[\int \frac{1}{x\ln^3 x} \ dx = \answer{- \ln^{-2} x/2} +C.\]
\end{problem}



\begin{example}[example 14] Compute 
\[\int \sin^4 x\cos x \ dx.\]
Let $u = \sin x$. Then we have,
\[u = \sin x\]
\[du = \cos x \ dx\]
and the integral can be written as 
\[\int \sin^4 x\cos x \ dx  = \int u^4 \ du.\]
The last integral can be computed as 
\[\int u^4 \ du = \tfrac{u^5}{5} + C\]
and by back substituting, we have 
\[\tfrac{u^5}{5} + C = \tfrac15 \sin^5 x + C.\]
Thus, using u-substitution we can conclude that
\[\int \sin^4 x\cos x \ dx =  \tfrac15 \sin^5 x + C.\]
\end{example}



\begin{problem}(problem 14a)
\begin{hint}
Let $u = \cos x$
\end{hint}
\begin{hint}
Compute $du$
\end{hint}
\[\int \cos^3 x\sin x \ dx = \answer{-\cos^4 x/4} +C.\]
\end{problem}



\begin{problem}(problem 14b)
\begin{hint}
Let $u = \tan x$
\end{hint}
\begin{hint}
Compute $du$
\end{hint}
\[\int \tan^5 x\sec^2 x \ dx = \answer{\tan^6 x/6} +C.\]
\end{problem}



\begin{example}[example 15] Compute 
\[\int \tan x \ dx.\]
First rewrite the integral:
\[\int \tan x \ dx =\int \frac{\sin x}{\cos x} \ dx.\]
Now, let $u = \cos x$; then $du = -\sin x \ dx$
and the integral can be written as
\begin{align*}
\int \frac{\sin x}{\cos x} \ dx &= \int \frac{1}{\cos x}\ \sin x \  dx \\
 &=  - \int \frac{1}{\cos x}\ \big(-\sin x\big) \  dx\\
&=-\int \frac{1}{u} \ du.
\end{align*}
The last integral can be computed as 
\[-\int \frac{1}{u} \ du = -\ln|u| + C\]
and by back substituting, we have 
\[-\ln|u| + C = -\ln|\cos x| + C = \ln|\sec x| +C.\]
Thus, using u-substitution we can conclude that
\[\int \tan x \ dx =  \ln|\sec x| + C.\]
\end{example}



\begin{problem}(problem 15)
\begin{hint}
Rewrite: $\cot x = \frac{\cos x}{\sin x}$
\end{hint}
\begin{hint}
Let $u = \sin x$
\end{hint}
\begin{hint}
Compute $du$
\end{hint}
\[\int \cot x \ dx = \answer{\ln|\sin x|} +C.\]
\end{problem}



\begin{example}[example 16] Compute 
\[\int \sec x \ dx.\]
First rewrite the integral:
\[\int \sec x \ dx =\int \sec x\frac{\sec x+\tan x}{\sec x+\tan x} \ dx.\]
Distributing in the numerator, we get
\[\int \sec x\frac{\sec x + \tan x}{\sec x +\tan x} \ dx = \int \frac{\sec^2 x +\sec x\tan x}{\sec x +\tan x} \ dx.\]
Now, let $u = \sec x + \tan x$, then $du = [\sec x\tan x + \sec^2 x] \ dx$ and the integral can be rewritten as
\[ \int \frac{\sec^2 x+\sec x\tan x}{\sec x+\tan x} \ dx = \int \frac{1}{u} \ du.\]
The last integral can be computed as
\[\int \frac{1}{u} \ du = \ln|u| + C\]
and by back substituting, we have 
\[\ln|u| + C = \ln|\sec x + \tan x| + C.\]
Thus, using u-substitution we can conclude that
\[\int \sec x \ dx =  \ln|\sec x + \tan x| + C.\]
\end{example}



\begin{center}
\begin{foldable}
\unfoldable{Here is a detailed, lecture style video on u-substitution:}
\youtube{5yb7_e9PCQU}
\end{foldable}
\end{center}

\end{document}
