\documentclass[handout]{ximera}
\usepackage{tcolorbox}
\input{../preamble}
\outcome{Compute derivatives involving inverse trig functions.}


\title{2.9 Derivatives of Inverse Trig Functions}


\begin{document}

\begin{abstract}
In this section we compute derivatives involving $\tan^{-1}(x), \sin^{-1}(x)$ and $\cos^{-1}(x)$.
\end{abstract}

\maketitle


We begin by computing the derivative of the inverse trigonometric function $f(x) = \tan^{-1}(x)$.  
The following Pythagorean trigonometric identity will be needed:


\[
1 + \tan^2(\theta) = \sec^2(\theta).
\]
This identity follows from $\cos^2(\theta) + \sin^2(\theta) = 1$ by dividing both sides by $\cos^2(\theta)$.

We begin the derivation by using the fact that $\tan(x)$ and $\tan^{-1}(x)$ are inverse functions, so that:

\[
\tan(\tan^{-1}(x)) = x.
\]

We differentiate both sides of this equation with respect to $x$:

\[
\dd{x} \tan(\tan^{-1}(x)) = \ddx x.
\]

Using the Chain Rule on the left side gives:

\[
\sec^2(\tan^{-1}(x)) \ddx \left[\tan^{-1}(x)\right] = 1.
\]

Now, we can solve this for the derivative of $\tan^{-1}(x)$:

\[
 \ddx \left[\tan^{-1}(x)\right] = \frac{1}{\sec^2\left(\tan^{-1}(x)\right)}.
\]

Next, we use the Pythagorean Identity:

\[
 \ddx \left[\tan^{-1}(x)\right] = \frac{1}{1 + \tan^2\left(\tan^{-1}(x)\right)}.
\]

Finally, using the property of inverse functions:

\[
 \ddx \left[\tan^{-1}(x)\right] = \frac{1}{1 + x^2}.
\]


Similar arguments can show that:

\[
 \ddx \left[\sin^{-1}(x)\right] = \frac{1}{\sqrt{1 - x^2}} \;\;\text{  and  } \;\;\ddx \left[\cos^{-1}(x)\right] = -\frac{1}{\sqrt{1 - x^2}}.
\]



\begin{foldable}
\unfoldable{Below is a graph of $f(x) = \tan^{-1}(x)$ (in blue) and its derivative, $f'(x) = \tfrac{1}{1+x^2}$ (in purple).
Notice that the slope of the tangent line to $f(x)$ (in red) is the height of the corresponding 
point on $f'(x)$. Use it to see a graphical representation of the answers to the problem above.}
\includeinteractive{invtanwithderiv.js}
\end{foldable}







\begin{example}[example 1]

Find the equation of the tangent line to the graph of $f(x) = \tan^{-1}(x)$ at $x=0.$\\
The point of tangency is $(0, f(0)) = (0, 0)$ since $\tan^{-1}(0) = 0$.
The slope of the tangent line is given by  $m = f'(0) = \tfrac{1}{1+0^2} = 1$.
To create the equation of the line we use the
Point slope form: $y-y_0 = m(x-x_0)$ and we get $y-0 = 1(x-0)$ or $y=x$.

\end{example}





\begin{problem}(problem 1a)
Find the equation of the tangent line to the graph of $f(x) = \tan^{-1}(x)$ at $x=1.$

\begin{hint}
The point of tangency is $(1, f(1))$
\end{hint}
\begin{hint}
Use the derivative to find the slope, $m$
\end{hint}
\begin{hint}
Point slope form: $y-y_0 = m(x-x_0)$
\end{hint}

The equation of the tangent line is \ $y = \answer{x/2 + \pi/4 - 1/2}$

\end{problem}



\begin{problem}(problem 1b)

Find the equation of the tangent line to the graph of $f(x) = \sin^{-1}(x)$ at $x=0.$

\begin{hint}
The point of tangency is $(0, f(0))$
\end{hint}
\begin{hint}
Use the derivative to find the slope, $m$
\end{hint}
\begin{hint}
Point slope form: $y-y_0 = m(x-x_0)$
\end{hint}

The equation of the tangent line is \ $y = \answer{x}$

\end{problem}



\begin{problem}(problem 1c)

Find the equation of the tangent line to the graph of $f(x) = \cos^{-1}(x)$ at $x=0.$

\begin{hint}
The point of tangency is $(0, f(0))$
\end{hint}
\begin{hint}
Use the derivative to find the slope, $m$
\end{hint}
\begin{hint}
Point slope form: $y-y_0 = m(x-x_0)$
\end{hint}

The equation of the tangent line is \ $y = \answer{-x + \pi/2}$

\end{problem}


\begin{example}[example 2]
Find $h'(x)$ if $h(x) = (1+x^2)\tan^{-1}(x)$.\\
We write $h(x)$ as a product: $h(x) = f(x)\cdot g(x)$ with
\[f(x) = 1+x^2 \quad \text{and} \quad g(x) = \tan^{-1}(x).\]
To use the product rule we need the derivatives:
\[f'(x) = 2x \quad \text{and} \quad g'(x) = \frac{1}{1+x^2}.\]
We can now write the derivative:
\begin{align*}
h'(x) &= f'(x)g(x) + f(x)g'(x) \\
&= 2x\tan^{-1}(x)  + (1+x^2)\frac{1}{1+x^2} \\
&=  2x\tan^{-1}(x) + 1.
\end{align*}
\end{example}


\begin{center}
\begin{foldable}
\unfoldable{Here is a video of the preceding example}
\youtube{NvlgmABasiQ} %vid of example 6
\end{foldable}
\end{center}



\begin{problem}(problem 2a)
  Compute
  \[
  \frac{d}{dx} x^3 \tan^{-1}(x)
  \]
  
    \begin{hint}
      Use the Product Rule with $x^3$ and $\tan^{-1}(x)$.
    \end{hint}
    \begin{hint}
      $(fg)' = f'g+g'f$.
    \end{hint}
    \begin{hint}
      The derivative of $x^3$ is $3x^2$
    \end{hint}
    \begin{hint}
      The derivative of $\tan^{-1}(x)$ is $\frac{1}{1+x^2}$
    \end{hint}
		The derivative of $x^3\tan^{-1}(x)$ with respect to $x$ is
		 $\answer{3x^2 \tan^{-1}(x) + \frac{x^3}{1+x^2}}$
		
\end{problem}

\begin{problem}(problem 2b)
  Compute
  \[
  \frac{d}{dx} (1-x^2) \sin^{-1}(x)
  \]
  
    \begin{hint}
      Use the Product Rule with $1-x^2$ and $\sin^{-1}(x)$.
    \end{hint}
    \begin{hint}
      $(fg)' = f'g+g'f$.
    \end{hint}
    \begin{hint}
      The derivative of $1 - x^2$ is $-2x$
    \end{hint}
    \begin{hint}
      The derivative of $\sin^{-1}(x)$ is $\frac{1}{\sqrt{1-x^2}}$
    \end{hint}
		\begin{hint}
       $(1-x^2) \frac{1}{\sqrt{1-x^2}} = \sqrt{1-x^2}$
    \end{hint}
		The derivative of $(1-x^2)\sin^{-1}(x)$ with respect to $x$ is
		 $\answer{-2x \sin^{-1}(x) + \sqrt{1-x^2}}$
		
\end{problem}


The Chain Rule versions of these formulas are:


\[
 \ddx \left[\tan^{-1}(g(x))\right] = \frac{g'(x)}{1 + g^2(x)},
\]
\[
 \ddx \left[\sin^{-1}(g(x))\right] = \frac{g'(x)}{\sqrt{1 - g^2(x)}}
\]

and

\[
 \ddx \left[\cos^{-1}(g(x))\right] = -\frac{g'(x)}{\sqrt{1 - g^2(x)}}.
\]


\begin{example}[example 3]
Find $h'(x)$ if $h(x) = \tan^{-1}(4x)$.\\
We write $h(x)$ as a composition: $h(x)=f(g(x))$ with 
\[g(x) = 4x  \quad \text{and} \quad  f(x) = \tan^{-1}(x).\]
 To find $h'(x)$ we need $f'(g(x))$ and $g'(x)$.  First, 
\[g'(x) = 4; \quad \text{next} \] 
\[f'(x) = \frac{1}{1+x^2} , \quad \text{so}\]
\[ f'(g(x)) = \frac{1}{1+g^2(x)} =\frac{1}{1+(4x)^2}=\frac{1}{1+16x^2}.\]
By the chain rule,
\[h'(x) = f'(g(x))g'(x) = \frac{1}{1+16x^2} \cdot 4 = \frac{4}{1+16x^2}.\]
\end{example}

\begin{center}
\begin{foldable}
\unfoldable{Here is a video of the example}
\youtube{-0ZwkfU9Xec}  %vid of example 14
\end{foldable}
\end{center}


\begin{problem}(problem 3a)
  Compute
  \[
  \frac{d}{dx} \tan^{-1}(3x)
  \]
  
    \begin{hint}
      The chain rule says:
      \[
      \frac{d}{dx} f(g(x)) = f'(g(x))\cdot g'(x)
      \]
    \end{hint}
    \begin{hint}
      The outside function is $f(x) = \tan^{-1}(x)$ and the inside
      function is $g(x) = 3x$.
    \end{hint}
    \begin{hint}
		  Leave the inside in, $f'(g(x))$
		\end{hint}
		\begin{hint}
		  Multiply by the derivative of the inside, $g'(x)$
		\end{hint}
    
		The derivative of $\tan^{-1}(3x)$ with respect to $x$ is
		 $\answer{\frac{3}{1+(3x)^2}}$
		
\end{problem}



\begin{problem}(problem 3b)
Find the equation of the tangent line to the graph of $f(x) = \cos(x)$ at $x=\pi/2.$


\begin{hint}
The point of tangency is $(\pi/2, f(\pi/2))$
\end{hint}
\begin{hint}
Use the derivative to find the slope, $m$
\end{hint}
\begin{hint}
Point slope form: $y-y_0 = m(x-x_0)$
\end{hint}

The equation of the tangent line is \ $y = \answer{-x + \pi/2}$

\end{problem}




\end{document}




