\documentclass{ximera}

\input{../preamble}

\outcome{Find the sum of a geometric series}

\title{Geometric Series}

\begin{document}

\begin{abstract}
We find the sum of a geometric series.
\end{abstract}

\maketitle

\section{Geometric Series}

\begin{definition}[Geometric Series] A \textbf{geometric series} is an infinite series of the form
\[
\sum_{n=0}^\infty ar^n = a + ar + ar^2 + ar^3 + \cdots.
\]
The parameter $r$ is called the \textbf{common ratio}.
\end{definition}

\begin{example}[example 1]
Consider the series:
\[
 \sum_{n=0}^\infty \frac{3}{2^n} 
 \]
 Write out the first four terms of the series. If the series is geometric, find the common ratio.
 
 The first four terms are \[
 3 + \frac32 + \frac34 + \frac38 + \cdots.
 \]

 The series is geometric and the common ratio is $\frac12$.
 \end{example}
 
 

\begin{problem}(problem 1a)
 Consider the series:
 \[
 \sum_{n=0}^\infty \frac{2}{3^n} 
 \]
 Is this series geometric?
 \begin{multipleChoice}
 \choice[correct]{yes}
 \choice{no}
 \end{multipleChoice}
 
 The first term is $a = \answer{2}$\\
 The common ratio is $r = \answer{1/3}$
 \end{problem}
 
 
 \begin{problem}(problem 1b)
 Consider the series:
 \[
 \sum_{n=2}^\infty \frac{3}{2^n} 
 \]
 Is this series geometric?
 \begin{multipleChoice}
 \choice[correct]{yes}
 \choice{no}
 \end{multipleChoice}
 
 The first term is $a = \answer{3/4}$\\
 The common ratio is $r = \answer{1/2}$
 \end{problem}
 
 
 \begin{example}[example 2]
 Consider the series:
\[
 \sum_{n=1}^\infty \frac{3}{n^2} 
 \]
 Write out the first four terms of the series. If the series is geometric, find the common ratio.
 
 The first four terms are 
 \[
 3 + \frac34 + \frac39 + \frac{3}{16} + \cdots.
 \]
 The ratio of the second term to the first is $\frac14$ but the ratio of the third term to the second is $\frac49$.
 The series is not geometric because it fails to have a \it{common} ratio.
 
 \end{example}
 
 
  \begin{problem}(problem 2a)
 Consider the series:
 \[
 \sum_{n=2}^\infty \frac{3}{2^n} 
 \]
 Is this series geometric?
 \begin{multipleChoice}
 \choice{yes}
 \choice[correct]{no}
 \end{multipleChoice}
 
 \end{problem}
 
 
   \begin{problem}(problem 2a)
 Consider the series:
 \[
 \sum_{n=1}^\infty \frac{1}{n} 
 \]
 Is this series geometric?
 \begin{multipleChoice}
 \choice{yes}
 \choice[correct]{no}
 \end{multipleChoice}
 
 \end{problem}
 

   \begin{problem}(problem 2b)
 Consider the series:
 \[
 \sum_{n=1}^\infty \sqrt n 
 \]
 Is this series geometric?
 \begin{multipleChoice}
 \choice{yes}
 \choice[correct]{no}
 \end{multipleChoice}
 
 \end{problem}
 
 
\section{Convergence}

\begin{theorem}[Convergence of Geometric Series] 
The geometric series
\[
\sum_{n=0}^\infty ar^n
\]
converges if and only if the common ratio $r$ satisfies the condition $-1 < r < 1$.
This condition can also be written as $|r| < 1$.
\end{theorem}

\begin{example}[example 3]
Does the geometric series $\displaystyle{\sum_{n=0}^\infty \frac{3}{2^n}}$ converge or diverge?\\
The common ratio of this geometric series is $r = \frac12$. Since $-1 < \frac 12 < 1$,
the series converges.
\end{example}


\begin{problem}(problem 3a)
 Does the geometric series
 \[
 \sum_{n=2}^\infty \frac{3}{2^n} 
 \]
 converge or diverge?\\
 The common ratio is $r = \answer{1/2}$\\
 The series
 \begin{multipleChoice}
 \choice[correct]{converges}
 \choice{diverges}
 \end{multipleChoice}
 \end{problem}
 

\begin{problem}(problem 3b)
 Does the geometric series
 \[
 \sum_{n=1}^\infty (-1)^n\frac{2}{3^n} 
 \]
 converge or diverge?\\
 The common ratio is $r = \answer{-1/3}$\\
 The series
 \begin{multipleChoice}
 \choice[correct]{converges}
 \choice{diverges}
 \end{multipleChoice}
 \end{problem}
 
 \begin{problem}(problem 3c)
 Does the geometric series
 \[
 \sum_{n=0}^\infty (-2)^n 
 \]
 converge or diverge?\\
 The common ratio is $r = \answer{-2}$\\
 The series
 \begin{multipleChoice}
 \choice{converges}
 \choice[correct]{diverges}
 \end{multipleChoice}
 \end{problem}
 
 
 
 
\begin{example}[example 4]
Does the geometric series $\displaystyle{\sum_{n=0}^\infty \frac{3^n}{2^{n+1}}}$ converge or diverge?\\
The common ratio of this geometric series is $r = \frac32$. Since $\frac32$ is not between $-1$ and $1$,
the series does not converge, i.e., it diverges.
\end{example}

\begin{problem}(problem 4a)
 Does the geometric series
 \[
 \sum_{n=0}^\infty \frac{2^{n+1}}{3^n} 
 \]
 converge or diverge?\\
 The common ratio is $r = \answer{2/3}$\\
 The series
 \begin{multipleChoice}
 \choice[correct]{converges}
 \choice{diverges}
 \end{multipleChoice}
 \end{problem}
 
 
 \begin{problem}(problem 4b)
 Does the geometric series
 \[
 \sum_{n=0}^\infty \frac{2^{2n}}{3^n} 
 \]
 converge or diverge?\\
 The common ratio is $r = \answer{4/3}$\\
 The series
 \begin{multipleChoice}
 \choice{converges}
 \choice[correct]{diverges}
 \end{multipleChoice}
 \end{problem}
 

\begin{example}[example 5]
Does the geometric series $\displaystyle{\sum_{n=0}^\infty \left(-\frac23\right)^n }$ converge or diverge?\\
The common ratio of this geometric series is $r = -\frac23$. Since $-1 < -\frac23 < 1$,
the series converges.
\end{example}

\begin{problem}(problem 5)
 Does the geometric series
 \[
 \sum_{n=0}^\infty \left(-\frac56 \right)^n
 \]
 converge or diverge?\\
 The common ratio is $r = \answer{-5/6}$\\
 The series
 \begin{multipleChoice}
 \choice[correct]{converges}
 \choice{diverges}
 \end{multipleChoice}
 \end{problem}

\section{Sum of a Geometric Series}

Consider the geometric series $\sum_{n=0}^\infty ar^n$ where $|r| < 1$ (so that the series converges).
The $N^{th}$ partial sum of this series is given by
\[
S_N = \sum_{n=0}^N ar^n = a + ar + ar^2 + \cdots + ar^{N-1} + ar^N.
\]
Multiply both sides by $r$:
\[
rS_N =  ar + ar^2 + + ar^3 + \cdots  + ar^N + ar^{N+1}.
\] 
Now subtract $rS_N$ from $S_N$:
\begin{align*}
S_N - rS_N &= \left(a + ar + \cdots + ar^{N-1} + ar^N\right) - \left(ar + ar^2 + \cdots  + ar^N + ar^{N+1} \right)\\
           &= a - ar^{N+1}.
\end{align*}
We can factor out $S_N$ on the left side and then divide by $1-r$ to obtain
\[
S_N = \frac{a - ar^{N+1}}{1-r}.
\]
We can now compute the sum of the geometric series by taking the limit as $N \to \infty$:
\[
S = \sum_{n=0}^\infty ar^n = \lim_{N \to \infty} \sum_{n=0}^N ar^n = \lim_{N \to \infty} S_N = \lim_{N \to \infty} \frac{a - ar^{N+1}}{1-r} = \frac{a}{1-r}.
\]
We present this formula in the theorem below.

\begin{theorem}[Sum of a Geometric Series]
If $-1 < r < 1$, then the sum of the geometric series 
\[
\sum_{n=0}^\infty ar^n = a + ar + ar^2 + \cdots
\] is given by 
\[
S = \frac{a}{1-r}.
\]
That is, if $-1 < r < 1$, then
\[
\sum_{n=0}^\infty ar^n = \frac{a}{1-r}.
\]
\end{theorem}

\begin{example}[example 6]
Find the sum of the geometric series 
\[
\sum_{n=0}^\infty \frac{3}{2^n}.
\]
The first term is $a = 3$, and the common ratio is $r = \frac12$. The sum of the series is
\[
\sum_{n=0}^\infty \frac{3}{2^n} = \frac{3}{1-\frac12} = \frac{3}{\left(\frac12\right)} = 6.
\]
\end{example}


\begin{problem}(problem 6a)
Find the sum of the geometric series 
\[
\sum_{n=0}^\infty \frac{5}{3^n}.
\]
The first term is $a = \answer{5}$\\
The common ratio is $r = \answer{1/3}$\\
The sum is $S= \answer{15/2}$

\end{problem}

\begin{problem}(problem 6b)
Find the sum of the geometric series 
\[
\sum_{n=1}^\infty \frac{4}{2^n}.
\]
The first term is $a = \answer{4}$\\
The common ratio is $r = \answer{1/2}$\\
The sum is $S= \answer{8}$

\end{problem}

\begin{problem}(problem 6c)
Find the sum of the geometric series 
\[
\sum_{n=0}^\infty \frac{3^n}{2^{2n}}.
\]
The first term is $a = \answer{1}$\\
The common ratio is $r = \answer{3/4}$\\
The sum is $S= \answer{4}$

\end{problem}



\begin{example}[example 7]
Find the sum of the geometric series 
\[
\sum_{n=0}^\infty \left(-\frac23\right)^n.
\]
The first term is $a = 1$, and the common ratio is $r = -\frac23$. The sum of the series is
\[
\sum_{n=0}^\infty \left(-\frac23\right)^n = \frac{1}{1-\left(-\frac23\right)} = \frac{1}{1 + \frac23} = \frac{1}{\left(\frac53\right)} = \frac35.
\]
\end{example}

\begin{problem}(problem 7a)
Find the sum of the geometric series 
\[
\sum_{n=1}^\infty \left(-\frac45\right)^n
\]
The first term is $a = \answer{-4/5}$\\
The common ratio is $r = \answer{-4/9}$\\
The sum is $S= \answer{4}$

\end{problem}


\begin{problem}(problem 7b)
Find the sum of the geometric series 
\[
\sum_{n=2}^\infty \left(-\frac{2}{\pi}\right)^n
\]
The first term is $a = \answer{4/\pi^2}$\\
The common ratio is $r = \answer{-2/\pi}$\\
The sum is $S= \answer{4/(\pi^2 + \pi)}$

\end{problem}

\begin{problem}(problem 7c)
Find the sum of the geometric series 
\[
\sum_{n=0}^\infty \left(\frac{2}{e}\right)^n
\]
The first term is $a = \answer{1}$\\
The common ratio is $r = \answer{2/e}$\\
The sum is $S= \answer{e/(e-2)}$

\end{problem}

\section{Video Lesson}


\begin{center}
\begin{foldable}
\unfoldable{Here is a detailed, lecture style video on Geometric Series:}
\youtube{oM28tybb_AE}
\end{foldable}
\end{center}


\section{More Problems}


\end{document}


\begin{example} %example #15
Find $h'(x)$ if $h(x) = x^{\sin(x)}$.\\
We will use the fact that the exponential and logarithm functions are inverses,
\[e^{\ln(x)} = x,\]
and the exponent property of logarithms, 
\[\ln(x^n) = n\ln(x),\]
to rewrite $h(x)$.  We have 
\[h(x) = x^{\sin(x)} = e^{\ln(x^{\sin(x)})} = e^{\sin(x)\ln(x)}\]
and we can now compute $h'(x)$ using a combination of the chain rule and product rule.
We can write $h(x)$ as a composition, $f(g(x))$ with 
\[g(x) = \sin(x)\ln(x) \quad \text{and} \quad f(x) = e^x.\]
Then to find $g'(x)$ we us the product rule and we get $g'(x) = \frac{\sin(x)}{x} + \cos(x)\ln(x)$.
Next $f'(x) = e^x$ and 
hence $f'(g(x)) = e^{g(x)} = e^{\sin(x)\ln(x)} = x^{\sin(x)}$.
We can then conclude $h'(x) = f'(g(x))g'(x) = x^{\sin(x)} \left[ \frac{\sin(x)}{x} + \cos(x)\ln(x)\right]$.
\end{example}

%more question formats below













%\begin{verbatim}
\begin{question}
What is your favorite color?
\begin{multipleChoice}
\choice[correct]{Rainbow}
\choice{Blue}
\choice{Green}
\choice{Red}
\end{multipleChoice}
\begin{freeResponse}
Hello
\end{freeResponse}
\end{question}
%\end{verbatim}





\begin{question}
  Which one will you choose?
  \begin{multipleChoice}
    \choice[correct]{I'm correct.}
    \choice{I'm wrong.}
    \choice{I'm wrong too.}
  \end{multipleChoice}
\end{question}


\begin{question}
  Which one will you choose?
  \begin{selectAll}
    \choice[correct]{I'm correct.}
    \choice{I'm wrong.}
    \choice[correct]{I'm also correct.}
    \choice{I'm wrong too.}
  \end{selectAll}
\end{question}


\begin{freeResponse}
What is the chain rule used for?
\end{freeResponse}
