\documentclass[handout]{ximera}

\input{../preamble}

\outcome{Find the Taylor Series for a Function}

\title{3.15 Taylor Series}

\begin{document}

\begin{abstract}
We find the Taylor Series for a function.
\end{abstract}

\maketitle

  
\section{Taylor Series}

In this section, we will find a power series expansion centered at $x = a$ for a given infinitely differentiable function, $f(x)$.
Such a series is called a Taylor Series.  In the case that $a = 0$, we call the series a Maclaurin Series.

In other words, for a given function $f(x)$ and a given center, $x = a$, we wish to create a power series so that
\[
f(x) = \sum_{n=0}^\infty c_n (x-a)^n = c_0 + c_1(x-a) + c_2(x-a)^2 + \cdots,
\]
where the series converges in an interval of the form $(a-r, a+r)$ for some $r >0$. This is an interval centered at $x = a$ of radius $r$.
The key to creating the Taylor Series is to find the coefficients, $c_n$.
To find $c_0$, let $x = a$ in the equation above. We get:
\[
f(a) = \sum_{n=0}^\infty c_n (a-a)^n = c_0 + c_1(a-a) + c_2(a-a)^2 + \cdots = c_0.
\]
Next, to find $c_1$, we differentiate both sides of the equation above, and then let $x = a$.
Differentiating gives
\[
f'(x) = c_1 + 2c_2(x-a) + 3c_3(x-a)^2 + \cdots,
\]
and substituting in $x = a$, this simplifies to 
\[
f'(a) = c_1 + 2c_2(a-a) + 3c_3(a-a)^2 + \cdots = c_1.
\]

Next, to find $c_2$, we differentiate both sides of the equation above, and then let $x = a$.
Differentiating gives
\[
f''(x) = 2c_2 + 3\cdot 2 c_3(x-a) + 4\cdot 3 c_4(x-a)^2 + \cdots,
\]
and substituting in $x = a$, this simplifies to 
\[
f''(a) = 2c_2 + 3\cdot 2 c_3(a-a) + 4\cdot 3 c_4(a-a)^2 + \cdots = 2c_2,
\]
so that $c_2 = \frac{f''(a)}{2}$.

Continuing in this fashion, we can find $c_3$:
\[
f'''(x) = 3 \cdot 2 \cdot 1 c_3 + 4\cdot 3 \cdot 2 c_4 (x-a) + 5 \cdot 4 \cdot 3 c_5 (x-a)^2 + \cdots,
\]
and letting $x = a$ gives
\[
f'''(a) = 3 \cdot 2 \cdot 1 c_3 + 4\cdot 3 \cdot 2 c_4 (a-a) + 5 \cdot 4 \cdot 3 c_5 (a-a)^2 + \cdots = 6c_3,
\]
so that $c_3 = \frac{f'''(a)}{6}$.
The pattern continues, so that $c_4 = \frac{f^{(4)}(a)}{4\cdot 3 \cdot 2 \cdot 1} = \frac{f^{(4)}(a)}{24}$
and $c_5 = \frac{f^{(5)}(a)}{5\cdot 4 \cdot 3 \cdot 2 \cdot 1} = \frac{f^{(5)}(a)}{120}$.
In general, we have 
\[
c_n = \frac{f^{(n)}(a)}{n\cdot (n-1) \cdot (n-2) \cdot \dots \cdot 1} = \frac{f^{(n)}(a)}{n!}.
\]
Thus, the Taylor Series representation of $f(x)$ centered at $x = a$ is given by

\[
f(x) = \sum_{n=0}^\infty c_n (x-a)^n = \sum_{n=0}^\infty \frac{f^{(n)}(a)}{n!} (x-a)^n.
\]


We present this results in the following theorem.

\begin{theorem}[Taylor Series]
Suppose the function $f(x)$ has derivatives of all orders at $x = a$. Then the \textbf{Taylor Series} 
representation for $f(x)$ centered at $x = a$ is given by
\[
f(x) = \sum_{n=0}^\infty \frac{f^{(n)}(a)}{n!} (x-a)^n.
\]

 In the case that $a = 0$, the series has the form
\[
 f(x) = \sum_{n=0}^\infty \frac{f^{(n)}(0)}{n!} x^n,
\]
and is called the \textbf{Maclaurin Series} for $f(x)$.
\end{theorem}

\begin{example}[example 1] Find the first four terms of the Taylor Series $f(x) = \sqrt x$ centered at $x = 4$.\\
Since we are asked to find the first four terms, we must find the coefficients $c _0, c_1, c_2$ and $c_3$
and the answer will have the form 
\[
\sqrt x = c_0 + c_1(x-4) + c_2(x-4)^2 + c_3(x-4)^3 + \cdots .
\]
To find the coefficients, we create the following table:

\[
\begin{array}{|c|c|c|c|} 
\hline
\bf{n} & \bf{f^{(n)}(x)} & \bf{f^{(n)}(a), \; a = 4} & \bf{c_n} \\[1em] 
\hline
 0 & x^{1/2} & 4^{1/2} = 2 & 2 \\[1em]
\hline
1 & \frac12 x^{-1/2} & \frac12 \cdot 4^{-1/2} = \frac14 & \frac14 \\[1em]
\hline
 2 & -\frac14 x^{-3/2} & -\frac14 \cdot 4^{-3/2} 
= -\frac14 \cdot \frac18 = -\frac{1}{32} & -\frac{1}{64} \\[1em]
\hline
 3 & \frac38 x^{-5/2} & \frac38 \cdot 4^{-5/2} = \frac38 \cdot \frac{1}{32} = \frac{3}{256} & \frac{1}{512}\\[1em]
\hline
\end{array}
\]



We can now use the coefficients in the right-hand column of the table to write the final answer. 
The first four terms of the Taylor Series for the function $f(x) = \sqrt x$ centered at $x = 4$ are
\begin{align*}
\sqrt x &= c_0 + c_1(x-4) + c_2(x-4)^2 + c_3(x-4)^3 + \cdots \\
        &= 2 + \frac14(x-4) -\frac{1}{64}(x-4)^2 + \frac{1}{512}(x-4)^3 + \cdots
\end{align*}

\end{example}



\begin{problem}(problem 1) Find the first four terms of the Taylor Series $f(x) = \sqrt x$ centered at $x = 1$.\\

The final answer has the form:
\begin{center}
\begin{multipleChoice}
\choice{a) \;\;\; $\sqrt x = c_0 + c_1(x-1) + c_2(x-1) + c_3(x-1) + \cdots$ }
\choice{b) \;\;\; $\sqrt x = c_0 + c_1(x- \sqrt 1) + c_2(x-\sqrt 2) + c_3(x-\sqrt 3) + \cdots$ }
\choice{c) \;\;\; $\sqrt x = c_0 + c_1(\sqrt x-1) + c_2(\sqrt x -1)^2 + c_3(\sqrt x-1)^3 + \cdots$ }
\choice[correct]{d) \;\;\; $\sqrt x = c_0 + c_1(x-1) + c_2(x-1)^2 + c_3(x-1)^3 + \cdots$ }
\end{multipleChoice}
\end{center}

Fill in the following table to find the coefficients:

\[
\begin{array}{|c|c|c|c|} 
\hline
\bf{n} & \bf{f^{(n)}(x)} & \bf{f^{(n)}(a),\; a = 1} & \bf{c_n} \\[1em] 
\hline
 0 & f(x) = x^{1/2} & f(1) = 1 & c_0 = \answer{1} \\[1em]
\hline
1 & f'(x) = \answer{\frac12 x^{-1/2}} & f'(1) = \answer{1/2} & c_1 = \answer{\frac12} \\[1em]
\hline
 2 & f''(x) =\answer{-\frac14 x^{-3/2}} & f''(1) = \answer{-1/4} & c_2 = \answer{-\frac{1}{8}} \\[1em]
\hline
 3 & f'''(x) =\answer{\frac38 x^{-5/2}} & f'''(1) = \answer{\frac38 } & c_3 = \answer{\frac{1}{16}}\\[1em]
\hline
\end{array}
\]


The first four terms of the Taylor Series for the function $f(x) = \sqrt x$ centered at $x = 1$ are
\[
\sqrt x = \answer{1 + \frac12(x-1) -\frac{1}{8}(x-1)^2 + \frac{1}{16}(x-1)^3} + \cdots
\]


\end{problem}


In the last example and problem, we computed only the first four terms of the Taylor Series, yielding a polynomial of degree 3.
This is a special polynomial.

\begin{definition}[Taylor Polynomial]
Give a function $f(x)$ and its first $n$ derivatives at $x = a$, $f^{(k)}(a), k= 0, 1, 2, \ldots, n$, the polynomial
\[
T_n (x) = \sum_{k=0}^n\frac{f^{(k)}(a)}{k!} (x-a)^k.
\]
is called the Taylor Polynomial of degree $n$ for $f(x)$ centered at $x=a$.
\end{definition}

\begin{remark}
The Taylor Polynomial of degree 1 for $f(x)$ centered at $x = a$,
\[
T_1(x) = f(a) + f'(a)(x-a)
\]
is also known as the Linearization of $f(x)$ at $x = a$ which is used in making linear approximations.
\end{remark}


\begin{example}[example 2] Find the Taylor Polynomial of degree 3, $T_3(x)$, for $f(x) = \sqrt[3] x$ centered at $x = -1$.\\
Since we are asked to find $T_3(x)$, we must find the coefficients $c _0, c_1, c_2$ and $c_3$
and the answer will have the form 
\[
T_3(x) = c_0 + c_1(x+1) + c_2(x+1)^2 + c_3(x+1)^3.
\]
To find the coefficients, we create the following table:

\[
\begin{array}{|c|c|c|c|} 
\hline
\bf{n} & \bf{f^{(n)}(x)} & \bf{f^{(n)}(a), \; a = -1} & \bf{c_n} \\[1em] 
\hline
 0 & x^{1/3} & (-1)^{1/3} = -1 & -1 \\[1em]
\hline
1 & \frac13 x^{-2/3} & \frac13 \cdot (-1)^{-2/3} = \frac13 & \frac13 \\[1em]
\hline
 2 & -\frac29 x^{-5/3} & -\frac29 \cdot (-1)^{-5/3} 
= -\frac29 \cdot (-1) = \frac29 & \frac{1}{9} \\[1em]
\hline
 3 & \frac{10}{27} x^{-8/3} & \frac{10}{27} \cdot (-1)^{-8/3} = \frac{10}{27} \cdot (1) = \frac{10}{27} & \frac{5}{81}\\[1em]
\hline
\end{array}
\]



We can now use the coefficients in the right-hand column of the table to write the final answer. 
The Taylor Polynomial of degree 3 for $f(x) = \sqrt[3] x$ centered at $x = -1$ is
\begin{align*}
T_3(x) &= c_0 + c_1(x+1) + c_2(x+1)^2 + c_3(x+1)^3  \\
        &= -1 + \frac13(x+1) + \frac{1}{9}(x+1)^2 + \frac{5}{81}(x+1)^3 
\end{align*}

\end{example}




\begin{problem}(problem 2a) Find the Taylor Polynomial of degree 3, $T_3(x)$, for $f(x) = \sqrt[3] x$ centered at $x = 8$.\\

The final answer has the form:
\begin{center}
\begin{multipleChoice}
\choice{a) \;\;\; $\sqrt[3] x = c_0 + c_1(x-8) + c_2(x-8) + c_3(x-8) $ }
\choice{b) \;\;\; $\sqrt[3] x = c_0 + c_1(x- \sqrt[3] 1) + c_2(x-\sqrt[3] 2) + c_3(x-\sqrt[3] 3) $ }
\choice[correct]{c) \;\;\; $\sqrt[3] x = c_0 + c_1(x-8) + c_2(x-8)^2 + c_3(x-8)^3 $ }
\choice{d) \;\;\; $\sqrt[3] x = c_0 + c_1(\sqrt[3]x-8) + c_2(\sqrt[3] x -8)^2 + c_3(\sqrt[3] x-8)^3 $ }
\end{multipleChoice}
\end{center}

Fill in the following table to find the coefficients:

\[
\begin{array}{|c|c|c|c|} 
\hline
\bf{n} & \bf{f^{(n)}(x)} & \bf{f^{(n)}(a), a = 8} & \bf{c_n} \\[1em] 
\hline
 0 & f(x) = x^{1/3} & f(8) = 2 & c_0 = \answer{2} \\[1em]
\hline
1 & f'(x) = \answer{\frac13 x^{-2/3}} & f'(8) = \answer{1/12} & c_1 = \answer{1/12} \\[1em]
\hline
 2 & f''(x) =\answer{-\frac29 x^{-5/3}} & f''(8) = \answer{-1/144} & c_2 = \answer{-\frac{1}{288}} \\[1em]
\hline
 3 & f'''(x) =\answer{\frac{10}{27} x^{-8/3}} & f'''(8) = \answer{5/3456 } & c_3 = \answer{\frac{5}{20736}}\\[1em]
\hline
\end{array}
\]


The first four terms of the Taylor Series for the function $f(x) = \sqrt[3] x$ centered at $x = 8$ are
\[
T_3(x) = \answer{2 + \frac{1}{12}(x-8) -\frac{1}{288}(x-8)^2 + \frac{5}{20736}(x-8)^3}
\]


\end{problem}





\begin{problem}(problem 2b) Find the Taylor Polynomial of degree 3, $T_3(x)$, for
 $f(x) = x\sqrt x$ centered at $x = 4$.\\

The function $f(x) = x\sqrt x$ can be written as a power function, $x^k$, for an appropriate value of $k$.
Write $x\sqrt x$ as a power function:
\begin{hint}
$x\sqrt x = x*x^{1/2}$; add exponents
\end{hint}
\[
x\sqrt x = \answer{x^{3/2}}
\]


The final answer has the form:
\begin{center}
\begin{multipleChoice}
\choice{a) \;\;\; $x\sqrt x = c_0 + c_1(x-4) + c_2(x-4) + c_3(x-4)$ }
\choice{b) \;\;\; $x\sqrt x = c_0 + c_1(x- 1\sqrt1) + c_2(x-2\sqrt2) + c_3(x-3\sqrt3)$ }
\choice{c) \;\;\; $x\sqrt x = c_0 + c_1(x\sqrt x -4) + c_2(x\sqrt x -4)^2 + c_3(x\sqrt x-4)^3$ }
\choice[correct]{d) \;\;\; $x\sqrt x = c_0 + c_1(x-4) + c_2(x-4)^2 + c_3(x-4)^3$ }
\end{multipleChoice}
\end{center}

Fill in the following table to find the coefficients:

\[
\begin{array}{|c|c|c|c|} 
\hline
\bf{n} & \bf{f^{(n)}(x)} & \bf{f^{(n)}(a), a = 4} & \bf{c_n} \\[1em] 
\hline
 0 & f(x) = x^{3/2} & f(4) = 8 & c_0 = \answer{8} \\[1em]
\hline
1 & f'(x) = \answer{\frac32 x^{1/2}} & f'(4) = \answer{3} & c_1 = \answer{3} \\[1em]
\hline
 2 & f''(x) =\answer{\frac34 x^{-1/2}} & f''(4) = \answer{3/8} & c_2 = \answer{3/16} \\[1em]
\hline
 3 & f'''(x) =\answer{-\frac38 x^{-3/2}} & f'''(4) = \answer{-3/64} & c_3 = \answer{-\frac{1}{128}}\\[1em]
\hline
\end{array}
\]


The first four terms of the Taylor Series for the function $f(x) = x\sqrt x$ centered at $x = 4$ are
\[
T_3(x) = \answer{8 + 3(x-4) +\frac{3}{16}(x-4)^2 - \frac{1}{128}(x-4)^3} + \cdots
\]


\end{problem}





\begin{example}[example 3] Find the Taylor Polynomial of degree 4, $T_4(x)$, for $f(x) = \ln(x)$ centered at $x = 1$.\\
Since we are asked to find the forth degree Taylor Polynomial, we must find the coefficients $c _0, c_1, c_2, c_3$ and $c_4$
and the answer will have the form 
\[
\ln(x) = c_0 + c_1(x-1) + c_2(x-1)^2 + c_3(x-1)^3 + c_4(x-1)^4.
\]
To find the coefficients, we create the following table:

\[
\begin{array}{|c|c|c|c|} 
\hline
\bf{n} & \bf{f^{(n)}(x)} & \bf{f^{(n)}(a), \; a = 1} & \bf{c_n} \\[1em] 
\hline
 0 & \ln(x) & \ln(1) = 0 & 0 \\[1em]
\hline
1 & \frac{1}{x} & 1 & 1 \\[1em]
\hline
 2 & -\frac{1}{x^2} & -1  & -1/2 \\[1em]
\hline
 3 & \frac{2}{x^3} & 2 & \frac13\\[1em]
\hline
 4 & -\frac{6}{x^4} & -6 & -\frac14\\[1em]
\hline
\end{array}
\]



We can now use the coefficients in the right-hand column of the table to write the final answer. 
The first five terms of the Taylor Series for the function $f(x) = \ln(x)$ centered at $x = 1$ are
\begin{align*}
T_4(x) &= c_0 + c_1(x-1) + c_2(x-1)^2 + c_3(x-1)^3 + c_4(x-1)^4\\
        &= 0 + 1(x-1) -\frac{1}{2}(x-1)^2 + \frac{1}{3}(x-1)^3-\frac{1}{4}(x-1)^4\\
        &= (x-1) -\frac{1}{2}(x-1)^2 + \frac{1}{3}(x-1)^3-\frac{1}{4}(x-1)^4
\end{align*}

\end{example}




\begin{problem}(problem 3) Find the Taylor Polynomial of degree 4, $T_4(x)$, for $f(x) = \ln(2x)$ centered at $x = 1$.\\


The final answer has the form:
\begin{center}
\begin{multipleChoice}
\choice{a) \;\;\; $\ln(2x) = c_0 + c_1(x-1) + c_2(x-1) + c_3(x-1) + c_4(x-1)$ }
\choice[correct]{b) \;\;\; $\ln(2x) = c_0 + c_1(x-1) + c_2(x-1)^2 + c_3(x-1)^3 + c_4(x-1)^4$ }
\choice{c) \;\;\; $\ln(2x) = c_0 + c_1(\ln(2x) -1) + c_2(\ln(2x) -1)^2 + c_3(\ln(2x)-1)^3+ c_4(\ln(2x)-1)^4$ }
\choice{d) \;\;\;  $\ln(2x) = c_0 + c_1(x- \ln(1)) + c_2(x-\ln(2)) + c_3(x-\ln(3))+ c_4(x-\ln(4))$}
\end{multipleChoice}
\end{center}

Fill in the following table to find the coefficients:

\[
\begin{array}{|c|c|c|c|} 
\hline
\bf{n} & \bf{f^{(n)}(x)} & \bf{f^{(n)}(a), a = 1} & \bf{c_n} \\[1em] 
\hline
 0 & f(x) = \ln(2x) & f(1) = \ln(2) & c_0 = \answer{\ln(2)} \\[1em]
\hline
1 & f'(x) = \answer{\frac{1}{x}} & f'(1) = \answer{1} & c_1 = \answer{1} \\[1em]
\hline
 2 & f''(x) =\answer{-\frac{1}{x^2}} & f''(1) = \answer{-1} & c_2 = \answer{-1/2} \\[1em]
\hline
 3 & f'''(x) =\answer{\frac{2}{x^3}} & f'''(1) = \answer{2} & c_3 = \answer{1/3}\\[1em]
\hline
 4 & f^{(4)}(x) =\answer{-\frac{6}{x^4}} & f^{(4)}(1) = \answer{-6} & c_4 = \answer{-1/4}\\[1em]
\hline
\end{array}
\]


The first five terms of the Taylor Series for the function $f(x) = \ln(2x)$ centered at $x = 1$ are
\[
T_4(x) = \answer{\ln(2) + (x-1) -\frac12(x-1)^2 + \frac13(x-1)^3-\frac14(x-1)^4}
\]


\end{problem}

Taylor Polynomials can be used to approximate function values, and the following theorem gives us an expression for the error in such an approximation.

\begin{theorem}[Taylor's Remainder Theorem]
If the function $f(x)$ is $n+1$ times differentiable at $x = a$ then the difference between $f(x)$ and $T_n(x)$
is given by 
\[
f(x) - T_n(x) = \frac{f^{(n+1)}(c)}{(n+1)!}(x-a)^n
\]
where $c$ is number between $a$ and $x$.
\end{theorem}

\section{Video Lessons}

\begin{center}
\begin{foldable}
\unfoldable{Here is a detailed, lecture style video on Taylor Series:}
\youtube{YMTCxncDa4k}
\end{foldable}
\end{center}



\begin{center}
\begin{foldable}
\unfoldable{Here is a detailed, lecture style video on Maclaurin Series:}
\youtube{aa9rcfNJrfk}
\end{foldable}
\end{center}







\end{document}





\begin{problem}
Compute 
\[
\int xe^{x^2} \; dx
\]

\begin{question}
Step 1: What method should we use?
\begin{multipleChoice}
\choice[correct]{u-sub}
\choice{integration by parts}
\choice{common denominator}
\end{multipleChoice}

\begin{question}
Step 2: What should $u$ equal?
\begin{multipleChoice}
\choice[correct]{$x^2$}
\choice{$e^{x^2}$}
\choice{banana}
\end{multipleChoice}

\begin{question}
The new integral is $\int \answer{1/2 e^u} \; du$

\begin{question}
The final answer is $\answer{1/2 e^{x^2}}$.

\end{question}
\end{question}
\end{question}
\end{question}

\end{problem}






\begin{table}[ht]
\caption{Finding the Coefficients, $c_n$}
\centering
\begin{tabular}{|c|c|c|c|}
\hline
\raisebox{7pt}{\phantom{i}}\textbf{$n$} & \textbf{$f^{(n)}(x)$} & \textbf{$f^{(n)}(a), a = 4$} & \textbf{$c_n$} \\
\hline
\raisebox{7pt}{\phantom{i}}$0$ & $x^{1/2}$ &\raisebox{8pt}{\phantom{M}} $4^{1/2} = 2$ & $2$ \\
\hline
\raisebox{7pt}{\phantom{i}}$1$ & $\frac12 x^{-1/2}$ & \raisebox{8pt}{\phantom{M}}$\displaystyle{\frac12 \cdot 4^{-1/2} = \frac14}$ & $\frac14$ \\
\hline
\raisebox{7pt}{\phantom{i}} $2$ & \raisebox{12pt}{\phantom{i}}$-\frac14 x^{-3/2}$ & $-\frac14 \cdot 4^{-3/2} 
= -\frac14 \cdot \frac18 = -\frac{1}{32}$ & $-\frac{1}{64}$ \\
\hline
\raisebox{7pt}{\phantom{i}} $3$ & $\frac38 x^{-5/2}$ & $\frac38 \cdot 4^{-5/2} = \frac38 \cdot \frac{1}{32} = -\frac{3}{256}$ & $-\frac{1}{512}$ \\
\hline
\end{tabular}
\end{table}




\begin{array}{|c|c|c|c|}  
\hline
\textbf{$n$} & \textbf{$f^{(n)}(x)$} & \textbf{$f^{(n)}(a), a = 4$} & \textbf{$c_n$} \\
\hline
$0$ & $x^{1/2}$ & $4^{1/2} = 2$ & $2$ \\
\hline
$1$ & $\frac12 x^{-1/2}$ & $\frac12 \cdot 4^{-1/2} = \frac14$ & $\frac14$ \\
\hline
 $2$ & $-\frac14 x^{-3/2}$ & $-\frac14 \cdot 4^{-3/2} 
= -\frac14 \cdot \frac18 = -\frac{1}{32}$ & $-\frac{1}{64}$ \\
\hline
 $3$ & $\frac38 x^{-5/2}$ & $\frac38 \cdot 4^{-5/2} = \frac38 \cdot \frac{1}{32} = -\frac{3}{256}$ & $-\frac{1}{512}$
\hline
\end{array}





\begin{example} %example #15
Find $h'(x)$ if $h(x) = x^{\sin(x)}$.\\
We will use the fact that the exponential and logarithm functions are inverses,
\[e^{\ln(x)} = x,\]
and the exponent property of logarithms, 
\[\ln(x^n) = n\ln(x),\]
to rewrite $h(x)$.  We have 
\[h(x) = x^{\sin(x)} = e^{\ln(x^{\sin(x)})} = e^{\sin(x)\ln(x)}\]
and we can now compute $h'(x)$ using a combination of the chain rule and product rule.
We can write $h(x)$ as a composition, $f(g(x))$ with 
\[g(x) = \sin(x)\ln(x) \quad \text{and} \quad f(x) = e^x.\]
Then to find $g'(x)$ we us the product rule and we get $g'(x) = \frac{\sin(x)}{x} + \cos(x)\ln(x)$.
Next $f'(x) = e^x$ and 
hence $f'(g(x)) = e^{g(x)} = e^{\sin(x)\ln(x)} = x^{\sin(x)}$.
We can then conclude $h'(x) = f'(g(x))g'(x) = x^{\sin(x)} \left[ \frac{\sin(x)}{x} + \cos(x)\ln(x)\right]$.
\end{example}

%more question formats below













%\begin{verbatim}
\begin{question}
What is your favorite color?
\begin{multipleChoice}
\choice[correct]{Rainbow}
\choice{Blue}
\choice{Green}
\choice{Red}
\end{multipleChoice}
\begin{freeResponse}
Hello
\end{freeResponse}
\end{question}
%\end{verbatim}





\begin{question}
  Which one will you choose?
  \begin{multipleChoice}
    \choice[correct]{I'm correct.}
    \choice{I'm wrong.}
    \choice{I'm wrong too.}
  \end{multipleChoice}
\end{question}


\begin{question}
  Which one will you choose?
  \begin{selectAll}
    \choice[correct]{I'm correct.}
    \choice{I'm wrong.}
    \choice[correct]{I'm also correct.}
    \choice{I'm wrong too.}
  \end{selectAll}
\end{question}


\begin{freeResponse}
What is the chain rule used for?
\end{freeResponse}
