\documentclass{ximera}

\input{../preamble}

\outcome{Find the interval of convergence of a power series}

\title{3.10 Power Series: Interval of Convergence}

\begin{document}

\begin{abstract}
We find the interval of convergence of a power series.
\end{abstract}

\maketitle

\section{Interval of Convergence}

\section{Power Series}

We will find the interval of convergence of a power series.

\begin{definition}[Power Series]
A \textbf{power series} with center at $x = a$ is an infinite series of the form
\[
\sum_{n=0}^\infty c_n(x-a)^n.
\]
\end{definition}

Some examples of power series are:
\[ 
\sum_{n=0}^\infty x^n, \; \sum_{n=0}^\infty \frac{x^n}{n!}, \;\text{and} \sum_{n=0}^\infty \frac{n^2(x+ 2)^n}{2^n}.
\]
The first two have center at $x = 0$ and the third is centered at $x = -2$. 
The question we ask when confronted with a power series is, ``for which values of $x$ does the series converge?"
The theory tells us that the power series will converge in an interval centered at the center of the power series.
To find this \textbf{interval of convergence}, we frequently use the ratio test.

\begin{example}[example 1]
Find the interval of convergence of the power series $\displaystyle{\sum_{n=0}^\infty x^n}$.\\
Noting that this series happens to be a geometric series (with common ratio $x$), we can use the fact that this series will converge 
if and only in $|x| < 1$.  This is equivalent to the interval $(-1, 1)$ and this is the interval of convergence of the power series.
In other words, for any value of $x$ in this interval, 
the resulting series will converge and for any value of $x$ outside of this interval, 
the series will diverge. Notice that the interval of convergence is centered around $x = 0$, which is the center of the power series.
\end{example}

\begin{problem}(problem 1)
Find the interval of convergence of the power series
\[
\sum_{n=0}^\infty \frac{x^n}{2^n}
\]
The interval of convergence is
\begin{multipleChoice}
\choice{$(-1/2, 1/2)$}
\choice{$(-1, 1)$}
\choice[correct]{$(-2, 2)$}
\choice{$(-\infty, \infty)$}
\end{multipleChoice}
\end{problem}


\begin{example}[example 2]
Find the interval of convergence of the power series $\displaystyle{\sum_{n=1}^\infty \frac{x^n}{n^2}}$.\\
We will use the ratio test:
\[
L = \lim_{n \to \infty} \left|\frac{x^{n+1}}{(n+1)^2} \cdot \frac{n^2}{x^n} \right| = \lim_{n \to \infty} \frac{n^2}{(n+1)^2}\cdot \left|  \frac{x^{n+1}}{x^n} \right| 
\]
\[
= \lim_{n \to \infty} \frac{n^2}{(n+1)^2}\cdot \left|  x \right| = |x|.
\]
By the rules for the ratio test, the series converges when $|x| < 1$ and diverges when $|x| > 1$.
Unfortunately, the ratio test gives no conclusion when $|x| = 1$, which corresponds to $x = \pm 1$.
To determine the behavior of the series at these values, we plug them into the power series.
If $x = 1$, the power series becomes
\[
\sum_{n=1}^\infty \frac{x^n}{n^2} = \sum_{n=1}^\infty \frac{1}{n^2},
\]
which is a $p$-series with $p = 2$. Since $p >1$, this series converges and therefore our power series converges when $x = 1$.
Next, if $x = -1$, the power series becomes:
\[
\sum_{n=1}^\infty \frac{x^n}{n^2} = \sum_{n=1}^\infty \frac{(-1)^n}{n^2},
\]
which is an alternating $p$-series and so it converges. Therefore our power series converges when $x = -1$.
The interval of convergence of the power series is thus $[-1, 1]$, and we again note that this is an interval centered about the 
center of the power series, $x = 0$.
\end{example}


\begin{problem}(problem 2)
Find the interval of convergence of the power series
\[
\sum_{n=1}^\infty \frac{x^n}{n}
\]
The interval of convergence is
\begin{multipleChoice}
\choice{$(-1, 1)$}
\choice[correct]{$[-1, 1)$}
\choice{$(-1, 1]$}
\choice{$[-1, 1]$}
\end{multipleChoice}
\end{problem}


\begin{example}[example 3]
Find the interval of convergence of the power series $\displaystyle{\sum_{n=1}^\infty \frac{x^n}{n!}}$.\\
We will use the ratio test:
\[
L = \lim_{n \to \infty} \left|\frac{x^{n+1}}{(n+1)!} \cdot \frac{n!}{x^n} \right| = \lim_{n \to \infty} \frac{n!}{(n+1)!}\cdot \left|  \frac{x^{n+1}}{x^n} \right| 
\]
\[
= \lim_{n \to \infty} \frac{1}{n+1}\cdot |x| = 0.
\]
By the rules for the ratio test, the series converges regardless of the value of $x$.
Hence the interval of convergence is $(-\infty, \infty)$.
\end{example}




\begin{problem}(problem 3)
Find the interval of convergence of the power series
\[
\sum_{n=0}^\infty \frac{(n+2)}{n!}x^n
\]
The interval of convergence is
\begin{multipleChoice}
\choice{$0$}
\choice{$(-1, 1)$}
\choice{$[-1, 1]$}
\choice[correct]{$(-\infty, \infty)$}
\end{multipleChoice}
\end{problem}


\begin{example}[example 4]
Find the interval of convergence of the power series $\displaystyle{\sum_{n=1}^\infty \frac{(x-3)^n}{n}}$.\\
We will use the ratio test:
\[
L = \lim_{n \to \infty} \left|\frac{(x-3)^{n+1}}{n+1} \cdot \frac{n}{(x-3)^n} \right| = \lim_{n \to \infty} \frac{n}{n+1} \cdot \left|  \frac{(x-3)^{n+1}}{(x-3)^n} \right| 
\]
\[
= \lim_{n \to \infty} \frac{n}{n+1}\cdot |x-3| = |x-3|.
\]
By the rules for the ratio test, the series converges when $|x-3| < 1$ and diverges when $|x-3| > 1$.
Unfortunately, the ratio test gives no conclusion when $|x-3| = 1$, which corresponds to $x = 2$ and $x = 4$.
To determine the behavior of the series at these values, we plug them into the power series.
If $x = 4$, the power series becomes
\[
\sum_{n=1}^\infty \frac{(x-3)^n}{n} = \sum_{n=1}^\infty \frac{1}{n},
\]
which is the divergent harmonic series.
Next, if $x = 2$, the power series becomes:
\[
\sum_{n=1}^\infty \frac{(x-3)^n}{n} = \sum_{n=1}^\infty \frac{(-1)^n}{n},
\]
which is the convergent alternating harmonic series.
The interval of convergence of the power series is thus $[2, 4)$, and we again note that this is an interval centered about the 
center of the power series, $x = 3$.
\end{example}



\begin{problem}(problem 4)
Find the interval of convergence of the power series
\[
\sum_{n=1}^\infty \frac{(x+2)^n}{n^2}
\]
The interval of convergence is
\begin{multipleChoice}
\choice{$(-3, -1)$}
\choice{$[-3, -1)$}
\choice{$(-3, -1]$}
\choice[correct]{$[-3, -1]$}
\end{multipleChoice}
\end{problem}

\begin{example}[example 5]
Find the interval of convergence of the power series $\displaystyle{\sum_{n=1}^\infty \frac{(x+2)^n}{(2n+1)3^n}}$.\\
We will use the ratio test:
\[
L = \lim_{n \to \infty} \left|\frac{(x+2)^{n+1}}{(2n+3)3^{n+1}} \cdot \frac{(2n+1) 3^n}{(x+2)^n} \right| = 
\lim_{n \to \infty} \frac{2n+1}{2n+3} \cdot \frac{3^n}{3^{n+1}} \cdot \left|  \frac{(x+2)^{n+1}}{(x+2)^n} \right| 
\]
\[
= \lim_{n \to \infty} \frac{2n+1}{2n+3} \cdot \frac13 \cdot \left|  x+2 \right| = \frac{|x+2|}{3}.
\]
By the rules for the ratio test, the series converges when $\dfrac{|x+2|}{3} < 1$ and diverges when $\dfrac{|x+2|}{3} > 1$.
Unfortunately, the ratio test gives no conclusion when $\dfrac{|x+2|}{3} = 1$, which corresponds to $x = -5$ and $x = 1$.
To determine the behavior of the series at these values, we plug them into the power series.
If $x = 1$, the power series becomes
\[
\sum_{n=1}^\infty \frac{(x+2)^n}{(2n+1)3^n} = \sum_{n=1}^\infty \frac{3^n}{(2n+1)3^n} = \sum_{n=1}^\infty \frac{1}{2n+1}
\]
which diverges by the limit comparison test with the harmonic series.
Next, if $x = -5$, the power series becomes:
\[
\sum_{n=1}^\infty \frac{(x+2)^n}{(2n+1)3^n} = \sum_{n=1}^\infty \frac{(-3)^n}{(2n+1)3^n} = \sum_{n=1}^\infty \frac{(-1)^n}{2n+1}
\]
which converges by the alternating series test.
The interval of convergence of the power series is thus $[-5, 1)$, and we again note that this is an interval centered about the 
center of the power series, $x = -2$.
\end{example}




\begin{problem}(problem 5)
Find the interval of convergence of the power series
\[
\sum_{n=1}^\infty \frac{(x-4)^n}{n2^n}
\]
The interval of convergence is
\begin{multipleChoice}
\choice{$(2, 6)$}
\choice{$[2, 6)$}
\choice{$(2, 6]$}
\choice[correct]{$[2, 6]$}
\end{multipleChoice}
\end{problem}



\begin{center}
\begin{foldable}
\unfoldable{Here is a detailed, lecture style video on the interval of convergence of a power series:}
\youtube{DdrevgO7_eY}
\end{foldable}
\end{center}

\begin{center}
\begin{foldable}
Here is a detailed, lecture style video on the interval of convergence of a power series:
\youtube{DdrevgO7_eY}
\end{foldable}
\end{center}





\end{document}


\begin{example} %example #15
Find $h'(x)$ if $h(x) = x^{\sin(x)}$.\\
We will use the fact that the exponential and logarithm functions are inverses,
\[e^{\ln(x)} = x,\]
and the exponent property of logarithms, 
\[\ln(x^n) = n\ln(x),\]
to rewrite $h(x)$.  We have 
\[h(x) = x^{\sin(x)} = e^{\ln(x^{\sin(x)})} = e^{\sin(x)\ln(x)}\]
and we can now compute $h'(x)$ using a combination of the chain rule and product rule.
We can write $h(x)$ as a composition, $f(g(x))$ with 
\[g(x) = \sin(x)\ln(x) \quad \text{and} \quad f(x) = e^x.\]
Then to find $g'(x)$ we us the product rule and we get $g'(x) = \frac{\sin(x)}{x} + \cos(x)\ln(x)$.
Next $f'(x) = e^x$ and 
hence $f'(g(x)) = e^{g(x)} = e^{\sin(x)\ln(x)} = x^{\sin(x)}$.
We can then conclude $h'(x) = f'(g(x))g'(x) = x^{\sin(x)} \left[ \frac{\sin(x)}{x} + \cos(x)\ln(x)\right]$.
\end{example}

%more question formats below













%\begin{verbatim}
\begin{question}
What is your favorite color?
\begin{multipleChoice}
\choice[correct]{Rainbow}
\choice{Blue}
\choice{Green}
\choice{Red}
\end{multipleChoice}
\begin{freeResponse}
Hello
\end{freeResponse}
\end{question}
%\end{verbatim}





\begin{question}
  Which one will you choose?
  \begin{multipleChoice}
    \choice[correct]{I'm correct.}
    \choice{I'm wrong.}
    \choice{I'm wrong too.}
  \end{multipleChoice}
\end{question}


\begin{question}
  Which one will you choose?
  \begin{selectAll}
    \choice[correct]{I'm correct.}
    \choice{I'm wrong.}
    \choice[correct]{I'm also correct.}
    \choice{I'm wrong too.}
  \end{selectAll}
\end{question}


\begin{freeResponse}
What is the chain rule used for?
\end{freeResponse}
