\documentclass[handout]{ximera}

\input{../preamble}

\pgfplotsset{compat=1.13}

\outcome{Learn the arithmetic of complex numbers}

\title{1.7 Hyperbolic Functions}

\begin{document}

\begin{abstract}
We learn the basic properties of the hyperbolic functions.
\end{abstract}

\maketitle

The hyperbolc sine and hyperbolic cosine functions are defined as
\[
\sinh x = \frac{e^x - e^{-x}}{2} \;\; \mbox{and} \;\; \cosh x = \frac{e^x + e^{-x}}{2}
\]

\begin{image}
\begin{tikzpicture}
\draw[<->, thick] (-3,0)--(3,0);

\draw[<->, thick] (0, 3)--(0,-3) node[ below=10pt, blue]{\large The Hyperbolic Sine, $y =\sinh x$};


\draw[ thick, domain=-1.7:1.7,smooth,variable=\x,blue] plot ({\x},{0.5*e^\x -0.5* e^-\x});


\draw[thin] (1,.2)--(1,-.2) node[below]{$1$};
\draw[thin] (-1,.2)--(-1,-.2) node[below]{$-1$};
\draw[thin] (2,.2)--(2,-.2) node[below]{$2$};
\draw[thin] (-2,.2)--(-2,-.2) node[below]{$-2$};

\draw[thin] (.2,1)--(-.2,1) node[left]{$1$};
\draw[thin] (.2,-1)--(-.2,-1) node[left]{$-1$};
\draw[thin] (.2,2)--(-.2,2) node[left]{$2$};
\draw[thin] (.2,-2)--(-.2,-2) node[left]{$-2$};


\end{tikzpicture}
\end{image}

\begin{image}
\begin{tikzpicture}
\draw[<->, thick] (-3,0)--(3,0);

\draw[<->, thick] (0, 3)--(0,-0.5) node[ below=10pt, blue]{The Hyperbolic Cosine, $y =\cosh x$};


\draw[ thick, domain=-1.7:1.7,smooth,variable=\x,blue] plot ({\x},{0.5*e^\x +0.5* e^-\x});


\draw[thin] (1,.2)--(1,-.2) node[below]{$1$};
\draw[thin] (-1,.2)--(-1,-.2) node[below]{$-1$};
\draw[thin] (2,.2)--(2,-.2) node[below]{$2$};
\draw[thin] (-2,.2)--(-2,-.2) node[below]{$-2$};

\draw[thin] (.2,1)--(-.2,1) node[left]{$1$};
\draw[thin] (.2,2)--(-.2,2) node[left]{$2$};



\end{tikzpicture}
\end{image}

\begin{example}[example 1]
Solve the equation $\cosh x = 6$ for $x$.\\
We use the definition of the hyperbolic cosine:
\[
\cosh x = \frac{e^x + e^{-x}}{2} = 6
\]
Ergo
\[
e^x +e^{-x} = 12
\]
Multiplying by $e^x$, we get
\[
e^{2x} - 12e^x +1 = 0 \;\; \mbox{or} \;\; u^2 - 12u + 1 = 0
\]
where $u = e^x$.  Now the quadratic formula gives
\[
u = \frac{12 \pm \sqrt{144 - 4}}{2} = 6 \pm \sqrt{35}
\]
Finally, we get the two solutions by taking the natural logarithm of $u$:
\[
x = \ln\left(6 \pm \sqrt{35}\right)
\]
These answers are negatives of one another (verify).
\end{example}

\begin{problem}[problem 1a]
Solve the following equation $\cosh x = 3$\\
The answers are (in increasing order):\\
$x = \answer{\ln(3-2\sqrt 2)}$ and $x = \answer{\ln(3+2\sqrt 2)}$
\end{problem}


\begin{problem}[problem 1b]
Solve the following equation $\sinh x = 3$\\
The answer is:\\
$x = \answer{\ln(3+\sqrt{10} 2)}$
\end{problem}

\begin{problem}(problem 1c) 
Find inverses for the hyperbolic sine and hyperbolic cosine functions.
\end{problem}

The hyperbolic sine function is an odd function:
\[
\sinh(-x) = -\sinh(x)
\]
and the hyperbolic cosine function is even:
\[
\cosh(-x) = -\cosh(x)
\]

The hyperbolic sine and cosine satisfy the fundamental identity
\[
\cosh^2 x - \sinh^2 x =1
\]
which means that the point $(\cosh t, \sinh t)$ lies on the (right branch of) the hyperbola
\[
x^2 -y^2 = 1
\]
This is why the functions are refered to as the hyperbolic functions.

The other four hyperbolic functions can be created from the hyperbolic sine and hyperbolic cosine functions:
\[
\tanh x = \frac{\sinh x}{\cosh x},\;\; \coth x = \frac{\cosh x}{\sinh x},
\]
\[
\sech x = \frac{1}{\cosh x}, \;\; \mbox{and}\;\; \csch x = \frac{1}{\sinh x}
\]

\begin{example}[example 2]
Find the derivative of the hyperbolic sine function.\\
The derivative of the hyperbolic sine function is given by
\[
\frac{d}{dx} \sinh(x) = \frac{d}{dx} \left( \frac{e^x -e^{-x}}{2} \right) = \frac{e^x + e^{-x}}{2} = \cosh x
\]
\end{example}

\begin{problem}(problem 2)
Find the derivatives of the other 5 hyperbolic functions.\\
$\frac{d}{dx} \cosh x = \answer{\sinh x}$\\
$\frac{d}{dx} \tanh x = \answer{\sech^2 x}$\\
$\frac{d}{dx} \sech x = \answer{-\sech x \tanh x}$\\
$\frac{d}{dx} \coth x = \answer{-\csch^2 x}$\\
$\frac{d}{dx} \csch x = \answer{-\csch x \coth x}$
\end{problem}


\begin{example}[example 3]
Find the Maclaurin series representation for the hyperbolic cosine.\\
Recall that the Maclaurin series for $e^x$ is given by
\[
e^x = \sum_{n=0}^\infty \frac{x^n}{n!}
\]
Thus
\[
\cosh x = \frac{e^x + e^{-x}}{2} = \frac12 \sum_{n=0}^\infty \frac{x^n}{n!} + \frac12 \sum_{n=0}^\infty \frac{(-x)^n}{n!}
\]
\[
= \sum_{\substack{n=0\\ n\; even}}^\infty \frac{x^n}{n!} = \sum_{n=0}^\infty \frac{x^{2n}}{(2n)!}
\]

\end{example}

\begin{problem}(problem 3)
Find the Maclauring series for the hyperbolic sine function.\\

\begin{multipleChoice}
\choice{$\sinh x=\displaystyle{\sum_{n=0}^\infty (-1)^n \frac{x^{2n+1}}{(2n+1)!}}$}
\choice{$\sinh x=\displaystyle{\sum_{n=0}^\infty  \frac{x^{2n+1}}{ n!}}$}
\choice[correct]{$\sinh x=\displaystyle{\sum_{n=0}^\infty  \frac{x^{2n+1}}{(2n+1)!}}$}
\end{multipleChoice}
\end{problem}


\end{document}

