\documentclass{ximera}
\usepackage{tcolorbox}
\input{../preamble}

\outcome{Compute an anti-derivative by reversing the chain rule.}

\title{0.3 Substitution}



\begin{document}

\begin{abstract}
In this section we learn to reverse the chain rule by making a substitution.
\end{abstract}

\maketitle

\section{$U$-Substitution}

We make a $u$-substitution to fill in the gaps in the following equation, which reverses the chain rule:

\[\int f(g(x))g'(x) \ dx = F(g(x)) + C. \]

If we let $ u = g(x)$ then $du = g'(x) \ dx$ and the integral can be rewritten as
\[\int f(g(x))g'(x) \ dx = \int f(u) \ du \]
which equals
\[F(u) + C,\]
and back-substituting gives
\[F(g(x)) + C. \]
Now we can see that
\[\int f(g(x))g'(x) \ dx = F(g(x)) + C. \]



\begin{example}[example 1]
Compute 
\[\int 2x\cos(x^2 + 1) \ dx.\]

Let $u = x^2 + 1$.  We have,
\[u = x^2 + 1\]
\[du = 2x \ dx\]

and the integral can be written as 
\[\int 2x\cos(x^2 + 1) \ dx = \int \cos(x^2 + 1) \ 2x\  dx = \int \cos(u) \ du.\]
The last integral can be computed as 
\[\int \cos(u) \ du = \sin(u) + C,\]
and by back-substituting, we have 
\[\sin(u) + C = \sin(x^2 + 1) + C.\]
Thus, using $u$-substitution we can conclude that
\[\int 2x\cos(x^2 + 1) \ dx =  \sin(x^2 + 1) + C.\]
\end{example}



\begin{problem}(problem 1)\\ Compute: $\displaystyle{\int 5x^4\sin(x^5 -7) \ dx}$.\\
Let $u = \answer{x^5 - 7}$. Then $du = \answer{5x^4 dx}$.\\
\begin{hint}
Don't forget the `dx' in your answer for `du'.
\end{hint}
Convert to an intergal in the variable $u$:
\[\int 5x^4\sin(x^5 -7) \ dx = \int\answer{\sin(u) du}\]
\begin{hint}
Don't forget the `du' in your integral.
\end{hint}
The final answer in terms of $x$ is:
\[\int 5x^4\sin(x^5 -7) \ dx = \answer{-\cos(x^5 -7)} +C.\]
\end{problem}


\begin{example}[example 2] Compute 
\[\int 2x(x^2 + 1)^4 \ dx.\]
Let $u = x^2 + 1$.  We have,
\[u = x^2 + 1\]
\[du = 2x \ dx\]

and the integral can be written as 
\[\int 2x(x^2 + 1)^4 \ dx = \int (x^2 + 1)^4 \ 2x \  dx = \int u^4 \ du.\]
The last integral can be computed as 
\[\int u^4 \ du = \tfrac{u^5}{5} + C,\]
and by back-substituting, we have 
\[\tfrac{u^5}{5} + C = \tfrac15(x^2 + 1)^5 + C .\]
Thus, using $u$-substitution we can conclude that
\[\int 2x(x^2 + 1)^4 \ dx  =  \tfrac15(x^2 + 1)^5 + C.\]
\end{example}

\begin{problem}(problem 2)\\
Compute $\displaystyle{\int 3x^2(x^3 + 2)^6 \ dx}$.\\
Let $u = \answer{x^3 + 2}$. Then $du = \answer{3x^2 dx}$.\\
\begin{hint}
Don't forget the `dx' in your answer for `du'.
\end{hint}
Convert to an intergal in the variable $u$:
\[\int 3x^2(x^3 + 2)^6 \ dx = \int\answer{u^6 du}\]
\begin{hint}
Don't forget the `du' in your integral.
\end{hint}
The final answer in terms of $x$ is:

\[\int 3x^2(x^3 + 2)^6 \ dx = \answer{(x^3 + 2)^7/7} +C.\]
\end{problem}



\begin{example}[example 3] Compute 
\[\int_0^2 2xe^{x^2 + 1} \ dx.\]
In this example, we have a definite integral.  When making a substitution in a definite integral, 
we must change the endpoints of integration in addition to the integrand and the differential.
As before, let $u = x^2 + 1$.  We have,
\[u = x^2 + 1\]
\[du = 2x \ dx\]
Now we prepare to change the endpoints. If $x = 0$, then $ u = 0^2 + 1 = 1$ and if $x = 2$, then $u = 2^2 +1 = 5$.
So, the endpoints in the original integral, 0 and 1, will be changed to 1 and 5 respectively.
\[\int_0^1 2xe^{x^2 + 1} \ dx  = \int_1^5  e^u \ du.\]
The last integral can be computed as 
\[\int_1^5 e^u \ du = e^u \Big{|}_1^5 = e^5 - e.\]

Thus, using $u$-substitution we can conclude that
\[\int_0^1 2xe^{x^2 + 1} \ dx =  e^5 - e.\]
\end{example}



\begin{problem}(problem 3)\\
Compute $\displaystyle{\int_1^2 -2xe^{-x^2} \ dx}$.\\
Let $u = \answer{-x^2}$. Then $du = \answer{-2x dx}$.\\
\begin{hint}
Don't forget the `dx' in your answer for `du'.
\end{hint}
If $x = 1$ then $u = \answer{-1}$ and \\
if $x = 2$ then $u = \answer{-4}$
Convert to an intergal in the variable $u$:
\[\int -2xe^{-x^2} \ dx = \int_{\answer{-1}}^{\answer{-4}} \answer{e^u du}\]
\begin{hint}
Don't forget the `du' in your integral.
\end{hint}
The final answer is:
\[\int_1^2 -2xe^{-x^2} \ dx = \answer{e^{-4} - e^{-1}} \]
\end{problem}

\begin{example}[example 4] Compute 
\[\int 2x\sqrt{x^2 + 1} \ dx.\]
Let $u = x^2 + 1$.  We have,
\[u = x^2 + 1\]
\[du = 2x \ dx\]

\[\int 2x\sqrt{x^2 + 1} \ dx = \int \sqrt{x^2 + 1} \cdot 2x\  dx = \int \sqrt{u} \ du.\]
The last integral can be computed as 
\[\int \sqrt u  \ du = \int u^{1/2} \ du = \tfrac{u^{3/2}}{3/2} + C = \tfrac23 u^{3/2} + C,\]
and by back-substituting, we have 
\[\tfrac23 u^{3/2}  + C = \frac23 (x^2 + 1)^{3/2} + C.\]
Thus, using $u$-substitution we can conclude that
\[\int 2x\sqrt{x^2 + 1} \ dx =  \tfrac23 (x^2 + 1)^{3/2} + C.\]
\end{example}

\begin{problem}(problem 4) Compute $\displaystyle{\int 4x^3 \sqrt{x^4 +2} \ dx}$.\\
Let $u = \answer{x^4 + 2}$. Then $du = \answer{4x^3 dx}$.\\
\begin{hint}
Don't forget the `dx' in your answer for `du'.
\end{hint}
Convert to an intergal in the variable $u$:
\[\int 4x^3 \sqrt{x^4 +2} \ dx = \int\answer{\sqrt u du}\]
\begin{hint}
Don't forget the `du' in your integral.
\end{hint}

\[\int 4x^3 \sqrt{x^4 +2} \ dx = \answer{2/3(x^4 +2)^{3/2}} +C.\]
\end{problem}



\begin{example}[example 5] Compute 
\[\int \frac{2x}{x^2 + 1} \ dx.\]
Let $u = x^2 + 1$.  We have,
\[u = x^2 + 1\]
\[du = 2x \ dx\]

\[\int \frac{2x}{x^2 + 1} \ dx = \int \frac{1}{x^2 + 1} \cdot 2x\  dx = \int \frac{1}{u} \ du.\]
The last integral can be computed as 
\[\int \frac{1}{u} \ du = \ln|u| + C,\]
and by back-substituting, we have 
\[\ln|u| + C =  \ln|x^2 + 1| + C=\ln(x^2 + 1) + C.\]
Thus, using $u$-substitution we can conclude that
\[\int \frac{2x}{x^2 + 1} \ dx =  \ln(x^2 + 1) + C.\]
\end{example}


\begin{problem} (problem 5) Compute $\displaystyle{\int \frac{4x^3}{x^4 +2} \ dx}$.\\
Let $u = \answer{x^4 + 2}$. Then $du = \answer{4x^3 dx}$.\\
\begin{hint}
Don't forget the `dx' in your answer for `du'.
\end{hint}
Convert to an intergal in the variable $u$:
\[\int \frac{4x^3}{x^4 +2} \ dx = \int\answer{1/u du}\]
\begin{hint}
Don't forget the `du' in your integral.
\end{hint}

\[\int \frac{4x^3}{x^4 +2} \ dx = \answer{\ln|x^4 +2|} +C.\]
\end{problem}



\begin{example}[example 6] Compute 
\[\int e^x\sin(e^x) \ dx.\]
We let $u = e^x$.  We have,
\[u = e^x\]
\[du = e^x \ dx\]

and the integral can be written as 
\[\int e^x\sin(e^x) \ dx = \int \sin(e^x) \cdot e^x \  dx = \int \sin(u) \ du.\]
The last integral can be computed as 
\[\int \sin(u) \ du = -\cos(u) + C,\]
and by back-substituting, we have 
\[-\cos(u) + C = -\cos(e^x) + C.\]
Thus, using $u$-substitution we can conclude that
\[\int e^x\sin(e^x) \ dx =  -\cos(e^x) + C.\]
\end{example}




\begin{problem}(problem 6)\\
Compute $\displaystyle{\int \frac{\cos(\ln(x))}{x} \ dx}$.\\
Let $u = \answer{\ln(x)}$. Then $du = \answer{1/x dx}$.\\
\begin{hint}
Don't forget the `dx' in your answer for `du'.
\end{hint}
Convert to an intergal in the variable $u$:
\[\int \frac{\cos(\ln(x))}{x} \ dx = \int\answer{\cos(u) du}\]
\begin{hint}
Don't forget the `du' in your integral.
\end{hint}

\[\int \frac{\cos(\ln(x))}{x} \ dx = \answer{\sin(\ln(x))} +C.\]
\end{problem}


\begin{example}[example 7] Compute 
\[\int 3x^2\sec(x^3)\tan(x^3) \ dx.\]
Let $u = x^3$.  Then we have,
\[u = x^3\]
\[du = 3x^2 \ dx\]

and the integral can be written as 
\begin{align*}
\int 3x^2\sec(x^3)\tan(x^3) \ dx &= \int \sec(x^3)\tan(x^3) \cdot 3x^2 \ dx\\
&= \int \sec(u)\tan(u) \ du.
\end{align*}
The last integral can be computed as 
\[\int \sec(u)\tan(u) \ du = \sec(u) + C,\]
and by back-substituting, we have 
\[\sec(u) + C = \sec(x^3) + C.\]
Thus, using $u$-substitution we can conclude that
\[\int 3x^2\sec(x^3)\tan(x^3) \ dx =  \sec(x^3) + C.\]
\end{example}

\begin{problem}(problem 7)
\begin{hint}
Let $u = e^x$
\end{hint}
\begin{hint}
Compute $du$
\end{hint}
\[\int e^x\sec(e^x)\tan(e^x) \ dx = \answer{\sec(e^x)} +C.\]
\end{problem}


\begin{example}[example 8] Compute 
\[\int x^3\cos(x^4) \ dx.\]
Let $u = x^4$.  Then,
\[u = x^4\]
\[du = 4x^3 \ dx\]

and the integral can be written as 
\begin{align*}
\int x^3\cos(x^4) \ dx &= \int \cos(x^4) \cdot x^3\  dx \\
&=  \int \cos(x^4)\cdot \tfrac14 \cdot 4x^3\  dx\\
&=  \int \tfrac14\cos(u) \ du.
\end{align*}
The last integral can be computed as 
\[\int \tfrac14 \cos(u) \ du = \tfrac14 \sin(u) + C,\]
and by back-substituting, we have 
\[\tfrac14 \sin(u) + C = \tfrac14 \sin(x^4) + C.\]
Thus, using $u$-substitution we can conclude that
\[\int x^3\cos(x^4) \ dx =  \tfrac14 \sin(x^4) + C.\]
\end{example}

\begin{problem}(problem 8)
\begin{hint}
Let $u = x^2$
\end{hint}
\begin{hint}
Compute $du$
\end{hint}
\[\int x\cos(x^2) \ dx = \answer{\sin(x^2)/2} +C.\]
\end{problem}


\begin{example}[example 9] Compute 
\[\int xe^{-x^2} \ dx.\]
Let $u = -x^2 $.  Then we have,
\[u = -x^2\]
\[du = -2x \ dx\]
and the integral can be written as
\begin{align*}
\int xe^{-x^2} \ dx &= \int e^{-x^2} \cdot x\  dx \\
&=  \int e^{-x^2}( -\tfrac12)\ (-2x)\  dx \\
&=  \int -\tfrac12 e^u \ du.
\end{align*}
The last integral can be computed as 
\[ \int -\tfrac12 e^u \ du = -\tfrac12 e^u + C,\]
and by back-substituting, we have 
\[-\tfrac12 e^u + C = -\tfrac12 e^{-x^2} + C.\]
Thus, using $u$-substitution we can conclude that
\[\int xe^{-x^2} \ dx =  -\tfrac12 e^{-x^2} + C.\]
\end{example}


\begin{problem}(problem 9)
\begin{hint}
Let $u = x^3$
\end{hint}
\begin{hint}
Compute $du$
\end{hint}
\[\int x^2e^{x^3} \ dx = \answer{e^{x^3}/3} +C.\]
\end{problem}




\begin{example}[example 10] Compute 
\[\int \sin(3x) \ dx.\]
Let $u = 3x$.  Then we have,
\[u = 3x\]
\[du = 3 \ dx\]
and the integral can be written as 
\[\int\sin(3x) \ dx =  \int \sin(3x) \cdot \tfrac13\cdot 3 \   dx =   \int \tfrac13 \sin(u) \ du.\]
The last integral can be computed as 
\[ \int \tfrac13 \sin(u) \ du = -\tfrac13 \cos(u) + C,\]
and by back-substituting, we have 
\[-\tfrac13 \cos(u) + C = -\tfrac13 \cos(3x) + C.\]
Thus, using $u$-substitution we can conclude that
\[\int \sin(3x) \ dx =  -\tfrac13 \cos(3x) + C.\]
\end{example}

\begin{problem}(problem 10)
\begin{hint}
Let $u = 3x$
\end{hint}
\begin{hint}
Compute $du$
\end{hint}
\[\int \cos(3x) \ dx = \answer{1/3 \sin(3x)} +C.\]
\end{problem}






\begin{example}[example 11] Compute 
\[\int e^{\frac{x}{2}} \ dx.\]
Let $u = \frac{x}{2}$.  Then we have,
\[u = \frac{x}{2}\]
\[du = \tfrac12 \ dx\]
and the integral can be written as 
\[\int e^{\frac{x}{2}} \ dx =  \int e^{\frac{x}{2}} \cdot 2\cdot \tfrac{1}{2}  \   dx =   \int 2e^u \ du.\]
The last integral can be computed as 
\[\int 2e^u \ du = 2 e^u + C,\]
and by back-substituting, we have 
\[2e^u + C = 2e^{\frac{x}{2}}+ C.\]
Thus, using $u$-substitution we can conclude that
\[\int e^{x/2} \ dx = 2e^{x/2} + C.\]
\end{example}


\begin{problem}(problem 11)
\begin{hint}
Let $u = 5x$
\end{hint}
\begin{hint}
Compute $du$
\end{hint}
\[\int e^{5x} \ dx = \answer{1/5 e^{5x}} +C.\]
\end{problem}


\begin{example}[example 12] Compute 
\[\int (4x+3)^5 \ dx.\]
Let $u = 4x+3$. Then we have,
\[u = 4x+3\]
\[du = 4 \ dx\]
and the integral can be written as 
\[\int (4x+3)^5 \ dx =   \int (4x+3)^5 \cdot \tfrac14\cdot 4  \   dx =   \int \tfrac14 u^5 \ du.\]
The last integral can be computed as 
\[\tfrac14  \int u^5 \ du = \tfrac14  \cdot \tfrac{u^6}{6} + C = \tfrac{u^6}{24} + C,\]
and by back-substituting, we have 
\[\tfrac{u^6}{24} + C = \tfrac{(4x+3)^6}{24}+ C.\]
Thus, using $u$-substitution we can conclude that
\[\int (4x+3)^5 \ dx = \tfrac{1}{24}(4x+3)^6 + C.\]
\end{example}




\begin{problem}(problem 12)
\begin{hint}
Let $u = 2x - 5$
\end{hint}
\begin{hint}
Compute $du$
\end{hint}
\[\int (2x - 5)^4 \ dx = \answer{\frac{1}{10}(2x-5)^5} +C.\]
\end{problem}


\begin{example}[example 13] Compute 
\[\int \frac{1}{x\ln^2(x)} \ dx.\]
Let $u = \ln(x)$. Then we have,
\[u = \ln(x)\]
\[du = \tfrac1x \ dx\]
and the integral can be written as 
\[\int \frac{1}{x\ln^2(x)} \ dx = \int \frac{1}{\ln^2(x)} \cdot \frac{1}{x}\  dx = \int \frac{1}{u^2} \ du.\]
The last integral can be computed as 
\[\int \frac{1}{u^2} \ du = \int u^{-2} \ du = \tfrac{u^{-1}}{-1} + C 
= -\frac{1}{u} + C,\]
and by back-substituting, we have 
\[-\frac{1}{u} + C =  -\frac{1}{\ln(x)} + C.\]
Thus, using $u$-substitution we can conclude that
\[\int \frac{1}{x\ln^2(x)} \ dx =  -\frac{1}{\ln(x)} + C.\]
\end{example}


\begin{problem}(problem 13)
\begin{hint}
Let $u = \ln(x)$
\end{hint}
\begin{hint}
Compute $du$
\end{hint}
\[\int \frac{1}{x\ln^3(x)} \ dx = \answer{- \ln^{-2}(x)/2} +C.\]
\end{problem}

\begin{example}[example 14] Compute 
\[\int \sin^4(x)\cos(x) \ dx.\]
Let $u = \sin(x)$. Then we have,
\[u = \sin(x)\]
\[du = \cos(x) \ dx\]
and the integral can be written as 
\[\int \sin^4(x)\cos(x) \ dx  = \int u^4 \ du.\]
The last integral can be computed as 
\[\int u^4 \ du = \tfrac{u^5}{5} + C,\]
and by back-substituting, we have 
\[\tfrac{u^5}{5} + C = \tfrac15 \sin^5(x) + C.\]
Thus, using $u$-substitution we can conclude that
\[\int \sin^4(x)\cos(x) \ dx =  \tfrac15 \sin^5(x) + C.\]
\end{example}



\begin{problem}(problem 14)
\begin{hint}
Let $u = \tan(x)$
\end{hint}
\begin{hint}
Compute $du$
\end{hint}
\[\int \tan^5(x)\sec^2(x) \ dx = \answer{\tan^6(x)/6} +C.\]
\end{problem}

\begin{example}[example 15] Compute 
\[\int \tan(x) \ dx.\]
First rewrite the integral:
\[\int \tan(x) \ dx =\int \frac{\sin(x)}{\cos(x)} \ dx.\]
Now, let $u = \cos(x)$; then $du = -\sin(x) \ dx$
and the integral can be written as
\begin{align*}
\int \frac{\sin(x)}{\cos(x)} \ dx &= \int \frac{1}{\cos(x)}\ \sin(x) \  dx \\
 &=  - \int \frac{1}{\cos(x)}\ \big(-\sin(x)\big) \  dx\\
&=-\int \frac{1}{u} \ du.
\end{align*}
The last integral can be computed as 
\[-\int \frac{1}{u} \ du = -\ln|u| + C,\]
and by back-substituting, we have 
\[-\ln|u| + C = -\ln|\cos(x)| + C = \ln|\sec(x)| +C.\]
Thus, using $u$-substitution we can conclude that
\[\int \tan(x) \ dx =  \ln|\sec(x)| + C.\]
\end{example}

\begin{problem}(problem 15)
\begin{hint}
Rewrite: $\cot(x) = \frac{\cos(x)}{\sin(x)}$
\end{hint}
\begin{hint}
Let $u = \sin(x)$
\end{hint}
\begin{hint}
Compute $du$
\end{hint}
\[\int \cot(x) \ dx = \answer{\ln|\sin(x)|} +C.\]


\end{problem}


\begin{example}[example 16] Compute 
\[\int \sec(x) \ dx.\]
First rewrite the integral:
\[\int \sec(x) \ dx =\int \sec(x)\frac{\sec(x)+\tan(x)}{\sec(x)+\tan(x)} \ dx.\]
Distributing in the numerator, we get
\[\int \sec(x)\frac{\sec(x)+\tan(x)}{\sec(x)+\tan(x)} \ dx = \int \frac{\sec^2(x)+\sec(x)\tan(x)}{\sec(x)+\tan(x)} \ dx.\]
Now, let $u = \sec(x) + \tan(x)$. Then $du = [\sec(x)\tan(x) + \sec^2(x)] \ dx$ and the integral can be rewritten as
\[ \int \frac{\sec^2(x)+\sec(x)\tan(x)}{\sec(x)+\tan(x)} \ dx = \int \frac{1}{u} \ du.\]
The last integral can be computed as
\[\int \frac{1}{u} \ du = \ln|u| + C,\]
and by back-substituting, we have 
\[\ln|u| + C = \ln|\sec(x) + \tan(x)| + C.\]
Thus, using $u$-substitution we can conclude that
\[\int \sec(x) \ dx =  \ln|\sec(x) + \tan(x)| + C.\]
\end{example}


\begin{center}
\begin{foldable}
\unfoldable{Here is a detailed, lecture style video on $u$-substitution:}
\youtube{5yb7_e9PCQU}
\end{foldable}
\end{center}

\end{document}
