\documentclass[handout]{ximera}

\input{../preamble}

\outcome{Define and compute partial derivatives.}

\title{3.3 Partial Derivatives}



\begin{document}

\begin{abstract}
In this section we define and compute partial derivatives.
\end{abstract}

\maketitle

The derivative of a function $f(x)$ is defined by:

\[
f\,'(x) =  \frac{d}{dx} f(x) = \lim_{h \to 0} \frac{f(x+h) -f(x)}{h}
\]

The symbol $\frac{d}{dx}$ is called the derivative operator. If we state that $y = f(x)$, then the derivative can also be written as $\frac{dy}{dx}$.
The expression in the limit is called the difference quotient and it gives the slope of a secant line.
%The situation with a function of two variables is more complicated because at a point on the graph of $z = f(x,y)$ there are 
%infinitely many directions to move rather than just two. 
The partial derivatives of a function of two variables are defined analogously to the single variable case.

\begin{definition}[Partial Derivatives]
The partial derivative of $f(x,y)$ with respect to $x$, denoted $f_x(x,y)$ or $\frac{\partial}{\partial x} f(x,y)$, is defined by
\[
f_x(x,y)= \lim_{h \to 0} \frac{f(x+h, y) -f(x, y)}{h}
\]

The partial derivative with respect to $y$, denoted $f_y(x,y)$ or $\frac{\partial}{\partial y} f(x,y)$, is defined by


\[
f_y(x,y) = \lim_{h \to 0} \frac{f(x, y+h) -f(x, y)}{h}
\]

The symbols $\frac{\partial}{\partial x}$ and $\frac{\partial}{\partial y}$ are called partial derivative operators.

\end{definition}



\begin{example}[Example 1]
Use the definition of partial derivative to compute $f_x(x,y)$ for the function
\[
f(x,y) = 2xy^2 + 4xy - 2x -1
\]
We compute $f(x+h, y)$ as an aside:
\begin{align*}
f(x+h, y) &= 2(x+h)y^2 + 4(x+h)y - 2(x+h)  -1\\
          &= 2xy^2 + 2hy^2 + 4xy + 4hy - 2x - 2h - 1
\end{align*}
Note that among the 7 terms in this expression, 4 of them are exactly the terms in the original function.
Hence, the numerator of the difference quotient will simplify to:
\[
f(x+h, y) - f(x,y) =  2hy^2 + 4hy - 2h
\]
Observe that each of these terms contains a factor of $h$. Thus the difference quotient simplifies to
\[
\frac{f(x+h, y) -f(x, y)}{h} = 2y^2 + 4y - 2
\]
Finally, we take the limit as $h \to 0$ to obtain the partial derivative with respect to $x$:
\[
f_x(x,y) = \lim_{h \to 0} \left(2y^2 + 4y - 2\right) = 2y^2 + 4y - 2
\]

\end{example}

\begin{remark}
Note that this result can be obtained by treating the variable $y$ as a constant and computing an ordinary derivative with respect to $x$.
\end{remark}

\begin{problem}(Problem 1)
Use the definition of partial derivative to compute $f_x(x,y)$ for the function
\[
f(x,y) = 3x^2y + 5xy - 2y - 4
\]
Start by computing $f(x+h, y)$:
\[
f(x+h, y) = \answer{3(x+h)^2y + 5(x+h)y - 2y - 4}
\]

The numerator of the difference quotient is:
\[
f(x+h,y) - f(x,y) = \answer{6hxy + 3h^2y + 5hy}
\]

The difference quotient simplifies to:
\[
\frac{f(x+h,y) - f(x,y)}{h} = \answer{6xy + 3hy + 5y}
\]


The partial derivative with respect to $x$ is
\[
\frac{\partial}{\partial x} f(x,y) = \answer{6xy + 5y}
\]

\end{problem}

\begin{example}[Example 2]
Use the definition of partial derivative to compute $f_y(x,y)$ for the function
\[
f(x,y) = 2xy^2 + 4xy - 2x -1
\]
We compute $f(x, y+h)$ as an aside:
\begin{align*}
f(x, y+h) &= 2x(y+h)^2 + 4x(y+h) - 2x  -1\\
          &= 2x(y^2 + 2hy + h^2) + 4xy + 4hx - 2x - 1\\
          &= 2xy^2 + 4hxy + 2h^2x + 4xy + 4hx - 2x - 1
\end{align*}
Note that among the 7 terms in this expression, 4 of them are exactly the terms in the original function.
Hence, the numerator of the difference quotient will simplify to:
\[
f(x+h, y) - f(x,y) =  4hxy + 2h^2x  + 4hx
\]
Observe that each of these terms contains a factor of $h$. Thus the difference quotient simplifies to
\[
\frac{f(x+h, y) -f(x, y)}{h} = 4xy + 2hx +4x
\]
Finally, we take the limit as $h \to 0$ to obtain the partial derivative with respect to $x$:
\[
f_x(x,y) = \lim_{h \to 0} \left(4xy + 2hx +4x\right) = 4xy + 4x
\]

\end{example}

\begin{remark}
Note that this result can be obtained by treating the variable $x$ as a constant and computing an ordinary derivative with respect to $y$.
\end{remark}

\begin{problem}(Problem 2)
Use the definition of partial derivative to compute $f_y(x,y)$ for the function
\[
f(x,y) = 3x^2y + 5xy - 2y - 4
\]

Start by computing $f(x, y+h)$:
\[
f(x, y+h) = \answer{3x^2(y+h) + 5x(y+h) - 2(y+h) - 4}
\]

The numerator of the difference quotient is:
\[
f(x,y+h) - f(x,y) = \answer{3hx^2 + 5hx - 2h}
\]

The difference quotient simplifies to:
\[
\frac{f(x,y+h) - f(x,y)}{h} = \answer{3x^2 + 5x -2}
\]

The partial derivative with respect to $y$ is
\[
\frac{\partial}{\partial y} f(x,y) = \answer{3x^2 + 5x -2}
\]
\end{problem}

As was noted in the remarks following each of the two previous examples, partial derivatives can be computed by considering one of the variables to be constant.

\begin{example}[Example 3]
Find $f_x(x,y)$ for the function 
\[
f(x,y) = x^4y^3 + 2xy + y\sin(x) - e^y
\]

Since we are trying to find the partial derivative with respect to $x$, we treat the variable $y$ as a constant.
Differentiating term by term in this fashion gives:
\[
f_x(x,y) = 4x^3y^3 + 2y + y\cos(x)
\]
\end{example}

\begin{problem}(Problem 3a)
Find $f_x(x,y)$ for the function 
\[
f(x,y) = x^5y^2 - 3x\sqrt y + y\ln(x) + 3y
\]

\[
f_x(x,y) = \answer{5x^4y^2 - 3\sqrt y + y/x}
\]
\end{problem}

\begin{problem}(Problem 3b)
Find $f_x(x,y)$ for the function 
\[
f(x,y) = \frac{2y}{x} + y^2\tan(x) + 4\sec(y)
\]
\[
f_x(x,y) = \answer{-\frac{2y}{x^2} + y\sec^2(x)}
\]
\end{problem}


\begin{example}[Example 4]
Find $f_y(x,y)$ for the function 
\[
f(x,y) = x^4y^3 + 2x\sqrt{y} + y^2\cos(x) - e^y
\]

Since we are trying to find the partial derivative with respect to $y$, we treat the variable $x$ as a constant.
Differentiating term by term in this fashion gives:
\[
f_y(x,y) = 3x^4y^2 + \frac{x}{\sqrt{y}} + 2y\cos(x) - e^y
\]
\end{example}

\begin{problem}(Problem 4a)
Find $f_y(x,y)$ for the function 
\[
f(x,y) = x^5y^2 - \frac{3x}{y} + y\ln(x) + 3y
\]

\[
f_y(x,y) = \answer{2x^5 y + \frac{3x}{y^2} + \ln(x) + 3}
\]
\end{problem}

\begin{problem}(Problem 4b)
Find $f_y(x,y)$ for the function 
\[
f(x,y) = \frac{2y}{x} + y^2\tan(x) + 4\sec(y)
\]

\[
f_y(x,y) = \answer{\frac{2}{x} + 2y\tan(x) + 4\sec(y)\tan(y)}
\]
\end{problem}

The next example uses the chain rule.  Recall that $\frac{d}{dx} \sqrt x = \frac{1}{2\sqrt x}$.

\begin{example}[Example 5]
Compute $f_x(x,t)$ and $f_t(x,t)$ for the function 
\[
f(x,t) = \sqrt{3x + 4t}
\]
First, note that the independent variables in the function $f$ are $x$ and $t$.
The function $f$ can be written as a composition of two functions:
\[
f(x,t) = \sqrt {u}, \quad \text{where} \quad u= u(x,t) = 3x + 4t
\]
From the chain rule,
\begin{align*}
f_x(x,t) &= \frac{d}{du}\left( \sqrt u\right) \cdot u_x\\
  & = \frac{1}{2\sqrt u} \cdot 3\\
  &= \frac{3}{2\sqrt{3x + 4t}}
\end{align*}
Similarly:
\begin{align*}
f_t(x,t) &= \frac{d}{du} \sqrt u \cdot u_t\\
  & = \frac{1}{2\sqrt u} \cdot 4\\
  &= \frac{4}{2\sqrt{3x + 4t}}\\
 &= \frac{2}{\sqrt{3x + 4t}}
\end{align*}
  
\end{example}

\begin{problem}(Problem 5)
Compute the partial derivatives $f_x$ and $f_y$ for the function
\[
f(x,y) = \cos(x^3y^4)
\]
\begin{hint}
Both partial derivatives require the chain rule
\end{hint}

\[
f_x = \answer{-3x^2y^4 \sin(x^3y^4)} \quad \text{and} \quad f_y = \answer{-4x^3y^3 \sin(x^3y^4)}
\]
\end{problem}

In the next example, we compute the partial derivatives of a function of three variables.

\begin{example}[Example 6]
Find $w_x, w_y$ and $w_z$ for the function
\[
w = y\tan(x+2z)
\]
To find $w_x$, we treat $y$ and $z$ as constants:
\[
w_x = y\sec^2(x+2z) \cdot 1 = y\sec^2(x+2z)
\]
Note that we used the chain rule with inside function $x + 2z$, whose derivative with respect to $x$ is just $1$.\\
To find $w_y$, we treat $x$ and $z$ as constants, so the factor $\tan(x+2z)$ is treated as constant and
\[
w_y = \tan(x+2z)
\]
Finally, to find $w_z$, we treat $x$ and $y$ as constants and we use the chain rule:
\[
w_z = y\sec^2(x+2z) \cdot 2 = 2y\sec^2(x+2z)
\]
\end{example}

\begin{problem}(Problem 6)
Compute the partial derivatives $f_x, f_y$ and $f_z$ for the function
\[
f(x,y,z) = \sqrt{x^2 + y^2 + z^2}
\]
\begin{hint}
All three partial derivatives require the chain rule
\end{hint}
\[
f_x = \answer{\frac{x}{\sqrt{x^2 + y^2 + z^2}}}
\]
\[
f_y = \answer{\frac{y}{\sqrt{x^2 + y^2 + z^2}}}
\]
\[
f_z = \answer{\frac{z}{\sqrt{x^2 + y^2 + z^2}}}
\]

\end{problem}

In the next example we use the product rule in addition to the chain rule.

\begin{example}[Example 7]
Compute $f_x(x,y)$ and $f_y(x,y)$ for the function 
\[
f(x,y) = x\sin(xy)
\]
Viewed as a function of $x$, $f$ is a product first and then a composition. We will need to use the product rule and then
the chain rule to compute $f_x$.
We have
\begin{align*}
f_x(x,y) &= \sin(x,y) + x \frac{\partial}{\partial x} \sin(xy)\\
         & = \sin(x,y) + x \cos(xy) \cdot y\\
         & = \sin(x,y) + xy \cos(xy)
\end{align*}
As a function of $y, f$ is a composition of the sine function and the function $xy$, so the chain rule gives:
\[
f_y(x,y) = x \cos(xy) \cdot x = x^2 \cos(xy)
\]

\end{example}


\begin{problem}(Problem 7a)
Let $z = x\ln(x+ 2y)$. Compute the partial derivatives:
\[
\frac{\partial z}{\partial x} = \answer{\frac{x}{x+2y} + \ln(x+2y)}
\]
\[
\frac{\partial z}{\partial y} = \answer{\frac{2x}{x+2y}}
\]
\end{problem}



\begin{problem}(Problem 7b)
Compute the partial derivatives $f_x, f_y$ and $f_z$ for the function
\[
f(x,y,z) = xy^2 e^{-xz}
\]
\begin{hint}
$f_x$ requires the product rule and the chain rule
\end{hint}

\[
f_x = \answer{y^2e^{-xz} - xy^2ze^{-xz}}
\]
\[
f_y = \answer{2xye^{-xz}}
\]
\begin{hint}
$f_z$ requires the chain rule
\end{hint}

\[
f_z = \answer{-x^2y^2 e^{-xz}}
\]
\end{problem}


\section{Higher Order Derivatives}

\begin{example}[Example 8]
Compute the mixed second order partial derivatives $f_{xy}$ and $f_{yx}$ for the function 
\[
f(x,y) = x^3y^4
\]
We will compute $f_{xy}$ first.  To do this, we compute the partial derivative of $f$ with respect to $x$ first and then compute the partial 
derivative with respect to $y$.  In other words, $f_{xy} = (f_x)_y$.  We have:
\[
f_x(x,y) = 3x^2y^4 \quad \text{and} \quad f_{xy} = 12x^2y^3
\]
Next, we compute $f_{yx}$ by computing the partial derivative with respect to $y$ first and then $x$:
\[
f_y(x,y) = 4x^3y^3 \quad \text{and} \quad f_{yx} = 12x^2y^3
\]
Notice that in this example
\[
f_{xy} = f_{yx}
\]
\end{example}

\begin{problem}(Problem 8)
Compute the mixed second order partial derivatives $f_{xy}$ and $f_{yx}$ for the function 
\[
f(x,y) = x^5 y^3
\]
Are they equal?
\end{problem}

The next theorem asserts that as long as the mixed second order partial derivatives $f_{xy}$ and $f_{yx}$  are continuous then they are equal.
\begin{theorem}[Clairault's Theorem]
If the mixed second order partial derivatives $f_{xy}(x,y)$ and $f_{yx}(x,y)$ are continuous in a disc centered at a point, 
then they are equal at that point.
\end{theorem}


\begin{remark}
In practice, the functions we will be differentiating are continuous on their domains, 
so we will freely interchange the order of differentiation.
\end{remark}

\begin{example}[Example 9]
Verify that $f_{xy} = f_{yx}$ for the function $f(x,y) = e^{xy}\sin(y)$.\\
We compute $f_{xy}$ first:
\[
f_x(x,y) = ye^{xy}\sin(y)
\]
and using the product rule (for three functions):
\[
f_{xy} = e^{xy}\sin(y) + xye^{xy}\sin(y) + ye^{xy}\cos(y)
\]
Next, we compute $f_{yx}$:
\[
f_y = xe^{xy}\sin(y) + e^{xy}\cos(y)
\]
and the product rule gives:
\[
f_{yx} = e^{xy}\sin(y) + xy e^{xy}\sin(y) +ye^{xy} \cos(y)
\]
Comparing, we can see that the result of Clairaut's Theorem holds, i.e., $f_{xy} = f_{yx}$.
\end{example}

\begin{problem}(Problem 9)
Verify that $f_{xy} = f_{yx}$ for the function $f(x,y) = e^x\tan(xy)$.\\
\[
f_x(x,y) = \answer{e^x \tan(xy) + ye^x \sec^2(xy)}
\]
\[
f_y(x,y) = \answer{xe^x\sec^2(xy)}
\]
\[
f_{xy}(x,y) = f_{yx}(x,y) = \answer{e^x\sec^2(xy) + xe^x\sec^2(xy) + 2xye^x \sec^2(xy)\tan(xy)}
\]
\end{problem}

\subsection{Harmonic Functions}
\begin{definition}[Harmonic]
A function $f(x,y)$ is called harmonic if 
\[
\Delta f = f_{xx} + f_{yy} = 0
\]
for all $(x,y)$. The symbol $\Delta$ is called the Laplace operator or the Laplacian.
\end{definition}

\begin{example}[Example 10]
Show that the function is harmonic:
\[
f(x,y) = \tan^{-1}\left(\frac{y}{x}\right)
\]
Recalling that 
\[
\frac{d}{dx}\tan^{-1}(x) = \frac{1}{1+x^2} \quad \text{and} \quad \frac{d}{dx} \left(\frac{1}{x}\right) = -\frac{1}{x^2}
\]
we begin with the partial derivatives with respect to $x$:
\[
f_x(x,y) = \frac{1}{1+\left(\frac{y}{x}\right)^2} \cdot \left(-\frac{y}{x^2}\right) = -\frac{y}{x^2 + y^2}
\]
The second derivative with respect to $x$ follows from the quotient rule:
\[
f_{xx}(x,y) = -\frac{(x^2 + y^2) \cdot 0 - y \cdot 2x}{(x^2 + y^2)^2} = \frac{2xy}{(x^2 + y^2)^2}
\]
Now for the partial derivatives with respect to $y$:
\[
f_y(x,y) = \frac{1}{1+\left(\frac{y}{x}\right)^2} \cdot \frac{1}{x} = \frac{1}{x + \frac{y^2}{x}} = \frac{x}{x^2 + y^2}
\]
And the second derivative with respect to $y$:
\[
f_{yy}(x,y) = \frac{(x^2+y^2)\cdot 0 - x \cdot 2y}{(x^2 + y^2)^2} = -\frac{2xy}{(x^2 + y^2)^2}
\]
Finally, we add the pure second derivatives to obtain the Laplacian:
\[
\Delta f(x,y) = f_{xx}(x,y) + f_{yy}(x,y) = \frac{2xy}{(x^2 + y^2)^2}-\frac{2xy}{(x^2 + y^2)^2} =0
\]
demonstrating that the original function is harmonic.
\end{example}

\begin{problem}(Problem 10a)
Show that the function is harmonic:
\[
f(x,y) = x^2 + 4xy - y^2 + 5x - 6y +2
\]

\end{problem}

\begin{problem}(Problem 10b)
Show that the function is harmonic:
\[
f(x,y) = e^x \cos(y)
\]

\end{problem}

\begin{problem}(Problem 10c)
Show that the function is harmonic:
\[
f(x,y) = \ln(x^2 + y^2)
\]

\end{problem}
\end{document}
