\documentclass[handout]{ximera}

\input{../preamble}

\outcome{Find limits at infinity}

\title{1.6 End Behavior}


\begin{document}

\begin{abstract}
Find limits at infinity.
\end{abstract}

\maketitle

\section{End Behavior}
 



%\begin{center}
%{\bf End Behavior}
%\end{center}

In this section we consider limits as $x$ approaches either $\infty$ or $-\infty$.
There is a connection to the value of these limits and horizontal asymptotes.

\begin{theorem}
(1) If the limit
\[
\lim_{x \to \infty} f(x) = L_1,
\]
then the line $y=L_1$ is a horizontal asymptote for the graph of $y = f(x)$ on the right end.\\
(2) If the limit
\[
\lim_{x \to -\infty} f(x) = L_2,
\]
then the line $y=L_2$ is a horizontal asymptote for the graph of $y = f(x)$ on the left end.
\end{theorem}



\begin{example}[example 1]
Find $\lim_{x \to \infty} \dfrac{1}{x}.$
  We argue as follows. If $x$ is a very large number, 
	then $1/x$ will be a very small number, near zero.  Furthermore, as $x$ increases, $1/x$ will decrease.
	
	Hence
	\[\lim_{x \to \infty} \frac{1}{x}= 0.\]
	This is evident from the graph of $y=1/x$ shown below.
	
	%\[\graph[panel, xAxisLabel=``x'', yAxisLabel=``y'', xmin=-3, xmax=75]{y = 1/x}\]
	
	The graph of the function $f(x) = \frac{1}{x}$ also provides evidence for this conclusion.  
	
	\[\graph{y=1/x}\]
	
	Lastly, the value of the limit corresponds to the horizontal asymptote of the graph, namely
	$y = 0$ in this example.
\end{example}




\begin{problem}(problem 1)
  Compute the limit:
  \[
  \lim_{x \to \infty} \frac{7}{x^2}
  \]
  
    \begin{hint}
      As $x$ goes to infinity, so does $x^2$
    \end{hint}
    \begin{hint}
      As the denominator grows, the fraction shrinks
    \end{hint}
    \begin{hint}
      The fraction never shrinks below 0
    \end{hint}
		The value of the limit is
		 $\answer{0}$
		
\end{problem}

An important generalization of the last example and problem, which follows from a similar analysis is 
\[\lim_{x \to \pm \infty} \frac{a}{x^n} = 0 \]
for any constant, $a$, and any positive exponent, $n$.

We will exploit this important fact in the next two examples.


\begin{example}[example 2]
Compute the limit:
\[
\lim_{x \to \infty} \frac{3x^2 + 5x + 2}{2x^2 -x- 4}.
\]

First note that as $x\to \pm \infty$, a polynomial, $p(x) \to \pm \infty$ according to it leading term.
In this example, since the lead terms $3x^2$ and $2x^2$ both go to $\infty$ as $x \to \infty$, 
our limit has the indeterminate form
$\frac{\infty}{\infty}$.
To resolve this issue, we will factor out of both the numerator and the denominator 
the highest power of $x$ seen in the denominator.  So, in this example, we will factor $x^2$ from both.
In the numerator, 
\[3x^2 + 5x + 2 = x^2\left(3 + \frac{5}{x} + \frac{2}{x^2}\right)\]
and in the denominator,
\[2x^2 -x -4 = x^2\left(2- \frac{1}{x} - \frac{4}{x^2}\right)\]

With these factorizations, our limit becomes

\begin{align*}
\lim_{x \to \infty} \frac{3x^2 + 5x + 2}{2x^2 -x- 4} &= 
\lim_{x \to \infty} \frac{x^2\left(3 + \frac{5}{x} + \frac{2}{x^2}\right)}{x^2\left(2- \frac{1}{x} - \frac{4}{x^2}\right)} \\ \\
&=\lim_{x \to \infty} \frac{3 + \frac{5}{x} + \frac{2}{x^2}}{2- \frac{1}{x} - \frac{4}{x^2}} \\ \\
&=\frac{3 + 0 + 0}{2- 0 - 0} \\ \\
&= \frac32.
\end{align*}

The result of this limit means that the line $y = 3/2$ is a horizontal asymptote
for the graph of $y = \frac{3x^2 + 5x + 2}{2x^2 -x- 4}$ on the right end.
\end{example}


\begin{problem}(problem 2a)
  Compute the limit:
  \[
  \lim_{x \to -\infty} \frac{4x^2 + 3x - 2}{2x^2 - 2x + 5}
  \]
  
    \begin{hint}
      When you `plug in' $x = -\infty$, you get an $\frac{\infty}{\infty}$ form
    \end{hint}
    \begin{hint}
      Determine the highest power of $x$ in the denominator
    \end{hint}
    \begin{hint}
      Factor this power from both the numerator and denominator and cancel it
    \end{hint}
    \begin{hint}
      $\frac{a}{x^n} \to 0$ as $x \to \infty$.
    \end{hint}
		The value of the limit is
		 $\answer{2}$
		
\end{problem}



\begin{problem}(problem 2b)
  Compute the limit:
  \[
  \lim_{x \to \infty} \frac{3 + 2x^2 - x^3}{5x^3 - 2x -4}
  \]
  
    \begin{hint}
      When you `plug in' $x = \infty$, you get an $\frac{\infty}{\infty}$ form
    \end{hint}
    \begin{hint}
      Determine the highest power of $x$ in the denominator
    \end{hint}
    \begin{hint}
      Factor this power from both the numerator and denominator and cancel it
    \end{hint}
    \begin{hint}
      $\frac{a}{x^n} \to 0$ as $x \to \infty$.
    \end{hint}
		The value of the limit is
		 $\answer{-\frac15}$
		
\end{problem}




\begin{example}[example 3]
Compute the limit:
\[
\lim_{x \to -\infty} \frac{4x^2 - 3x - 6}{x^3 +8x^2 -3x + 7}.
\]


First note that as $x\to \pm \infty$, a polynomial, $p(x) \to \pm \infty$ according to it leading term.
In this example, the lead terms $4x^2$ and $x^3$  go to $\infty$ and $-\infty$ respectively, as $x \to -\infty$. 
Hence, our limit has the indeterminate form
$\frac{\infty}{-\infty}$.
To resolve this indeterminate form, we will factor out 
the highest power of $x$ in the denominator, namely $x^3$, from both the numerator and the denominator.  
In the numerator we get, 
\[4x^2 - 3x - 6 = x^3\left(\frac{4}{x} - \frac{3}{x^2} - \frac{6}{x^3}\right)\]
and in the denominator we get,
\[x^3 +8x^2 -3x + 7 = x^3\left(1 +  \frac{8}{x} - \frac{3}{x^2} + \frac{7}{x^3}\right)\]

Factoring the $x^3$ and canceling, the limit can be resolved as follows:

\begin{align*}
\lim_{x \to -\infty}\frac{4x^2 - 3x - 6}{x^3 +8x^2 -3x + 7} &= 
\lim_{x \to -\infty} \frac{x^3\left(\frac{4}{x}-\frac{3}{x^2} -\frac{6}{x^3}\right)}
{x^3\left(1 + \frac{8}{x}-\frac{3}{x^2}+\frac{7}{x^3}\right)} \\ \\
&=\lim_{x \to -\infty} \frac{\frac{4}{x}-\frac{3}{x^2} -\frac{6}{x^3}}{1 + \frac{8}{x}-\frac{3}{x^2}+\frac{7}{x^3}} \\ \\
&=\frac{0 - 0 - 0}{1 +0- 0 + 0} \\ \\
&= \frac01 \\
&= 0.
\end{align*}

The result of this limit means that the line $y = 0$ (the $x$-axis) is a horizontal asymptote
for the graph of $y = \dfrac{4x^2 - 3x - 6}{x^3 +8x^2 -3x + 7}$ on the right end.
\end{example}


\begin{problem}(problem 3a)
  Compute the limit:
  \[
  \lim_{x \to -\infty} \frac{x^2 - 5x - 6}{2x^3 + x -5}
  \]
  
    \begin{hint}
      When you `plug in' $x = \infty$, you get an $\frac{\infty}{\infty}$ form
    \end{hint}
    \begin{hint}
      Determine the highest power of $x$ in the denominator
    \end{hint}
    \begin{hint}
      Factor this power from both the numerator and denominator
    \end{hint}
    \begin{hint}
      Cancel the power of $x$ that was factored out
    \end{hint}
    \begin{hint}
      $\frac{a}{x^n} \to 0$ as $x \to -\infty$.
    \end{hint}
		The value of the limit is
		 $\answer{0}$
		
\end{problem}


\begin{problem}(problem 3b)
  Compute the limit:
  \[
  \lim_{x \to \infty} \frac{3x^3 - 5x + 6}{3-x+ 2x^3- x^4}
  \]
  
    \begin{hint}
      When you `plug in' $x = \infty$, you get an$\frac{\infty}{\infty}$ form
    \end{hint}
    \begin{hint}
      Determine the highest power of $x$ in the denominator
    \end{hint}
    \begin{hint}
      Factor this power from both the numerator and denominator
    \end{hint}
    \begin{hint}
      Cancel the power of $x$ that was factored out
    \end{hint}
    \begin{hint}
      $\frac{a}{x^n} \to 0$ as $x \to \infty$.
    \end{hint}
		The value of the limit is
		 $\answer{0}$
		
\end{problem}


\begin{problem}(problem 3c)
  Compute the limit:
  \[
  \lim_{x \to -\infty} \frac{x^3 - x + 1}{2x^2- 3}
  \]
  
    \begin{hint}
      When you `plug in' $x = \infty$, you get an $\frac{\infty}{\infty}$ form
    \end{hint}
    \begin{hint}
      Determine the highest power of $x$ in the denominator
    \end{hint}
    \begin{hint}
      Factor this power from both the numerator and denominator
    \end{hint}
    \begin{hint}
      Cancel the power of $x$ that was factored out
    \end{hint}
    \begin{hint}
      $\frac{a}{x^n} \to 0$ as $x \to \infty$.
    \end{hint}
		The value of the limit is
		(type infinity for $\infty$, -infinity for $-\infty$ or DNE)
		 $\answer{-\infty}$
		
\end{problem}


\begin{example}[example 4]

Compute the limit: 
\[
\lim_{x\to -\infty} e^x.
\]

Suppose $x$ is a large negative number.  Since $x$ is negative, $x = -|x|$ and so
\[
e^x = e^{-|x|} = \frac{1}{e^{|x|}},
\]
using the definition of negative exponents: $x^{-n} = \frac{1}{x^n}$.

Now note that as $x\to -\infty, |x| \to \infty$ and so 
\[
e^{|x|} \to \infty.
\]

Thus, 
\[
\frac{1}{e^{|x|}} \to 0,
\]
hence

\[
\lim_{x\to -\infty} e^x = 0.
\]

This means that the line $y=0$ is a horizontal asymptote of the graph of $y = e^x$,
as shown in the graph below.

\[
\graph{y=e^x}
\]

\end{example}

\begin{problem}(problem 4)
Compute 
\[ \lim_{x \to \infty} e^{-2x}\]

\begin{hint}
$e^x \to 0$ as $x \to -\infty$
\end{hint}

The value of the limit is
		(type infinity for $\infty$, -infinity for $-\infty$ or DNE)
		 $\answer{0}$
\end{problem}


\begin{example}[example 5]
Discuss
\[
\lim_{x\to \infty} \sin x
\]

As $x$ increases, the sine function oscillates between $-1$ and $1$ without approaching any particular value.
Hence
\[
\lim_{x\to \infty} \sin x \ \text{DNE}
\]
due to oscillation.
This is illustrated in the graph of $y=\sin x$ shown below.

\[
\graph{y=\sin(x)}
\]

\end{example}

\begin{problem}(problem 5)
Find the limit:
\[
 \lim_{x \to -\infty} \cos x
\]

\begin{hint}
$\cos(x)$ oscillates between $-1$ and $1$ with period $2\pi$
\end{hint}

The value of the limit is
		(type infinity for $\infty$, -infinity for $-\infty$ or DNE)
		 $\answer{DNE}$
\end{problem}

\begin{center}
\begin{foldable}
\unfoldable{Here is a detailed, lecture style video on finding limits at infinity:}
\youtube{FyhXNtLGr2o}
\end{foldable}
\end{center}





\end{document}













