\documentclass[handout]{ximera}

\input{../preamble}

\outcome{Determine tangent planes to surfaces.}

\title{3.5 Tangent Planes}



\begin{document}

\begin{abstract}
In this section we determine tangent planes to surfaces.
\end{abstract}

\maketitle

\begin{proposition}
Let $f(x,y)$ be a function of two variables and let $(x_0, y_0)$ be a point on the (smooth) level curve $f(x,y) = k$, i.e. $f(x_0, y_0) = k$.
Then, the gradient vector at this point, $\grad f(x_0, y_0)$ is orthogonal to the level curve.
\end{proposition}
\begin{proof}
Let $\vec r(t)$ be a parameterization of the (smooth) level curve $f(x,y) = k$ and let $\vec u \neq \vec 0$ be the direction 
vector for $\vec r(t)$ at the point $(x_0, y_0)$, i.e., 
$\vec u = \vec T(t)$. Then the rate of change of $f(x,y)$ in the direction of $\vec u$ at $(x_0, y_0)$ is zero since $f(x,y)$ is 
constant on the level curve $f(x,y) = k$ which implies that
\[
D_{\vec u} f(x_0, y_0) = 0
\]
But,
\[
0 = D_{\vec u} f(x_0, y_0)  = \grad f(x_0, y_0) \dotp \vec u
\]
from which we can conclude that the gradient is orthogonal to the level curve at the point $(x_0, y_0)$.
\end{proof}


\begin{example}[Example 1]
Verify the proposition by showing directly that the gradient vector is orthogonal to the level curve of the paraboloid $z = f(x,y) = x^2 + y^2$ at any point $(x,y)$.\\
The level curves have the form 
\[
x^2 + y^2 = k
\]
which (for $k >0$) is a circle centered at the origin with radius $\sqrt k$. 
A basic fact from geometry is that at any point on a circle, the radius drawn to that point is perpendicular to the tangent line at that point.
To verify the proposition, note that the gradient vector is in the same direction as the radius vector at any point $(x, y)$:
\[
\grad f(x,y) = \vector{2x, 2y} = 2\vector{x,y}
\]
For the case $k = 0$, the level curve is just the origin and at the origin, the gradient is the zero vector 
which is considered to be orthogonal to any vector.
\end{example}

\begin{problem}(Problem 1a)
Verify the proposition by showing directly that the gradient is orthogonal to the level curve  of the plane $z = f(x,y) = ax + by$ at any point $(x,y)$.
\begin{hint}
To find the direction vector of the line $ax + by = k$ rewrite the line as $\vec r(x) = \vector{x, \frac{k-ax}{b}}$
\end{hint}
\end{problem}


\begin{problem}(Problem 1b)
Verify the proposition by showing directly that the gradient is orthogonal to the level curve  of the hemisphere $z = f(x,y) = \sqrt{1 - x^2 - y^2}$ at any point $(x,y)$.
\begin{hint}
At any point on a circle, the tangent line is perpendicular to the radius.
\end{hint}
\end{problem}

Here is a video solution of problem 1:\\
\begin{foldable}
\youtube{QwuCfeUs2JU}
\end{foldable}

To create the normal vector to a surface at a point, we need the analogue of the previous proposition for level surfaces.

\begin{proposition}
Let $f(x,y,z)$ be a function of three variables and let $(x_0, y_0, z_0)$ be a point on the level surface $f(x,y, z) = k$.
Then, the gradient vector at this point, $\grad f(x_0, y_0, z_0)$ is orthogonal to the level surface.
\end{proposition}
\begin{proof}
Let $\vec r(t)$ be any smooth curve on the level surface $f(x,y, z) = k$ passing through the point $(x_0, y_0, z_0)$ with direction vector $\vec u$ at this point.
Since $f$ is constant on $\vec r(t)$, the directional derivative $D_{\vec u} f(x_0, y_0, z_0)$ is zero, and, as in the previous proposition, 
$\grad f(x_0, y_0, z_0) \perp \vec u$.  
Since the curve $\vec r(t)$ is an arbitrary curve on the surface passing through $(x_0, y_0, z_0)$, the gradient vector must be 
orthogonal to the surface itself at this point.
\end{proof}

\begin{example}[Example 2]
Verify the proposition by showing that the gradient vector is orthogonal to the level surfaces of $f(x, y, z) = x^2 + y^2 + z^2$ at any point.\\
The level surfaces have the form
\[
x^2 + y^2 + z^2 = k
\]
which are spheres centered at the origin with radius $\sqrt k$ (for $k>0$).
At any point $(x, y, z)$, the gradient vector is
\[
\grad f(x, y, z) = \vector{2x, 2y, 2z} = 2\vector{x, y, z}
\]
which is in the direction of the radius of the sphere at that point. Since the radius is orthogonal to the sphere at any point,
the gradient, $\grad f(x,y,z)$ is orthogonal to the level surface $f(x, y, z,) = k$ at any point, as claimed by the proposition.
\end{example}

\begin{problem}(Problem 2)
Verify the preceding proposition by showing directly that the gradient is orthogonal to the level curve  of $f(x,y, z) = ax + by + cz$ at any point $(x,y, z)$.
\begin{hint}
The level curves are planes with normal vector $\vector{a, b, c}$
\end{hint}
\end{problem}


\begin{theorem}[Tangent Plane]
The tangent plane to the surface $z = f(x,y)$ at the point $(x_0, y_0, z_0)$ is given by
\[
z = z_0 + f_x(x_0, y_0)(x - x_0) + f_y(x_0, y_0)(y - y_0)
\]
\end{theorem}
\begin{proof}
The surface $z = f(x,y)$ is the level surface $g(x,y,z) = 0$ where $g(x,y,z) = z - f(x,y)$.
According to the previous proposition, the vector $\grad g(x_0, y_0, z_0)$ is orthogonal to the surface at the point $(x_0, y_0, z_0)$.
Hence, this vector is the normal to the plane and the equation of the plane is
\[
\grad g(x_0, y_0, z_0) \dotp \vector{x- x_0, y-y_0, z-z_0} = 0
\]
Since $\grad g(x_0, y_0, z_0) = \vector{-f_x(x_0, y_0), -f_y(x_0, y_0), 1}$, 
the equation of the plane can be rewritten as
\[
-f_x(x_0, y_0)(x-x_0) - f_y(x_0, y_0)(y-y_0) + (z-z_0) = 0
\]
which in turn can be written as
\[
z = z_0 + f_x(x_0, y_0)(x-x_0) + f_y(x_0, y_0)(y-y_0)
\]
as claimed.
\end{proof}

\begin{corollary}
The equation of the tangent plane to a surface of the form $g(x, y, x) = 0$ at the point $(x_0, y_0, z_0)$ is given by
\[
\grad g(x_0, y_0, z_0) \dotp \vector{x - x_0, y - y_0, z - z_0} = 0
\]
\end{corollary}

\begin{example}[Example 3]
Find the equation of the tangent plane to the paraboloid $z = x^2 + y^2$ at the point $(3, -4, 25)$.\\
Write $g(x, y, z) = z - f(x,y) = 0$ and compute the gradient of $g$:
\[
\grad g(3, -4, 25) = \vector{-f_x(3, -4), -f_y(3, -4), 1} = \vector{-6, 8, 1}
\]
Then the equation of the tangent plane is
\[
\vector{-6, 8, 1} \dotp \vector{x-3, y+4, z-25} = 0
\]
which yields
\[
z = 25 + 6(x-3) - 8(y+4)
\]
or
\[
z = 6x - 8y - 25
\]
\end{example}

\begin{problem}(Problem 3a)
Find the equation of the tangent plane to the paraboloid $z = x^2 + y^2$ at the point $(-2, 1, 5)$.\\
\[
z = \answer{-5-4x+2y}
\]

\end{problem}


\begin{problem}(Problem 3b)
Find the equation of the tangent plane to the elliptic paraboloid $z = x^2 + 4y^2$ at the point $(4, -1, 20)$.\\
\[
z = \answer{-26 + 8x -8y}
\]
\end{problem}

Here is a video solution of problem 3b:\\
\begin{foldable}
\youtube{nMrN0PzH4s8}
\end{foldable}


\begin{example}[Example 4]
Find the equation of the tangent plane to the surface $z = \ln(x^2 + y^2)$ at the point $(-6, 8, 2\ln 10)$.\\
Write $g(x, y, z) = z - f(x,y) = 0$ and compute the gradient of $g$:
\[
\grad g(-6, 8, 2\ln 10) = \vector{-f_x(-6, 8), -f_y(-6, 8), 1} = \vector{-\frac{3}{25}, \frac{4}{25}, 1}
\]
Then the equation of the tangent plane is
\[
\vector{-\frac{3}{25}, \frac{4}{25}, 1} \dotp \vector{x+6, y-8, z-2\ln 10} = 0
\]
which yields
\[
z = 2\ln 10 - \frac{3}{25}(x+6) +\frac{4}{25}(y-8)
\]
\end{example}

\begin{problem}(Problem 4a)
Find the equation of the tangent plane to the hemisphere $z = \sqrt{50 -x^2 - y^2}$ at the point $(3, 4, 5)$.\\
\[
z = \answer{10-\frac35 x - \frac45 y}
\]

\end{problem}


\begin{problem}(Problem 4b)
Find the equation of the tangent plane to the surface $z =e^{xy}$ at the point $(2, 1, e^2)$.\\
\[
z = \answer{-3e^2 + e^2 x + 2e^2 y}
\]
\end{problem}

\begin{example}[Example 5]
Find the equation of the tangent plane to the hyperboloid of one sheet given by 
\[
\frac{x^2}{4} + \frac{y^2}{9} - \frac{z^2}{16} = 1
\]
at the point $(2, 3, 4)$.\\
Rewrite the surface as
\[
g(x,y,z) = \frac{x^2}{4} + \frac{y^2}{9} - \frac{z^2}{16} - 1 = 0
\]
Compute the gradient of $g$:
\[
\grad g(x,y,z) = \vector{\frac{x}{2} , \frac{2y}{9}, - \frac{z}{8}}
\]
and evaluate it at the given point:
\[
\grad g(2,3,4) = \vector{1, \frac{2}{3}, -\frac12}
\]
The equation of the tangent plane is given by 
\[
\grad g(2, 3, 4) \dotp \vector{x-2, y-3, z-4} = 0
\]
which gives
\[
(x-2) + \frac23 (y-3) - \frac12 (z-4) = 0
\]
or
\[
6x + 4y - 3z = 12
\]
\end{example}

\begin{problem}(Problem 5a)
Find the equation of the tangent plane to the ellipsoid given by 
\[
\frac{x^2}{12} + \frac{y^2}{6} + \frac{z^2}{8} = 1
\]
at the point $(2, -1, -2)$.\\
\[
\answer{2x-2y-3z} = 12
\]
\end{problem}

\begin{problem}(Problem 5b)
Find the equation of the tangent plane to the hyperboloid of two sheets given by 
\[
\frac{x^2}{8} + \frac{y^2}{32} - \frac{z^2}{8} = -1
\]
at the point $(2, 4, -4)$.\\
\[
\answer{2x+y + 4z} = -8
\]
\end{problem}

Here is a video solution of problem 5b:\\
\begin{foldable}
\youtube{gLRKxXYgDss}
\end{foldable}



\section{Linear Approximation}
We can use the equation of the tangent plane to approximate the values of a function $f(x,y)$ near the point of tangency.

Suppose the value $f(x_0, y_0)$ is known. The linear approximation to the function $f$ at a point $(x,y)$ near the point $(x_0, y_0)$
is given by
\[
f(x,y) \approx f(x_0, y_0) + f_x(x_0, y_0)(x-x_0) + f_y(x_0, y_0)(y-y_0)
\]

\begin{example}[Example 6]
The temperature $T$ (in Celsius) at a point $(x,y)$ on a metal plate is given by 
\[
T = x^2 - xy + 3y^2
\]
Use a linear approximation to estimate the temperature at the point $(2.95, -0.96)$.\\
The point $(2.95, -0.96)$ is near the point $(3,-1)$ where the temperature and its gradient are easily computed.
We have
\[
\grad T(x,y) = \vector{2x - y, 6y - x}
\]
and at the point $(3, -1)$ the gradient is
\[
\grad T(3, -1) = \vector{7, -9}
\]
Since $T(3, -1) = 9 + 3 + 3 = 15$, the linear approximation is given by
\begin{align*}
T = f(x,y) &\approx T(3, -1) + \grad T(3, -1) \dotp \vector{x-3, y+1}
           &= 15 + 7(x-3) - 9(y+1)\\
\end{align*}
Hence, the temperature at $(2.95, -0.96)$ is approximately
\[
T \approx 15 + 7(2.95 - 3) - 9(-0.96 + 1) = 14.29^\circ \text{C}
\]
\end{example}


\begin{problem}(Problem 6)
The body mass index $I$ of a person weighing $W$ kilograms that has a height $H$ meters is given by
\[
I = \frac{W}{H^2}
\]
Estimate the BMI of a person weighing $101.6$ kg with a height of $1.98$ meters.\\
The BMI of a person weighing $100$ kg with a height of $2$ meters is $I = \answer{25}$
\[
\grad I(W,H) = \vector{\answer{1/H^2}, \answer{-2W/H^3}}
\]
\[
\grad I(100, 2) = \vector{\answer{1/4}, \answer{-25}}
\]
The BMI of a person with weight $101.6$ kg and height $1.98$ meters is approximately (one decimal place)
\[
I \approx \answer{25.9}
\]
\end{problem}



\end{document}
