\documentclass[handout]{ximera}

\input{../preamble}

\outcome{Determine the behavior of an infinite series}

\title{3.9 Ratio Test}

\begin{document}

\begin{abstract}
Use the Ratio Test to determine whether an infinite series converges or diverges.
\end{abstract}

\maketitle

\section{Ratio Test}

In this section we will determine whether an infinite series converges or diverges using the Ratio Test. 
The idea behind this test is to determine if the given series is behaving similarly to a geometric series.
For a geometric series, 
\[
\sum_{n=0}^\infty a_n = \sum_{n=0}^\infty ar^n,
\]
the ratio of successive terms is constant, i.e., 
\[
\frac{a_{n+1}}{a_n} = \frac{ar^{n+1}}{ar^n} = r.
\]
Furthermore, a geometric series converges if this ratio is between $-1$ and $1$.
For a general series, the ratio of successive terms is not constant, but if the limit of the ratio of successive terms
approaches a value, $L$, between $-1$ and $1$, then the series behaves like a geometric series with ratio equal to $L$.
We state this precisely in the following theorem.

\begin{theorem}[Ratio Test]
For the series
\[
\sum_{n=0}^\infty a_n,
\]
let
\[
L = \lim_{n \to \infty} \left|\frac{a_{n+1}}{a_n}\right|.
\]
The series converges (absolutely) if $L < 1$ and diverges if $L>1$. 
If $L = 1,$ then no conclusion can be made.

\end{theorem}
 
\begin{remark}
For any $p$-series,
\[
\sum_{n=1}^\infty \frac{1}{n^p},
\]
\[
L =  \lim_{n \to \infty} \left|\frac{\frac{1}{(n+1)^p}}{\frac{1}{n^p}}\right| = \lim_{n \to \infty} \frac{n^p}{(n+1)^p} =  \lim_{n \to \infty} \left(\frac{n}{n+1}\right)^p = 1
\]
and so the ratio test gives no conclusion about $p$-series.
\end{remark}

\begin{example}[example 1]
Determine whether the series converges or diverges:
\[
\sum_{n=1}^\infty \frac{n}{2^n}.
\]

By the Ratio Test,
\[
L =  \lim_{n \to \infty} \left|\frac{\frac{n+1}{2^{n+1}}}{\frac{n}{2^n}}\right| =  \lim_{n \to \infty} \frac{(n+1)2^n}{n2^{n+1}} 
=  \lim_{n \to \infty} \frac{n+1}{2n} = \frac12.
\]
Since $L = 1/2 < 1$, the series converges.
\end{example}



\begin{problem}(problem 1a)
Determine whether the series converges or diverges:
\[
\sum_{n=1}^\infty \frac{n+2}{3^n}.
\]
\[
L = \lim_{n \to \infty} \left|\frac{a_{n+1}}{a_n}\right| = \answer{1/3}
\]
By the ratio test, this series \wordChoice{\choice[correct]{converges}
\choice{diverges}}

\end{problem}


\begin{problem}(problem 1b)
Determine whether the series converges or diverges:
\[
\sum_{n=1}^\infty \frac{2^n}{n^3}.
\]
\[
L = \lim_{n \to \infty} \left|\frac{a_{n+1}}{a_n}\right| = \answer{2}
\]
By the ratio test, this series \wordChoice{\choice{converges}
\choice[correct]{diverges}}

\end{problem}



\begin{problem}(problem 1c)
Determine whether the series converges or diverges:
\[
\sum_{n=1}^\infty \frac{n^2}{n^4 +1}.
\]
\[
L = \lim_{n \to \infty} \left|\frac{a_{n+1}}{a_n}\right| = \answer{1}
\]
By the ratio test, this series \wordChoice{\choice{converges}
\choice{diverges}\choice[correct]{no conclusion}}

\end{problem}


\begin{example}[example 2]
Determine whether the series converges or diverges:
\[
\sum_{n=1}^\infty (-1)^n\frac{n^2}{3^n}.
\]

By the Ratio Test,
\[
L =  \lim_{n \to \infty} \left|\frac{(-1)^{n+1}\frac{(n+1)^2}{3^{n+1}}}{(-1)^n\frac{n^2}{3^n}}\right| =  \lim_{n \to \infty} \frac{(n+1)^2 3^n}{n^2 3^{n+1}} 
=  \lim_{n \to \infty} \frac{(n+1)^2}{3n^2} = \frac13.
\]
Since $L = 1/3 < 1$, the series converges.
\end{example}





\begin{problem}(problem 2a)
Determine whether the series converges or diverges:
\[
\sum_{n=1}^\infty (-1)^n\frac{n}{2^n}.
\]
\[
L = \lim_{n \to \infty} \left|\frac{a_{n+1}}{a_n}\right| = \answer{1/2}
\]
By the ratio test, this series \wordChoice{\choice[correct]{converges}
\choice{diverges}}

\end{problem}



\begin{problem}(problem 2b)
Determine whether the series converges or diverges:
\[
\sum_{n=1}^\infty (-1)^n\frac{3^n}{2n+1}.
\]
\[
L = \lim_{n \to \infty} \left|\frac{a_{n+1}}{a_n}\right| = \answer{3}
\]
By the ratio test, this series \wordChoice{\choice{converges}
\choice[correct]{diverges}}

\end{problem}



\begin{example}[example 3]
Determine whether the series converges or diverges:
\[
\sum_{n=0}^\infty \frac{1}{n!}.
\]

By the Ratio Test,
\[
L =  \lim_{n \to \infty} \left|\frac{\frac{1}{(n+1)!}}{\frac{1}{n!}}\right| =  \lim_{n \to \infty} \frac{n!}{(n+1)!} =  \lim_{n \to \infty} \frac{1}{n+1} = 0.
\]
Since $L = 0 < 1$, the series converges.
\end{example}



\begin{problem}(problem 3a)
Determine whether the series converges or diverges:
\[
\sum_{n=0}^\infty \frac{2^n}{n!}.
\]
\[
L = \lim_{n \to \infty} \left|\frac{a_{n+1}}{a_n}\right| = \answer{0}
\]
By the ratio test, this series \wordChoice{\choice[correct]{converges}
\choice{diverges}}

\end{problem}



\begin{problem}(problem 3b)
Determine whether the series converges or diverges:
\[
\sum_{n=0}^\infty (-1)^n\frac{n!}{10^n}.
\]
\[
L = \lim_{n \to \infty} \left|\frac{a_{n+1}}{a_n}\right| = \answer{\infty}
\]
By the ratio test, this series \wordChoice{\choice{converges}
\choice[correct]{diverges}}

\end{problem}

\begin{example}[example 4]
Determine whether the series converges or diverges:
\[
\sum_{n=1}^\infty \frac{n^5 10^{n+1}}{(2n)!}.
\]

By the Ratio Test,
\[
L =  \lim_{n \to \infty} \left|\frac{\frac{(n+1)^5 10^{n+2}}{(2n+2)!}}{\frac{n^5 10^{n+1}}{(2n)!}}\right| 
=  \lim_{n \to \infty} \frac{(n+1)^5 10^{n+2}(2n)!}{n^5 10^{n+1}(2n+2)!}
\]
\[
 =  \lim_{n \to \infty} \frac{(n+1)^5}{n^5} \cdot \frac{10^{n+2}}{10^{n+1}} \cdot \frac{(2n)!}{(2n+2)!} 
 \]
 \[
 = 
  \lim_{n \to \infty} \left(\frac{n+1}{n}\right)^5 \cdot 10 \cdot \frac{1}{(2n+2)(2n+1)} = 1 \cdot 10 \cdot 0 = 0.
\]
Since $L = 0 < 1$, the series converges.
\end{example}


\begin{problem}(problem 4)
Determine whether the series converges or diverges:
\[
\sum_{n=0}^\infty \frac{(n+1)4^n}{n!}.
\]
\[
L = \lim_{n \to \infty} \left|\frac{a_{n+1}}{a_n}\right| = \answer{0}
\]
By the ratio test, this series \wordChoice{\choice[correct]{converges}
\choice{diverges}}

\end{problem}






\begin{example}[example 5]
Determine whether the series converges or diverges:
\[
\sum_{n=1}^\infty \frac{n!}{n^n}.
\]


By the Ratio Test,
\[
L =  \lim_{n \to \infty} \left|\frac{\frac{(n+1)!}{(n+1)^{n+1}}}{\frac{n!}{n^n}}\right| = 
\lim_{n \to \infty} \frac{(n+1)!}{(n+1)^{n+1}}\cdot \frac{n^n}{n!}
=  \lim_{n \to \infty} \frac{(n+1)!}{n!} \cdot  \frac{n^n}{(n+1)^n}\cdot \frac{1}{n+1}
\]
\[
= \lim_{n \to \infty} (n+1) \cdot \left(\frac{n}{n+1}\right)^n \cdot \frac{1}{n+1} = \lim_{n \to \infty} \left(\frac{n}{n+1}\right)^n = \frac{1}{e}.
\]


Since $L = 1/e < 1$, the series converges.

\begin{remark}
We used the famous limit:
\[
\lim_{n \to \infty} \left(\frac{n+1}{n}\right)^n = \lim_{n \to \infty} \left(1 + \frac{1}{n}\right)^n = e.
\]
\end{remark}


\end{example}



\begin{problem}(problem 5)
Determine whether the series converges or diverges:
\[
\sum_{n=1}^\infty \frac{(n!)^2}{(2n)!}.
\]
\[
L = \lim_{n \to \infty} \left|\frac{a_{n+1}}{a_n}\right| = \answer{1/4}
\]
By the ratio test, this series \wordChoice{\choice[correct]{converges}
\choice{diverges}}

\end{problem}




\section{Video Lessons}

Click on the arrow head in the blue box to reveal the videos.\\

Here is Dr. Incognito's video:
\begin{expandable}
\begin{center}
\youtube{XmNK0SK2bO4}
\end{center}
\end{expandable}

Here is the Khan Academy Video:
\begin{expandable}
\begin{center}
\youtube{av947KCWf2U}
\end{center}
\end{expandable}

Here is an MIT video:
\begin{expandable}
\begin{center}
\youtube{rUis1mSzwyA}
\end{center}
\end{expandable}

\end{document}








\begin{center}
\begin{foldable}
Here is a detailed, lecture style video on the Ratio Test:
\youtube{XmNK0SK2bO4}
\end{foldable}
\end{center}


\begin{center}
\begin{expandable}
\foldable{Here is a detailed, lecture style video on the Ratio Test:}
\youtube{XmNK0SK2bO4}
\end{expandable}
\end{center}















\begin{example} %example #15
Find $h'(x)$ if $h(x) = x^{\sin(x)}$.\\
We will use the fact that the exponential and logarithm functions are inverses,
\[e^{\ln(x)} = x,\]
and the exponent property of logarithms, 
\[\ln(x^n) = n\ln(x),\]
to rewrite $h(x)$.  We have 
\[h(x) = x^{\sin(x)} = e^{\ln(x^{\sin(x)})} = e^{\sin(x)\ln(x)}\]
and we can now compute $h'(x)$ using a combination of the chain rule and product rule.
We can write $h(x)$ as a composition, $f(g(x))$ with 
\[g(x) = \sin(x)\ln(x) \quad \text{and} \quad f(x) = e^x.\]
Then to find $g'(x)$ we us the product rule and we get $g'(x) = \frac{\sin(x)}{x} + \cos(x)\ln(x)$.
Next $f'(x) = e^x$ and 
hence $f'(g(x)) = e^{g(x)} = e^{\sin(x)\ln(x)} = x^{\sin(x)}$.
We can then conclude $h'(x) = f'(g(x))g'(x) = x^{\sin(x)} \left[ \frac{\sin(x)}{x} + \cos(x)\ln(x)\right]$.
\end{example}

%more question formats below













%\begin{verbatim}
\begin{question}
What is your favorite color?
\begin{multipleChoice}
\choice[correct]{Rainbow}
\choice{Blue}
\choice{Green}
\choice{Red}
\end{multipleChoice}
\begin{freeResponse}
Hello
\end{freeResponse}
\end{question}
%\end{verbatim}





\begin{question}
  Which one will you choose?
  \begin{multipleChoice}
    \choice[correct]{I'm correct.}
    \choice{I'm wrong.}
    \choice{I'm wrong too.}
  \end{multipleChoice}
\end{question}


\begin{question}
  Which one will you choose?
  \begin{selectAll}
    \choice[correct]{I'm correct.}
    \choice{I'm wrong.}
    \choice[correct]{I'm also correct.}
    \choice{I'm wrong too.}
  \end{selectAll}
\end{question}


\begin{freeResponse}
What is the chain rule used for?
\end{freeResponse}
